@prefix : <http://www.semanticweb.org/ontologies/2022/6/geological_taxonomy#> .
@prefix owl: <http://www.w3.org/2002/07/owl#> .
@prefix rdf: <http://www.w3.org/1999/02/22-rdf-syntax-ns#> .
@prefix xml: <http://www.w3.org/XML/1998/namespace> .
@prefix xsd: <http://www.w3.org/2001/XMLSchema#> .
@prefix rdfs: <http://www.w3.org/2000/01/rdf-schema#> .
@base <http://www.w3.org/2002/07/owl#> .

[ rdf:type owl:Ontology
 ] .

#################################################################
#    Classes
#################################################################

###  http://www.semanticweb.org/ontologies/2022/6/geological_taxonomy#Abnormally_Dry
:Abnormally_Dry rdf:type owl:Class ;
                rdfs:subClassOf :Drought ;
                rdfs:comment """It is the D0 category that refers short-term dryness slowing planting, growth of crops or pastures.

Resource: https://droughtmonitor.unl.edu/About/WhatistheUSDM.aspx""" .


###  http://www.semanticweb.org/ontologies/2022/6/geological_taxonomy#Adakite
:Adakite rdf:type owl:Class ;
         rdfs:subClassOf :Basalt ;
         rdfs:comment """A class of basaltic rocks containing low yttrium and ytterbium

Resource: https://geology.fandom.com/wiki/List_of_rock_types""" .


###  http://www.semanticweb.org/ontologies/2022/6/geological_taxonomy#Albolls
:Albolls rdf:type owl:Class ;
         rdfs:subClassOf :Mollisols ;
         rdfs:comment """Albolls have a bleached subsurface horizon called the albic horizon and are usually wet

Resource: https://www.sciencedirect.com/topics/agricultural-and-biological-sciences/mollisol""" .


###  http://www.semanticweb.org/ontologies/2022/6/geological_taxonomy#Alfisols
:Alfisols rdf:type owl:Class ;
          rdfs:subClassOf :Soil ;
          rdfs:comment """The central concept of Alfisols is that of soils that have an argillic, a kandic, or a natric horizon and a base saturation of 35% or greater.

Resource: https://www.nrcs.usda.gov/wps/portal/nrcs/detail/soils/survey/class/maps/?cid=nrcs142p2_053590

Justification: Depending upon soil Moisture regimes""" .


###  http://www.semanticweb.org/ontologies/2022/6/geological_taxonomy#Alkali_feldspar_granite
:Alkali_feldspar_granite rdf:type owl:Class ;
                         rdfs:subClassOf :Igneous_rocks ;
                         rdfs:comment """Alkali feldspar granite, some varieties of which are called 'red granite', is a felsic igneous rock and a type of granite rich in the mineral potassium feldspar (K-spar).

Resource: https://en.wikipedia.org/wiki/Alkali_feldspar_granite""" .


###  http://www.semanticweb.org/ontologies/2022/6/geological_taxonomy#Amphibolite
:Amphibolite rdf:type owl:Class ;
             rdfs:subClassOf :Metamorphic_rocks ;
             rdfs:comment """A metamorphic rock containing mainly amphibole and plagioclase

Resource: https://en.wikipedia.org/wiki/List_of_rock_types""" .


###  http://www.semanticweb.org/ontologies/2022/6/geological_taxonomy#Andesite
:Andesite rdf:type owl:Class ;
          rdfs:subClassOf :Igneous_rocks ;
          rdfs:comment """Andesite is a volcanic rock of intermediate composition.

Resource: https://en.wikipedia.org/wiki/Andesite""" .


###  http://www.semanticweb.org/ontologies/2022/6/geological_taxonomy#Andisols
:Andisols rdf:type owl:Class ;
          rdfs:subClassOf :Soil ;
          rdfs:comment """The central concept of Andisols is that of soils dominated by short-range-order minerals. They include weakly weathered soils with much volcanic glass as well as more strongly weathered soils.

Resource: https://www.nrcs.usda.gov/wps/portal/nrcs/detail/soils/survey/class/maps/?cid=nrcs142p2_053592

Justification: These suborders are defined based on soil temperature and soil moisture regimes.
https://www.nasa.gov/centers/johnson/pdf/486016main_Takahashi.pdf""" .


###  http://www.semanticweb.org/ontologies/2022/6/geological_taxonomy#Anorthosite
:Anorthosite rdf:type owl:Class ;
             rdfs:subClassOf :Igneous_rocks ;
             rdfs:comment """An intrusive igneous felsic rock composed predominantly of plagioclase

Resource: https://geology.fandom.com/wiki/Anorthosite""" .


###  http://www.semanticweb.org/ontologies/2022/6/geological_taxonomy#Anthracite
:Anthracite rdf:type owl:Class ;
            rdfs:subClassOf :Metamorphic_rocks ;
            rdfs:comment """Anthracite is a type of coal with a highest rank. Coal rank measures the carbon content which is in correlation with calorific value and metamorphic grade.

Resource: https://www.sandatlas.org/rock-types/#Anthracite""" .


###  http://www.semanticweb.org/ontologies/2022/6/geological_taxonomy#Anthrepts
:Anthrepts rdf:type owl:Class ;
           rdfs:subClassOf :Inceptisols ;
           rdfs:comment """Inceptisols that have a plaggen or anthropic epipedon

Resource: https://sites.google.com/site/dinpuithai/Home/key10/key10k""" .


###  http://www.semanticweb.org/ontologies/2022/6/geological_taxonomy#Aplite
:Aplite rdf:type owl:Class ;
        rdfs:subClassOf :Igneous_rocks ;
        rdfs:comment """Aplite is an intrusive igneous rock in which the mineral composition is the same as granite, but in which the grains are much finer, under 1 mm across.

Resource: https://en.wikipedia.org/wiki/Aplite""" .


###  http://www.semanticweb.org/ontologies/2022/6/geological_taxonomy#Aqualfs
:Aqualfs rdf:type owl:Class ;
         rdfs:subClassOf :Alfisols ;
         rdfs:comment """In the horizons that have aquic conditions, enough active ferrous iron to give a positive reaction to alpha,alphadipyridyl at a time when the soil is not being irrigated.

Resource: https://sites.google.com/site/dinpuithai/Home/taxonomy/j-alfisols""" .


###  http://www.semanticweb.org/ontologies/2022/6/geological_taxonomy#Aquands
:Aquands rdf:type owl:Class ;
         rdfs:subClassOf :Andisols ;
         rdfs:comment """Andisols with a water table at or near the surface for much of the year.

Resource: https://en.wikipedia.org/wiki/Andisol""" .


###  http://www.semanticweb.org/ontologies/2022/6/geological_taxonomy#Aquents
:Aquents rdf:type owl:Class ;
         rdfs:subClassOf :Entisols ;
         rdfs:comment """Wet Entisols (aquic conditions in the upper part)

Resource: \"Illustrated Guide to Soil Taxonomy\" book by Unites States Department of Agriculture""" .


###  http://www.semanticweb.org/ontologies/2022/6/geological_taxonomy#Aquepts
:Aquepts rdf:type owl:Class ;
         rdfs:subClassOf :Inceptisols ;
         rdfs:comment """They show redoximorphic features and are saturated with water at some period in the year. Aquepts usually have cambic horizons and commonly in the US, they have fragipans

Resource: https://web.archive.org/web/20040918225129/http://grunwald.ifas.ufl.edu/Nat_resources/soil_orders/inceptisols.htm""" .


###  http://www.semanticweb.org/ontologies/2022/6/geological_taxonomy#Aquerts
:Aquerts rdf:type owl:Class ;
         rdfs:subClassOf :Vertisols ;
         rdfs:comment """Vertisols that have, in one or more horizons within 50 cm of the mineral soil surface, aquic conditions for some time in normal years (or artificial drainage)

Resource: https://sites.google.com/site/dinpuithai/Home/key10/key10f""" .


###  http://www.semanticweb.org/ontologies/2022/6/geological_taxonomy#Aquods
:Aquods rdf:type owl:Class ;
        rdfs:subClassOf :Spodosols ;
        rdfs:comment """Wet Spodosols (aquic conditions in the upper part)

Resource: \"Illustrated Guide to Soil Taxonomy\" book by Unites States Department of Agriculture""" .


###  http://www.semanticweb.org/ontologies/2022/6/geological_taxonomy#Aquolls
:Aquolls rdf:type owl:Class ;
         rdfs:subClassOf :Mollisols ;
         rdfs:comment """Aquolls are wet Mollisols and may have a histic epipedon

Resource: https://www.sciencedirect.com/topics/agricultural-and-biological-sciences/mollisol""" .


###  http://www.semanticweb.org/ontologies/2022/6/geological_taxonomy#Aquox
:Aquox rdf:type owl:Class ;
       rdfs:subClassOf :Oxisols ;
       rdfs:comment """Oxisols that have aquic conditions for some time in normal years (or artificial drainage) in one or more horizons within 50 cm of the mineral soil surface

Resource: https://sites.google.com/site/dinpuithai/Home/key10/key10e""" .


###  http://www.semanticweb.org/ontologies/2022/6/geological_taxonomy#Aquults
:Aquults rdf:type owl:Class ;
         rdfs:subClassOf :Ultisols ;
         rdfs:comment """Ultisols that have aquic conditions for some time in normal years (or artificial drainage) in one or more horizons within 50 cm of the mineral soil surface

Resource: https://sites.google.com/site/dinpuithai/Home/key10/key10h""" .


###  http://www.semanticweb.org/ontologies/2022/6/geological_taxonomy#Areal
:Areal rdf:type owl:Class ;
       rdfs:subClassOf :Floods ;
       rdfs:comment """Areal floods are caused when excessive snowmelt or high rainfall accumulates on land, sometimes to hazardous depths	

Resource: https://www.worldatlas.com/articles/how-many-types-of-floods-are-there.html""" .


###  http://www.semanticweb.org/ontologies/2022/6/geological_taxonomy#Arents
:Arents rdf:type owl:Class ;
        rdfs:subClassOf :Entisols ;
        rdfs:comment """Entisols that have, in one or more layers at a depth between 25 and 100 cm below the mineral soil surface, 3 percent or more (by volume) fragments of diagnostic horizons that are not arranged in any discernible order.

Resource: https://sites.google.com/site/dinpuithai/Home/key10/key10l""" .


###  http://www.semanticweb.org/ontologies/2022/6/geological_taxonomy#Argids
:Argids rdf:type owl:Class ;
        rdfs:subClassOf :Aridisols ;
        rdfs:comment """Characterized by an accumulation of clay by translocation, the Argids are present in areas adjoining soils with an ustic SMR.

Resource: https://www.sciencedirect.com/topics/agricultural-and-biological-sciences/aridisol""" .


###  http://www.semanticweb.org/ontologies/2022/6/geological_taxonomy#Argillite
:Argillite rdf:type owl:Class ;
           rdfs:subClassOf :Sedimentary_rocks ;
           rdfs:comment """Sedimentary rock, mostly of indurated clay particles

Resource: https://en.wikipedia.org/wiki/List_of_rock_types""" .


###  http://www.semanticweb.org/ontologies/2022/6/geological_taxonomy#Aridisols
:Aridisols rdf:type owl:Class ;
           rdfs:subClassOf :Soil ;
           rdfs:comment """The central concept of Aridisols is that of soils that are too dry for mesophytic plants to grow.

Resource: https://www.nrcs.usda.gov/wps/portal/nrcs/detail/soils/survey/class/maps/?cid=nrcs142p2_053594

Justification: Depending upon the composition and accumulation of the soluble fraction and results of dominant soil-forming processes.
https://www.sciencedirect.com/topics/agricultural-and-biological-sciences/aridisol""" .


###  http://www.semanticweb.org/ontologies/2022/6/geological_taxonomy#Arkose
:Arkose rdf:type owl:Class ;
        rdfs:subClassOf :Sedimentary_rocks ;
        rdfs:comment """A sedimentary rock similar to sandstone

Resource: https://geology.fandom.com/wiki/List_of_rock_types""" .


###  http://www.semanticweb.org/ontologies/2022/6/geological_taxonomy#Asthenosphere
:Asthenosphere rdf:type owl:Class ;
               rdfs:subClassOf :Upper_mantle ;
               rdfs:comment """layer in Earth's mantle between the lithosphere (above) and the upper mantle (below). It is the weak and easily deformed layer of the Earth that acts as a “lubricant” for the tectonic plates to slide over.

Resource: https://education.nationalgeographic.org/resource/mantle
http://ser.sese.asu.edu/GEO110/GEO110_S03/Dis2b.pdf""" .


###  http://www.semanticweb.org/ontologies/2022/6/geological_taxonomy#Banded_iron_formation
:Banded_iron_formation rdf:type owl:Class ;
                       rdfs:subClassOf :Sedimentary_rocks ;
                       rdfs:comment """A fine grained chemical sedimentary rock composed of iron oxide minerals

Resource: https://geology.fandom.com/wiki/List_of_rock_types""" .


###  http://www.semanticweb.org/ontologies/2022/6/geological_taxonomy#Basalt
:Basalt rdf:type owl:Class ;
        rdfs:subClassOf :Igneous_rocks ;
        rdfs:comment """Basalt is an aphanitic (fine-grained) extrusive igneous rock formed from the rapid cooling of low-viscosity lava rich in magnesium and iron exposed at or very near the surface of a rocky planet or moon.

Resource: https://en.wikipedia.org/wiki/Basalt

Justification: Depending upon the type of the flow of Basaltic lava and different formation process from basalt""" .


###  http://www.semanticweb.org/ontologies/2022/6/geological_taxonomy#Basaltic_trachyandesite
:Basaltic_trachyandesite rdf:type owl:Class ;
                         rdfs:subClassOf :Trachyandesite ;
                         rdfs:comment """A alkaline/basic rocktype intermediate between andesite and phonolite, difficult to define without the TAS diagram.

Resource: https://www.mindat.org/min-48461.html""" .


###  http://www.semanticweb.org/ontologies/2022/6/geological_taxonomy#Basanite
:Basanite rdf:type owl:Class ;
          rdfs:subClassOf :Igneous_rocks ;
          rdfs:comment """Basanite is an igneous, volcanic (extrusive) rock with aphanitic to porphyritic texture.

Resource: https://en.wikipedia.org/wiki/Basanite""" .


###  http://www.semanticweb.org/ontologies/2022/6/geological_taxonomy#Bauxite
:Bauxite rdf:type owl:Class ;
         rdfs:subClassOf :Sedimentary_rocks ;
         rdfs:comment """Bauxite is an aluminum-rich sedimentary rock. It is a principal ore of aluminum.

Resource: https://www.sandatlas.org/rock-types/""" .


###  http://www.semanticweb.org/ontologies/2022/6/geological_taxonomy#Benmoreite
:Benmoreite rdf:type owl:Class ;
            rdfs:subClassOf :Trachyandesite ;
            rdfs:comment """Benmoreite is a silica-undersaturated volcanic rock of intermediate composition.

Resource: https://en.wikipedia.org/wiki/List_of_rock_types""" .


###  http://www.semanticweb.org/ontologies/2022/6/geological_taxonomy#Blairmorite
:Blairmorite rdf:type owl:Class ;
             rdfs:subClassOf :Igneous_rocks ;
             rdfs:comment """Blairmorite is a very rare porphyritic volcanic rock named after the community of Blairmore in southwestern Alberta, Canada.

Resource: https://en.wikipedia.org/wiki/Blairmorite""" .


###  http://www.semanticweb.org/ontologies/2022/6/geological_taxonomy#Blizzards
:Blizzards rdf:type owl:Class ;
           rdfs:subClassOf :Extratropical_cyclone ;
           owl:disjointWith <http://www.semanticweb.org/ontologies/2022/6/geological_taxonomy#Nor'easter> ;
           rdfs:comment """A blizzard is a severe snowstorm characterized by strong sustained winds and low visibility, lasting for a prolonged period of time

Resource: https://en.wikipedia.org/wiki/Blizzard""" .


###  http://www.semanticweb.org/ontologies/2022/6/geological_taxonomy#Block_slide
:Block_slide rdf:type owl:Class ;
             rdfs:subClassOf :Translational_slide ;
             rdfs:comment """translational slide in which the moving mass consists of a single unit or a few closely related units that move downslope as a relatively coherent mass

Resource: https://pubs.usgs.gov/fs/2004/3072/pdf/fs2004-3072.pdf

Justification: Based on the type of material""" .


###  http://www.semanticweb.org/ontologies/2022/6/geological_taxonomy#Blueschist
:Blueschist rdf:type owl:Class ;
            rdfs:subClassOf :Metamorphic_rocks ;
            rdfs:comment """A metamorphic rock composed of sodic amphiboles with a distinct blue color

Resource: https://geology.fandom.com/wiki/List_of_rock_types""" .


###  http://www.semanticweb.org/ontologies/2022/6/geological_taxonomy#Bog_iron
:Bog_iron rdf:type owl:Class ;
          rdfs:subClassOf :Sedimentary_rocks ;
          rdfs:comment """Bog iron is a type of iron ore composed of limonite with impurities like clay or plant debris.

Resource: https://www.sandatlas.org/rock-types/""" .


###  http://www.semanticweb.org/ontologies/2022/6/geological_taxonomy#Boninite
:Boninite rdf:type owl:Class ;
          rdfs:subClassOf :Igneous_rocks ;
          rdfs:comment """Boninite is an extrusive rock high in both magnesium and silica, thought to be usually formed in fore-arc environments, typically during the early stages of subduction. 

Resource: https://en.wikipedia.org/wiki/Boninite""" .


###  http://www.semanticweb.org/ontologies/2022/6/geological_taxonomy#Borates
:Borates rdf:type owl:Class ;
         rdfs:subClassOf :Mineral ;
         rdfs:comment """Borate mineral, any of various naturally occurring compounds of boron and oxygen.	

Resource: https://www.britannica.com/science/borate-mineral""" .


###  http://www.semanticweb.org/ontologies/2022/6/geological_taxonomy#Breaching_of_a_barrier
:Breaching_of_a_barrier rdf:type owl:Class ;
                        rdfs:subClassOf :Coastal_Floods ;
                        rdfs:comment """Breaching occurs when the barrier is broken down or destroyed by waves allowing the seawater to extend inland and flood the areas	

Resource: https://en.wikipedia.org/wiki/Coastal_flooding""" .


###  http://www.semanticweb.org/ontologies/2022/6/geological_taxonomy#Breccia
:Breccia rdf:type owl:Class ;
         rdfs:subClassOf :Sedimentary_rocks ;
         rdfs:comment """A sedimentary or tectonic rock composed of fragments of other, broken rocks

Resource: https://geology.fandom.com/wiki/List_of_rock_types""" .


###  http://www.semanticweb.org/ontologies/2022/6/geological_taxonomy#Calcarenite
:Calcarenite rdf:type owl:Class ;
             rdfs:subClassOf :Sedimentary_rocks ;
             rdfs:comment """A clastic sedimentary rock that is made up predominantly of recycled carbonate particles of sand size; a consolidated calcareous sand

Resource: https://mrdata.usgs.gov/geology/state/sgmc-lith.php?text=calcarenite""" .


###  http://www.semanticweb.org/ontologies/2022/6/geological_taxonomy#Calcflinta
:Calcflinta rdf:type owl:Class ;
            rdfs:subClassOf :Hornfels ;
            rdfs:comment """Calcflinta, or calc-flinta, is a fine grained calc–silicate rock found amongst the metamorphic rocks of the eastern Highlands of Scotland

Resource: https://en.wikipedia.org/wiki/Calcflinta""" .


###  http://www.semanticweb.org/ontologies/2022/6/geological_taxonomy#Calcids
:Calcids rdf:type owl:Class ;
         rdfs:subClassOf :Aridisols ;
         rdfs:comment """Characterized by an accumulation of carbonates, the soils have a calcic, petrocalcic, or a hypercalcic horizon.

Resource: https://www.sciencedirect.com/topics/agricultural-and-biological-sciences/aridisol""" .


###  http://www.semanticweb.org/ontologies/2022/6/geological_taxonomy#Cambids
:Cambids rdf:type owl:Class ;
         rdfs:subClassOf :Aridisols ;
         rdfs:comment """Characterized by a transformation of material, these soils are the most extensive of the Aridisols

Resource: https://www.sciencedirect.com/topics/agricultural-and-biological-sciences/aridisol""" .


###  http://www.semanticweb.org/ontologies/2022/6/geological_taxonomy#Carbonates
:Carbonates rdf:type owl:Class ;
            rdfs:subClassOf :Mineral ;
            rdfs:comment """The carbonate minerals are those in which the main anionic group is carbonate, [CO3]2−	

Resource: https://en.wikipedia.org/wiki/Mineral#Classification

Justification: classified based on the presence of hydroxyl anion(OH-)""" .


###  http://www.semanticweb.org/ontologies/2022/6/geological_taxonomy#Carbonatite
:Carbonatite rdf:type owl:Class ;
             rdfs:subClassOf :Igneous_rocks ;
             rdfs:comment """Carbonatite is a type of intrusive or extrusive igneous rock defined by mineralogic composition consisting of greater than 50% carbonate minerals. 

Resource: https://en.wikipedia.org/wiki/Carbonatite""" .


###  http://www.semanticweb.org/ontologies/2022/6/geological_taxonomy#Cataclasite
:Cataclasite rdf:type owl:Class ;
             rdfs:subClassOf :Metamorphic_rocks ;
             rdfs:comment """Cataclasite is a metamorphic rock that is formed by mechanical shear stress during faulting.

Resource: https://www.chemeurope.com/en/encyclopedia/Cataclasite.html""" .


###  http://www.semanticweb.org/ontologies/2022/6/geological_taxonomy#Chalk
:Chalk rdf:type owl:Class ;
       rdfs:subClassOf :Sedimentary_rocks ;
       rdfs:comment """A sedimentary rock composed primarily of coccolith fossils

Resource: https://geology.fandom.com/wiki/List_of_rock_types""" .


###  http://www.semanticweb.org/ontologies/2022/6/geological_taxonomy#Charnockite
:Charnockite rdf:type owl:Class ;
             rdfs:subClassOf :Igneous_rocks ;
             rdfs:comment """Charnockite, any member of a series of metamorphic rocks with variable chemical composition, first described from the state of Tamil Nadu in southern India and named for Job Charnock. 

Resource: https://www.britannica.com/science/charnockite

Justification: Classified based on presence of quartz, pyroxene.""" .


###  http://www.semanticweb.org/ontologies/2022/6/geological_taxonomy#Chert
:Chert rdf:type owl:Class ;
       rdfs:subClassOf :Sedimentary_rocks ;
       rdfs:comment """A fine grained chemical sedimentary rock composed of silica

Resource: https://geology.fandom.com/wiki/List_of_rock_types""" .


###  http://www.semanticweb.org/ontologies/2022/6/geological_taxonomy#Claystone
:Claystone rdf:type owl:Class ;
           rdfs:subClassOf :Sedimentary_rocks ;
           rdfs:comment """A sedimentary rock formed from clay

Resource: https://geology.fandom.com/wiki/List_of_rock_types""" .


###  http://www.semanticweb.org/ontologies/2022/6/geological_taxonomy#Cloudy
:Cloudy rdf:type owl:Class ;
        rdfs:subClassOf :Weather_conditions ;
        rdfs:comment """Cloudy weather is when a significant amount of clouds is covering the sky (at least half the sky).

Resource: https://weather.fandom.com/wiki/Types_of_Weather#Cloudy

Justification: Classified based on the covering of sky by clouds""" .


###  http://www.semanticweb.org/ontologies/2022/6/geological_taxonomy#Coal
:Coal rdf:type owl:Class ;
      rdfs:subClassOf :Sedimentary_rocks ;
      rdfs:comment """A sedimentary rock formed from organic matter

Resource: https://geology.fandom.com/wiki/List_of_rock_types""" .


###  http://www.semanticweb.org/ontologies/2022/6/geological_taxonomy#Coastal_Floods
:Coastal_Floods rdf:type owl:Class ;
                rdfs:subClassOf :Floods ;
                rdfs:comment """Coastal flooding normally occurs when dry and low-lying land is submerged by seawater.

Resource: https://en.wikipedia.org/wiki/Coastal_flooding

Justification: Classified based on how seawater enters the land""" .


###  http://www.semanticweb.org/ontologies/2022/6/geological_taxonomy#Cold_wave
:Cold_wave rdf:type owl:Class ;
           rdfs:subClassOf :Extreme_Temperature ;
           owl:disjointWith :Heat_wave ;
           rdfs:comment """A period of abnormally cold weather.

Resource: http://desinventar.cimafoundation.org/definitions.html""" .


###  http://www.semanticweb.org/ontologies/2022/6/geological_taxonomy#Collapse_Earthquakes
:Collapse_Earthquakes rdf:type owl:Class ;
                      rdfs:subClassOf :Earthquakes ;
                      rdfs:comment """A collapse earthquake are small earthquakes in underground caverns and mines that are caused by seismic waves produced from the explosion of rock on the surface.

Resource: https://www.un-spider.org/category/disaster-type/earthquake""" .


###  http://www.semanticweb.org/ontologies/2022/6/geological_taxonomy#Comendite
:Comendite rdf:type owl:Class ;
           rdfs:subClassOf :Rhyolite ;
           owl:disjointWith :Pantellerite ;
           rdfs:comment """Hard, peralkaline igneous rock, a type of light blue grey rhyolite

Resource: https://en.wikipedia.org/wiki/List_of_rock_types""" .


###  http://www.semanticweb.org/ontologies/2022/6/geological_taxonomy#Conglomerate
:Conglomerate rdf:type owl:Class ;
              rdfs:subClassOf :Sedimentary_rocks ;
              rdfs:comment """A sedimentary rock composed of large rounded fragments of other rocks

Resource: https://geology.fandom.com/wiki/List_of_rock_types

Justification: Depending upon the method of deposition.""" .


###  http://www.semanticweb.org/ontologies/2022/6/geological_taxonomy#Continental_crust
:Continental_crust rdf:type owl:Class ;
                   rdfs:subClassOf :Crust ;
                   owl:disjointWith :Oceanic_crust ;
                   rdfs:comment """layer of rocks that forms the continents and the areas of shallow seabed close to their shores, known as continental shelves, is less dense and composed of (felsic) sodium potassium aluminium silicate rocks, like granite.

Resource: https://en.wikipedia.org/wiki/Continental_crust""" .


###  http://www.semanticweb.org/ontologies/2022/6/geological_taxonomy#Continental_lithosphere
:Continental_lithosphere rdf:type owl:Class ;
                         rdfs:subClassOf :Lithosphere ;
                         owl:disjointWith :Oceanic_lithosphere ;
                         rdfs:comment """Continental lithosphere is associated with continental crust and underlies the continents and continental shelfs.

Resource: https://en.wikipedia.org/wiki/Lithosphere""" .


###  http://www.semanticweb.org/ontologies/2022/6/geological_taxonomy#Continuous_creep
:Continuous_creep rdf:type owl:Class ;
                  rdfs:subClassOf :Creep ;
                  rdfs:comment """Shear stress continuously exceeds the strength of the material(rock debris and soil)

Resource: https://www.nature.scot/landforms-and-geology/scotlands-rocks-landforms-and-soils/landforms/landslides/types-landslide
https://courses.lumenlearning.com/geo/chapter/reading-slump-and-creep/""" .


###  http://www.semanticweb.org/ontologies/2022/6/geological_taxonomy#Coquina
:Coquina rdf:type owl:Class ;
         rdfs:subClassOf :Sedimentary_rocks ;
         rdfs:comment """A sedimentary carbonate rock formed by accumulation of abundant shell fossils and fragments

Resource: https://geology.fandom.com/wiki/List_of_rock_types""" .


###  http://www.semanticweb.org/ontologies/2022/6/geological_taxonomy#Creep
:Creep rdf:type owl:Class ;
       rdfs:subClassOf :Flows ;
       owl:disjointWith :Lateral_Spreads ;
       rdfs:comment """slow downslope movement of particles that occurs on every slope covered with loose, weathered material.

Resource: https://www.britannica.com/science/creep-slope-movement

Justification: Classification based on the effects of seasonal changes, gravitational force, point of failure""" .


###  http://www.semanticweb.org/ontologies/2022/6/geological_taxonomy#Crown_Fire
:Crown_Fire rdf:type owl:Class ;
            rdfs:subClassOf :Wildfire ;
            rdfs:comment """These fires burn and spread from treetop to treetop. spread at a rapid pace.	

Resource: https://www.supplycache.com/blogs/news/the-different-types-of-wildland-fires""" .


###  http://www.semanticweb.org/ontologies/2022/6/geological_taxonomy#Crust
:Crust rdf:type owl:Class ;
       rdfs:subClassOf :Units_of_Earth_structure ;
       rdfs:comment """outermost solid shell of a rocky planet, dwarf planet or natural satellite, which is chemically distinct from the underlying mantle

Resource: https://en.wikipedia.org/wiki/Crust_(geology)

Justification: depending on composition of density, different rocks""" .


###  http://www.semanticweb.org/ontologies/2022/6/geological_taxonomy#Cryalfs
:Cryalfs rdf:type owl:Class ;
         rdfs:subClassOf :Alfisols ;
         rdfs:comment """Alfisols that have a cryic or isofrigid temperature regime. 

Resource: https://sites.google.com/site/dinpuithai/Home/taxonomy/j-alfisols""" .


###  http://www.semanticweb.org/ontologies/2022/6/geological_taxonomy#Cryands
:Cryands rdf:type owl:Class ;
         rdfs:subClassOf :Andisols ;
         rdfs:comment """Andisols that have a cryic soil temperature regime.


Resource: https://sites.google.com/site/dinpuithai/Home/key10/key10d""" .


###  http://www.semanticweb.org/ontologies/2022/6/geological_taxonomy#Cryepts
:Cryepts rdf:type owl:Class ;
         rdfs:subClassOf :Inceptisols ;
         rdfs:comment """Inceptisols that have a cryic soil temperature regime.

Resource: https://sites.google.com/site/dinpuithai/Home/key10/key10k""" .


###  http://www.semanticweb.org/ontologies/2022/6/geological_taxonomy#Cryerts
:Cryerts rdf:type owl:Class ;
         rdfs:subClassOf :Vertisols ;
         rdfs:comment """Vertisols that have a cryic soil temperature regime

Resource: https://sites.google.com/site/dinpuithai/Home/key10/key10f""" .


###  http://www.semanticweb.org/ontologies/2022/6/geological_taxonomy#Cryids
:Cryids rdf:type owl:Class ;
        rdfs:subClassOf :Aridisols ;
        rdfs:comment """Aridisols that have a cryic soil temperature regime

Resource: https://sites.google.com/site/dinpuithai/Home/key10/key10g""" .


###  http://www.semanticweb.org/ontologies/2022/6/geological_taxonomy#Cryods
:Cryods rdf:type owl:Class ;
        rdfs:subClassOf :Spodosols ;
        rdfs:comment """Cold Spodosols (cryic temperature regime)

Resource: \"Illustrated Guide to Soil Taxonomy\" book by Unites States Department of Agriculture""" .


###  http://www.semanticweb.org/ontologies/2022/6/geological_taxonomy#Cryolls
:Cryolls rdf:type owl:Class ;
         rdfs:subClassOf :Mollisols ;
         rdfs:comment """Cryolls have a frigid, cryic, or pergelic Soil temperature regimes

Resource: https://www.sciencedirect.com/topics/agricultural-and-biological-sciences/mollisol""" .


###  http://www.semanticweb.org/ontologies/2022/6/geological_taxonomy#Cyclone
:Cyclone rdf:type owl:Class ;
         rdfs:subClassOf :Natural_disasters ;
         rdfs:comment """Cyclone is a large air mass that rotates around a strong center of low atmospheric pressure

Resource: https://en.wikipedia.org/wiki/Cyclone

Justification: depending upon where it originates, affecting size of area""" .


###  http://www.semanticweb.org/ontologies/2022/6/geological_taxonomy#Dacite
:Dacite rdf:type owl:Class ;
        rdfs:subClassOf :Igneous_rocks ;
        rdfs:comment """A felsic to intermediate volcanic rock with high iron content

Resource: https://geology.fandom.com/wiki/Dacite""" .


###  http://www.semanticweb.org/ontologies/2022/6/geological_taxonomy#Debris_fall
:Debris_fall rdf:type owl:Class ;
             rdfs:subClassOf :Falls ;
             owl:disjointWith :Rockfall ;
             rdfs:comment """A relatively free downward or forward falling of unconsolidated or poorly consolidated earth or rocky debris from a cliff, cave, or arch

Resource: https://encyclopedia2.thefreedictionary.com/debris+fall""" .


###  http://www.semanticweb.org/ontologies/2022/6/geological_taxonomy#Debris_slide
:Debris_slide rdf:type owl:Class ;
              rdfs:subClassOf :Block_slide ;
              owl:disjointWith :Rock_slide ;
              rdfs:comment """If debris slide down a slope on a distinct shear plane, the movements are called debris slides.

Resource: http://www.wrds.uwyo.edu/wrds/wsgs/hazards/landslides/classscheme.htm""" .


###  http://www.semanticweb.org/ontologies/2022/6/geological_taxonomy#Debris_topples
:Debris_topples rdf:type owl:Class ;
                rdfs:subClassOf :Topples ;
                owl:disjointWith :Rock_topples ;
                rdfs:comment """Topples in which debris are the material type

Resource: https://en.wikipedia.org/wiki/Landslide_classification#Types_and_classification""" .


###  http://www.semanticweb.org/ontologies/2022/6/geological_taxonomy#Diabase
:Diabase rdf:type owl:Class ;
         rdfs:subClassOf :Igneous_rocks ;
         rdfs:comment """Diabase, also called dolerite or microgabbro, is a mafic, holocrystalline, subvolcanic rock equivalent to volcanic basalt or plutonic gabbro.

Resource: https://en.wikipedia.org/wiki/Diabase""" .


###  http://www.semanticweb.org/ontologies/2022/6/geological_taxonomy#Diamictite
:Diamictite rdf:type owl:Class ;
            rdfs:subClassOf :Conglomerate ;
            rdfs:comment """Diamictite is a poorly sorted or non-sorted terrigenous non-calcareous sedimentary rock.

Resource: https://www.sandatlas.org/rock-types/#Diamictite""" .


###  http://www.semanticweb.org/ontologies/2022/6/geological_taxonomy#Diatomite
:Diatomite rdf:type owl:Class ;
           rdfs:subClassOf :Sedimentary_rocks ;
           rdfs:comment """A sedimentary rock formed from diatom fossils

Resource: https://geology.fandom.com/wiki/List_of_rock_types""" .


###  http://www.semanticweb.org/ontologies/2022/6/geological_taxonomy#Diorite
:Diorite rdf:type owl:Class ;
         rdfs:subClassOf :Igneous_rocks ;
         rdfs:comment """Diorite is an intrusive igneous rock formed by the slow cooling underground of magma that has a moderate content of silica and a relatively low content of alkali metals.

Resource: https://en.wikipedia.org/wiki/Diorite

Justification: Based on presence of orbicular structure""" .


###  http://www.semanticweb.org/ontologies/2022/6/geological_taxonomy#Direct_flooding
:Direct_flooding rdf:type owl:Class ;
                 rdfs:subClassOf :Coastal_Floods ;
                 rdfs:comment """where the sea height exceeds the elevation of the land, often where waves have not built up a natural barrier such as a dune	

Resource: https://en.wikipedia.org/wiki/Coastal_flooding""" .


###  http://www.semanticweb.org/ontologies/2022/6/geological_taxonomy#Dolomite
:Dolomite rdf:type owl:Class ;
          rdfs:subClassOf :Sedimentary_rocks .


###  http://www.semanticweb.org/ontologies/2022/6/geological_taxonomy#Drought
:Drought rdf:type owl:Class ;
         rdfs:subClassOf :Natural_disasters ;
         rdfs:comment """A drought is an event of prolonged shortages in the water supply, whether atmospheric (below-average precipitation), surface water or ground water.	

Resource: https://en.wikipedia.org/wiki/Drought

Justification: Classified based Palmer Drought Severity Index(PDSI)
https://droughtmonitor.unl.edu/About/WhatistheUSDM.aspx""" .


###  http://www.semanticweb.org/ontologies/2022/6/geological_taxonomy#Dunite
:Dunite rdf:type owl:Class ;
        rdfs:subClassOf :Igneous_rocks ;
        rdfs:comment """Dunite, also known as olivinite, is an intrusive igneous rock of ultramafic composition and with phaneritic (coarse-grained) texture.

Resource: https://en.wikipedia.org/wiki/Dunite""" .


###  http://www.semanticweb.org/ontologies/2022/6/geological_taxonomy#Durids
:Durids rdf:type owl:Class ;
        rdfs:subClassOf :Aridisols ;
        rdfs:comment """Characterized by accumulations of silica, but infrequently found; associated with soils formed from volcanic materials. 

Resource: https://www.sciencedirect.com/topics/agricultural-and-biological-sciences/aridisol""" .


###  http://www.semanticweb.org/ontologies/2022/6/geological_taxonomy#Earthquakes
:Earthquakes rdf:type owl:Class ;
             rdfs:subClassOf :Natural_disasters ;
             rdfs:comment """shaking of the surface of the Earth resulting from a sudden release of energy in the Earth's lithosphere that creates seismic waves.

Resource: https://en.wikipedia.org/wiki/Earthquake

Justification: Classified based on the origin of earthquake process""" .


###  http://www.semanticweb.org/ontologies/2022/6/geological_taxonomy#Eclogite
:Eclogite rdf:type owl:Class ;
          rdfs:subClassOf :Metamorphic_rocks ;
          rdfs:comment """An ultra-high grade metamorphosed basalt or gabbro; also a facies of metamorphic rocks

Resource: https://geology.fandom.com/wiki/List_of_rock_types""" .


###  http://www.semanticweb.org/ontologies/2022/6/geological_taxonomy#Elements
:Elements rdf:type owl:Class ;
          rdfs:subClassOf :Mineral ;
          rdfs:comment """Native element minerals are those elements that occur in nature in uncombined form with a distinct mineral structure.	

Resource: https://en.wikipedia.org/wiki/Native_element_mineral

Justification: Classified based on physical characters and chemical relations
https://www.911metallurgist.com/blog/descriptive-mineralogy-classification""" .


###  http://www.semanticweb.org/ontologies/2022/6/geological_taxonomy#Enderbite
:Enderbite rdf:type owl:Class ;
           rdfs:subClassOf :Charnockite ;
           rdfs:comment """Enderbite is an igneous rock of the charnockite series, consisting essentially of quartz, antiperthite (or perthite), orthopyroxene (usually hypersthene) and magnetite, and is equivalent to an orthopyroxene bearing tonalite.

Resource: https://en.wikipedia.org/wiki/Enderbite""" .


###  http://www.semanticweb.org/ontologies/2022/6/geological_taxonomy#Entisols
:Entisols rdf:type owl:Class ;
          rdfs:subClassOf :Soil ;
          rdfs:comment """The central concept of Entisols is that of soils that have little or no evidence of development of pedogenic horizons. 

Resource: https://www.nrcs.usda.gov/wps/portal/nrcs/detail/soils/survey/class/maps/?cid=nrcs142p2_053596

Justification: Divided between  near surface saturation; sandy texture; formation in recent stratified alluvial sediments; and a virtual lack of horizon formation, mostly in areas of young erosional surfaces.
\"Illustrated Guide to Soil Taxonomy\" book by Unites States Department of Agriculture""" .


###  http://www.semanticweb.org/ontologies/2022/6/geological_taxonomy#Epidosite
:Epidosite rdf:type owl:Class ;
           rdfs:subClassOf :Metamorphic_rocks ;
           rdfs:comment """Epidosite is a metamorphic rock consisting of epidote and quartz. This rock type is a product of hydrothermal metamorphism.

Resource: https://www.sandatlas.org/epidosite/""" .


###  http://www.semanticweb.org/ontologies/2022/6/geological_taxonomy#Essexite
:Essexite rdf:type owl:Class ;
          rdfs:subClassOf :Igneous_rocks ;
          rdfs:comment """Essexite, also called nepheline monzogabbro, is a dark gray or black holocrystalline plutonic igneous rock.

Resource: https://en.wikipedia.org/wiki/Essexite""" .


###  http://www.semanticweb.org/ontologies/2022/6/geological_taxonomy#Evaporite
:Evaporite rdf:type owl:Class ;
           rdfs:subClassOf :Sedimentary_rocks ;
           rdfs:comment """A chemical sedimentary rock formed by accumulation of minerals after evaporation

Resource: https://geology.fandom.com/wiki/List_of_rock_types""" .


###  http://www.semanticweb.org/ontologies/2022/6/geological_taxonomy#Exceptional_Drought
:Exceptional_Drought rdf:type owl:Class ;
                     rdfs:subClassOf :Drought ;
                     rdfs:comment """It is D4 category and causes exceptional crop/pasture losses and shortages of water in reservoirs, streams, and wells creating water emergencies.

Resource: https://droughtmonitor.unl.edu/About/WhatistheUSDM.aspx""" .


###  http://www.semanticweb.org/ontologies/2022/6/geological_taxonomy#Explosion_Earthquakes
:Explosion_Earthquakes rdf:type owl:Class ;
                       rdfs:subClassOf :Earthquakes ;
                       rdfs:comment """Man triggered kind of earthquakes and represent the biggest impact of modern-day nuclear war.

Resource: https://www.conserve-energy-future.com/howearthquakesoccur.php""" .


###  http://www.semanticweb.org/ontologies/2022/6/geological_taxonomy#Extratropical_cyclone
:Extratropical_cyclone rdf:type owl:Class ;
                       rdfs:subClassOf :Cyclone ;
                       owl:disjointWith :Tropical_cyclone ;
                       rdfs:comment """Extratropical cyclones cover and affects a larger area and can originate over the land and sea.

Resource: https://www.insightsonindia.com/world-geography/physical-geography-of-the-world/climatology/cyclones-and-anticyclones/difference-between-extratropical-and-tropical-cyclones/#:~:text=Extratropical%20cyclones%20cover%20a%20larger,compared%20to%20the%20tropical%20cyclone.

Justification: depending upon direction of winds""" .


###  http://www.semanticweb.org/ontologies/2022/6/geological_taxonomy#Extreme_Drought
:Extreme_Drought rdf:type owl:Class ;
                 rdfs:subClassOf :Drought ;
                 rdfs:comment """It is D3 category and causes major crop/pasture losses.

Resource: https://droughtmonitor.unl.edu/About/WhatistheUSDM.aspx""" .


###  http://www.semanticweb.org/ontologies/2022/6/geological_taxonomy#Extreme_Temperature
:Extreme_Temperature rdf:type owl:Class ;
                     rdfs:subClassOf :Natural_disasters ;
                     rdfs:comment """A general term for temperature variations above (extreme heat) or below (extreme cold) normal conditions.

Resource: http://desinventar.cimafoundation.org/definitions.html

Justification: Classified based on temperature""" .


###  http://www.semanticweb.org/ontologies/2022/6/geological_taxonomy#Falls
:Falls rdf:type owl:Class ;
       rdfs:subClassOf :Landslide ;
       rdfs:comment """Detachment of soil or rock from a steep slope along a surface on which little or no shear displacement takes place.

Resource: https://en.wikipedia.org/wiki/Landslide_classification#Types_and_classification

Justification: Divided based on type of material""" .


###  http://www.semanticweb.org/ontologies/2022/6/geological_taxonomy#Fenite
:Fenite rdf:type owl:Class ;
        rdfs:subClassOf :Metamorphic_rocks ;
        rdfs:comment """Fenite is a metasomatic alteration associated particularly with carbonatite intrusions and created, very rarely, by advanced carbon dioxide alteration (carbonation) of felsic and mafic rocks.

Resource: https://en.wikipedia.org/wiki/Fenite""" .


###  http://www.semanticweb.org/ontologies/2022/6/geological_taxonomy#Fibrists
:Fibrists rdf:type owl:Class ;
          rdfs:subClassOf :Histosols ;
          rdfs:comment """Histosols that are primarily made up of only slightly decomposed organic materials, often called peat.

Resource: https://en.wikipedia.org/wiki/Histosol""" .


###  http://www.semanticweb.org/ontologies/2022/6/geological_taxonomy#Flash_flood
:Flash_flood rdf:type owl:Class ;
             rdfs:subClassOf :Floods ;
             rdfs:comment """A flash flood is a rapid flooding of low-lying areas: washes, rivers, dry lakes and depressions.	

Resource: https://en.wikipedia.org/wiki/Flash_flood""" .


###  http://www.semanticweb.org/ontologies/2022/6/geological_taxonomy#Flint
:Flint rdf:type owl:Class ;
       rdfs:subClassOf :Sedimentary_rocks ;
       rdfs:comment """Flint is a sedimentary cryptocrystalline form of the mineral quartz,[1][2] categorized as the variety of chert that occurs in chalk or marly limestone.

Resource: https://en.wikipedia.org/wiki/Flint""" .


###  http://www.semanticweb.org/ontologies/2022/6/geological_taxonomy#Floods
:Floods rdf:type owl:Class ;
        rdfs:subClassOf :Natural_disasters ;
        rdfs:comment """A flood is an overflow of water that submerges land that is usually dry.	

Resource: https://en.wikipedia.org/wiki/Flood

Justification: Depending upon the area affected""" .


###  http://www.semanticweb.org/ontologies/2022/6/geological_taxonomy#Flows
:Flows rdf:type owl:Class ;
       rdfs:subClassOf :Landslide ;
       rdfs:comment """A flow is a spatially continuous movement in which surfaces of shear are short-lived, closely spaced, and usually not preserved.

Resource: https://en.wikipedia.org/wiki/Landslide_classification

Justification: Classified based on the speed of the material flowing
https://geology.com/usgs/landslides/#flows""" .


###  http://www.semanticweb.org/ontologies/2022/6/geological_taxonomy#Fluvents
:Fluvents rdf:type owl:Class ;
          rdfs:subClassOf :Entisols ;
          rdfs:comment """Entisols that formed in stratified alluvial sediments as evidenced
by the irregular decrease/increase of carbon content with increasing depth

Resource: \"Illustrated Guide to Soil Taxonomy\" book by Unites States Department of Agriculture""" .


###  http://www.semanticweb.org/ontologies/2022/6/geological_taxonomy#Fog
:Fog rdf:type owl:Class ;
     rdfs:subClassOf :Weather_conditions ;
     rdfs:comment """Fog is literally a cloud at ground level, which raises ambient humidity to its maximum, and considerably decreases visibility.

Resource: https://weather.fandom.com/wiki/Types_of_Weather#Fog""" .


###  http://www.semanticweb.org/ontologies/2022/6/geological_taxonomy#Foidolite
:Foidolite rdf:type owl:Class ;
           rdfs:subClassOf :Igneous_rocks ;
           rdfs:comment """Foidolite is a rare phaneritic (coarse-grained) intrusive igneous rock in which more than 60% of light-coloured minerals are feldspathoids.

Resource: https://en.wikipedia.org/wiki/Foidolite""" .


###  http://www.semanticweb.org/ontologies/2022/6/geological_taxonomy#Folists
:Folists rdf:type owl:Class ;
         rdfs:subClassOf :Histosols ;
         rdfs:comment """Histosols that are not saturated with water for long periods of time during the year.

Resource: https://en.wikipedia.org/wiki/Histosol""" .


###  http://www.semanticweb.org/ontologies/2022/6/geological_taxonomy#Foyaite
:Foyaite rdf:type owl:Class ;
         rdfs:subClassOf :Igneous_rocks ;
         rdfs:comment """Foyaite is a rare igneous rock consisting of nepheline and alkali feldspar with a trachytic texture. Foyaite is a variety of nepheline syenite.

Resource: https://www.sandatlas.org/rock-types/#Foyaite""" .


###  http://www.semanticweb.org/ontologies/2022/6/geological_taxonomy#Gabbro
:Gabbro rdf:type owl:Class ;
        rdfs:subClassOf :Igneous_rocks ;
        rdfs:comment """Gabbro is a phaneritic (coarse-grained), mafic intrusive igneous rock formed from the slow cooling of magnesium-rich and iron-rich magma into a holocrystalline mass deep beneath the Earth's surface.

Resource: https://en.wikipedia.org/wiki/Gabbro""" .


###  http://www.semanticweb.org/ontologies/2022/6/geological_taxonomy#Gelands
:Gelands rdf:type owl:Class ;
         rdfs:subClassOf :Andisols ;
         rdfs:comment """Andisols that have, in normal years, a mean annual soil temperature of 0 oC or colder and a mean summer soil temperature


Resource: https://sites.google.com/site/dinpuithai/Home/key10/key10d""" .


###  http://www.semanticweb.org/ontologies/2022/6/geological_taxonomy#Gelepts
:Gelepts rdf:type owl:Class ;
         rdfs:subClassOf :Inceptisols ;
         rdfs:comment """Inceptisols that have, in normal years, a mean annual soil temperature of 0 oC or colder and a mean summer soil temperature.

Resource: https://sites.google.com/site/dinpuithai/Home/key10/key10k""" .


###  http://www.semanticweb.org/ontologies/2022/6/geological_taxonomy#Gelisols
:Gelisols rdf:type owl:Class ;
          rdfs:subClassOf :Soil ;
          rdfs:comment """The central concept of Gelisols is that of soils that have permafrost within 100 cm of the soil surface and/or have gelic materials within 100 cm of the soil surface and have permafrost within 200 cm.

Resource: https://www.nrcs.usda.gov/wps/portal/nrcs/detail/soils/survey/class/maps/?cid=nrcs142p2_053598

Justification: Depending upon the soil material (organic vs. mineral) and the presence of gelic materials.
https://acsess.onlinelibrary.wiley.com/doi/full/10.2136/sh2013-54-4-gc""" .


###  http://www.semanticweb.org/ontologies/2022/6/geological_taxonomy#Gelods
:Gelods rdf:type owl:Class ;
        rdfs:subClassOf :Spodosols ;
        rdfs:comment """Very cold Spodosols that lack permafrost (gelic temperature
regime)

Resource: \"Illustrated Guide to Soil Taxonomy\" book by Unites States Department of Agriculture""" .


###  http://www.semanticweb.org/ontologies/2022/6/geological_taxonomy#Gelolls
:Gelolls rdf:type owl:Class ;
         rdfs:subClassOf :Mollisols ;
         rdfs:comment """Mollisols that have, in normal years, a mean annual soil temperature of 0 oC or colder and a mean summer soil temperature

Resource: https://sites.google.com/site/dinpuithai/Home/key10/key10i""" .


###  http://www.semanticweb.org/ontologies/2022/6/geological_taxonomy#Geological_Object
:Geological_Object rdf:type owl:Class ;
                   rdfs:subClassOf :Geological_entities ;
                   rdfs:comment """A material object constituted by some geological material.

Resource: https://github.com/Loop3D/GKM/blob/1.0.2/Loop3D-GSO/Modules/GSO-Geologic_Process.ttl

Justification: Classified based on the origination from distinct geological processes at different periods of time""" .


###  http://www.semanticweb.org/ontologies/2022/6/geological_taxonomy#Geological_entities
:Geological_entities rdf:type owl:Class ;
                     rdfs:comment """Geological thing with distinct and independent existence.

Justification: Different entities of geology""" .


###  http://www.semanticweb.org/ontologies/2022/6/geological_taxonomy#Geological_phenomena
:Geological_phenomena rdf:type owl:Class ;
                      rdfs:subClassOf :Geological_entities ;
                      rdfs:comment """Phenomenon which occurs without human inputs.

Justification: Classification based on the disaster and atmospheric conditions""" .


###  http://www.semanticweb.org/ontologies/2022/6/geological_taxonomy#Geyserite
:Geyserite rdf:type owl:Class ;
           rdfs:subClassOf :Sedimentary_rocks ;
           rdfs:comment """Geyserite, or siliceous sinter, is a form of opaline silica that is often found as crusts or layers around hot springs and geysers.

Resource: https://en.wikipedia.org/wiki/Geyserite""" .


###  http://www.semanticweb.org/ontologies/2022/6/geological_taxonomy#Gneiss
:Gneiss rdf:type owl:Class ;
        rdfs:subClassOf :Metamorphic_rocks ;
        rdfs:comment """A coarse grained metamorphic rock

Resource: https://geology.fandom.com/wiki/List_of_rock_types""" .


###  http://www.semanticweb.org/ontologies/2022/6/geological_taxonomy#Gossan
:Gossan rdf:type owl:Class ;
        rdfs:subClassOf :Metamorphic_rocks ;
        rdfs:comment """Gossan is intensely oxidized, weathered or decomposed rock, usually the upper and exposed part of an ore deposit or mineral vein.

Resource: https://en.wikipedia.org/wiki/Gossan""" .


###  http://www.semanticweb.org/ontologies/2022/6/geological_taxonomy#Granite
:Granite rdf:type owl:Class ;
         rdfs:subClassOf :Igneous_rocks ;
         rdfs:comment """Granite ( or is a coarse-grained intrusive igneous rock composed mostly of quartz, alkali feldspar, and plagioclase.

Resource: https://en.wikipedia.org/wiki/Granite""" .


###  http://www.semanticweb.org/ontologies/2022/6/geological_taxonomy#Granodiorite
:Granodiorite rdf:type owl:Class ;
              rdfs:subClassOf :Igneous_rocks ;
              rdfs:comment """Granodiorite is a coarse-grained (phaneritic) intrusive igneous rock similar to granite, but containing more plagioclase feldspar than orthoclase feldspar.

Resource: https://en.wikipedia.org/wiki/Granodiorite""" .


###  http://www.semanticweb.org/ontologies/2022/6/geological_taxonomy#Granophyre
:Granophyre rdf:type owl:Class ;
            rdfs:subClassOf :Igneous_rocks ;
            rdfs:comment """Granophyre is a subvolcanic rock that contains quartz and alkali feldspar in characteristic angular intergrowths such as those in the accompanying image.

Resource: https://en.wikipedia.org/wiki/Granophyre""" .


###  http://www.semanticweb.org/ontologies/2022/6/geological_taxonomy#Granulite
:Granulite rdf:type owl:Class ;
           rdfs:subClassOf :Metamorphic_rocks ;
           rdfs:comment """Granulites are a class of high-grade metamorphic rocks of the granulite facies that have experienced high-temperature and moderate-pressure metamorphism.

Resource: https://en.wikipedia.org/wiki/Granulite""" .


###  http://www.semanticweb.org/ontologies/2022/6/geological_taxonomy#Graywacke
:Graywacke rdf:type owl:Class ;
           rdfs:subClassOf :Sedimentary_rocks ;
           rdfs:comment """Greywacke or graywacke (German grauwacke, signifying a grey, earthy rock) is a variety of sandstone generally characterized by its hardness, dark color, and poorly sorted angular grains of quartz, feldspar, and small rock fragments or lithic fragments set in a compact, clay-fine matrix. It is a texturally immature sedimentary rock generally found in Paleozoic strata.

Resource: https://en.wikipedia.org/wiki/Greywacke""" .


###  http://www.semanticweb.org/ontologies/2022/6/geological_taxonomy#Greenschist
:Greenschist rdf:type owl:Class ;
             rdfs:subClassOf :Metamorphic_rocks ;
             rdfs:comment """Greenschists are metamorphic rocks that formed under the lowest temperatures and pressures usually produced by regional metamorphism, typically 300–450 °C (570–840 °F) and 2–10 kilobars (29,000–145,000 psi).

Resource: https://en.wikipedia.org/wiki/Greenschist

Justification: Depending upon the alteration to a greenish color by the formation of the minerals""" .


###  http://www.semanticweb.org/ontologies/2022/6/geological_taxonomy#Greenstone
:Greenstone rdf:type owl:Class ;
            rdfs:subClassOf :Greenschist ;
            rdfs:comment """A field term applied to any compact, dark-green, altered or metamorphosed basic igneous rock (e.g. spilite, basalt, gabbro, diabase) that owes its color to the presence of chlorite, actinolite, or epidote.

Resource: https://mrdata.usgs.gov/geology/state/sgmc-lith.php?code=5.3.3.3""" .


###  http://www.semanticweb.org/ontologies/2022/6/geological_taxonomy#Greisen
:Greisen rdf:type owl:Class ;
         rdfs:subClassOf :Metamorphic_rocks ;
         rdfs:comment """Greisen is a pneumatolytically altered granitic rock. Greisen contains lots of quartz and mica plus several exotic minerals like cassiterite, tourmaline, topaz, etc. Greised is a metamorphic rock that metamorphosed itself — hot fluids that altered the rock were provided by the cooling magma body itself

Resource: https://www.sandatlas.org/rock-types/""" .


###  http://www.semanticweb.org/ontologies/2022/6/geological_taxonomy#Greywacke
:Greywacke rdf:type owl:Class ;
           rdfs:subClassOf :Sedimentary_rocks ;
           rdfs:comment """Greywacke or graywacke (German grauwacke, signifying a grey, earthy rock) is a variety of sandstone generally characterized by its hardness, dark color, and poorly sorted angular grains of quartz, feldspar, and small rock fragments or lithic fragments set in a compact, clay-fine matrix. 

Resource: https://en.wikipedia.org/wiki/Greywacke""" .


###  http://www.semanticweb.org/ontologies/2022/6/geological_taxonomy#Gritstone
:Gritstone rdf:type owl:Class ;
           rdfs:subClassOf :Sedimentary_rocks ;
           rdfs:comment """Essentially a coarse sandstone formed from small pebbles

Resource: https://geology.fandom.com/wiki/List_of_rock_types""" .


###  http://www.semanticweb.org/ontologies/2022/6/geological_taxonomy#Ground_Fire
:Ground_Fire rdf:type owl:Class ;
             rdfs:subClassOf :Wildfire ;
             rdfs:comment """A ground fire is a type of wildfire that occurs in the subsurface where fuels such as peat, coal, tree roots, and other buried organic matter ignite and burn under the ground.	

Resource: https://www.supplycache.com/blogs/news/the-different-types-of-wildland-fires""" .


###  http://www.semanticweb.org/ontologies/2022/6/geological_taxonomy#Gypsids
:Gypsids rdf:type owl:Class ;
         rdfs:subClassOf :Aridisols ;
         rdfs:comment """Characterized by an accumulation of gypsum

Resource: https://www.sciencedirect.com/topics/agricultural-and-biological-sciences/aridisol""" .


###  http://www.semanticweb.org/ontologies/2022/6/geological_taxonomy#Gypsum
:Gypsum rdf:type owl:Class ;
        rdfs:subClassOf :Sedimentary_rocks ;
        rdfs:comment """Rock gypsum (a.k.a. gyprock) is a chemical sedimentary rock.  It is an example of an evaporite - it forms by the evaporation of water (usually seawater) and the precipitation of dissolved minerals.

Resource: http://www.jsjgeology.net/Rock-gypsum.htm""" .


###  http://www.semanticweb.org/ontologies/2022/6/geological_taxonomy#Halides
:Halides rdf:type owl:Class ;
         rdfs:subClassOf :Mineral ;
         rdfs:comment """The halide minerals are compounds in which a halogen (fluorine, chlorine, iodine, or bromine) is the main anion.	

Resource: https://en.wikipedia.org/wiki/Mineral#Classification""" .


###  http://www.semanticweb.org/ontologies/2022/6/geological_taxonomy#Harzburgite
:Harzburgite rdf:type owl:Class ;
             rdfs:subClassOf :Igneous_rocks ;
             rdfs:comment """Harzburgite, an ultramafic, igneous rock, is a variety of peridotite consisting mostly of the two minerals olivine and low-calcium (Ca) pyroxene (enstatite)

Resource: https://en.wikipedia.org/wiki/Harzburgite""" .


###  http://www.semanticweb.org/ontologies/2022/6/geological_taxonomy#Hawaiite
:Hawaiite rdf:type owl:Class ;
          rdfs:subClassOf :Basalt ;
          rdfs:comment """A class of basalts formed from ocean island (hot spot) magmatism.

Resource: https://geology.fandom.com/wiki/List_of_rock_types""" .


###  http://www.semanticweb.org/ontologies/2022/6/geological_taxonomy#Heat_wave
:Heat_wave rdf:type owl:Class ;
           rdfs:subClassOf :Extreme_Temperature ;
           rdfs:comment """A period of abnormally hot and/or unusually humid weather.

Resource: http://desinventar.cimafoundation.org/definitions.html""" .


###  http://www.semanticweb.org/ontologies/2022/6/geological_taxonomy#Hemists
:Hemists rdf:type owl:Class ;
         rdfs:subClassOf :Histosols ;
         rdfs:comment """Histosols that are primarily made up of moderately decomposed organic materials.

Resource: https://en.wikipedia.org/wiki/Histosol""" .


###  http://www.semanticweb.org/ontologies/2022/6/geological_taxonomy#Histels
:Histels rdf:type owl:Class ;
         rdfs:subClassOf :Gelisols ;
         rdfs:comment """Organic soil materials.

Resource: https://acsess.onlinelibrary.wiley.com/doi/full/10.2136/sh2013-54-4-gc""" .


###  http://www.semanticweb.org/ontologies/2022/6/geological_taxonomy#Histosols
:Histosols rdf:type owl:Class ;
           rdfs:subClassOf :Soil ;
           rdfs:comment """The central concept of Histosols is that of soils that are dominantly organic. 

Resource: https://www.nrcs.usda.gov/wps/portal/nrcs/detail/soils/survey/class/maps/?cid=nrcs142p2_053599

Justification: Depending upon the degree of decomposition of the organic matter.
https://www.sciencedirect.com/topics/agricultural-and-biological-sciences/histosols""" .


###  http://www.semanticweb.org/ontologies/2022/6/geological_taxonomy#Hornblendite
:Hornblendite rdf:type owl:Class ;
              rdfs:subClassOf :Igneous_rocks ;
              rdfs:comment """Hornblendite is a plutonic rock consisting mainly of the amphibole hornblende. Hornblende-rich ultramafic rocks are rare and when hornblende is the dominant mineral phase they are classified as hornblendites with qualifiers such as garnet hornblendite identifying a second abundant contained mineral.

Resource: https://en.wikipedia.org/wiki/Hornblendite""" .


###  http://www.semanticweb.org/ontologies/2022/6/geological_taxonomy#Hornfels
:Hornfels rdf:type owl:Class ;
          rdfs:subClassOf :Metamorphic_rocks ;
          rdfs:comment """Hornfels is the group name for a set of contact metamorphic rocks that have been baked and hardened by the heat of intrusive igneous masses and have been rendered massive, hard, splintery, and in some cases exceedingly tough and durable.

Resource: https://en.wikipedia.org/wiki/Hornfels

Justificaation: Depending upon the composition of hornfels""" .


###  http://www.semanticweb.org/ontologies/2022/6/geological_taxonomy#Humods
:Humods rdf:type owl:Class ;
        rdfs:subClassOf :Spodosols ;
        rdfs:comment """Spodosols with a large accumulation of carbon in the spodic
horizon

Resource: \"Illustrated Guide to Soil Taxonomy\" book by Unites States Department of Agriculture""" .


###  http://www.semanticweb.org/ontologies/2022/6/geological_taxonomy#Humults
:Humults rdf:type owl:Class ;
         rdfs:subClassOf :Ultisols ;
         rdfs:comment """Ultisols that have one or both of the following:
1. 0.9 percent (by weighted average) or more organic carbon in the upper 15 cm of the argillic or kandic horizon; or
2. 12 kg/m2 or more organic carbon between the mineral soil surface and a depth of 100 cm.


Resource: https://sites.google.com/site/dinpuithai/Home/key10/key10h""" .


###  http://www.semanticweb.org/ontologies/2022/6/geological_taxonomy#Hurricane
:Hurricane rdf:type owl:Class ;
           rdfs:subClassOf :Tropical_cyclone ;
           rdfs:comment """A tropical cyclone with maximum sustained winds of 74 mph (64 knots) or higher.	

Resource: https://www.nhc.noaa.gov/climo/""" .


###  http://www.semanticweb.org/ontologies/2022/6/geological_taxonomy#Hyaloclastite
:Hyaloclastite rdf:type owl:Class ;
               rdfs:subClassOf :Igneous_rocks ;
               rdfs:comment """Hyaloclastite is a volcanoclastic accumulation or breccia consisting of glass fragments (clasts) formed by quench fragmentation of lava flow surfaces during submarine or subglacial extrusion.

Resource: https://en.wikipedia.org/wiki/Hyaloclastite""" .


###  http://www.semanticweb.org/ontologies/2022/6/geological_taxonomy#Icelandite
:Icelandite rdf:type owl:Class ;
            rdfs:subClassOf :Igneous_rocks ;
            rdfs:comment """Icelandite is a type of volcanic rock, an andesite that is enriched in iron but deficient in aluminium (< 16.5% Al2O3).

Resource: https://en.wikipedia.org/wiki/Icelandite""" .


###  http://www.semanticweb.org/ontologies/2022/6/geological_taxonomy#Igneous_rocks
:Igneous_rocks rdf:type owl:Class ;
               rdfs:subClassOf :Rock ;
               rdfs:comment """Igneous rock is formed through the cooling and solidification of magma or lava.

Resource: https://en.wikipedia.org/wiki/Igneous_rock

Justification: Igneous rocks are classified according to mode of occurrence, texture, mineralogy, chemical composition, and the geometry of the igneous body.
https://en.wikipedia.org/wiki/Igneous_rock#Classification""" .


###  http://www.semanticweb.org/ontologies/2022/6/geological_taxonomy#Ignimbrite
:Ignimbrite rdf:type owl:Class ;
            rdfs:subClassOf :Igneous_rocks ;
            rdfs:comment """Ignimbrite is a type of volcanic rock. More specifically, ignimbrite is a variety of hardened tuff. 

Resource: https://en.wikipedia.org/wiki/Ignimbrite""" .


###  http://www.semanticweb.org/ontologies/2022/6/geological_taxonomy#Ijolite
:Ijolite rdf:type owl:Class ;
         rdfs:subClassOf :Igneous_rocks ;
         rdfs:comment """Ijolite is an igneous rock consisting essentially of nepheline and augite.

Resource: https://en.wikipedia.org/wiki/Ijolite""" .


###  http://www.semanticweb.org/ontologies/2022/6/geological_taxonomy#Inceptisols
:Inceptisols rdf:type owl:Class ;
             rdfs:subClassOf :Soil ;
             rdfs:comment """The central concept of Inceptisols is that of soils of humid and subhumid regions that have altered horizons that have lost bases or iron and aluminum but retain some weatherable minerals.

Resource: https://www.nrcs.usda.gov/wps/portal/nrcs/detail/soils/survey/class/maps/?cid=nrcs142p2_053601

Justification: The suborders of Inceptisols are distinguished by soil moisture, epipedon properties, and soil temperature regime.
https://web.archive.org/web/20040918225129/http://grunwald.ifas.ufl.edu/Nat_resources/soil_orders/inceptisols.htm""" .


###  http://www.semanticweb.org/ontologies/2022/6/geological_taxonomy#Interplate_earthquake
:Interplate_earthquake rdf:type owl:Class ;
                       rdfs:subClassOf :Tectonic_Earthquakes ;
                       owl:disjointWith :Intraplate_earthquake ;
                       rdfs:comment """Earthquake that occurs at the boundary between two tectonic plates.

Resource: https://en.wikipedia.org/wiki/Interplate_earthquake""" .


###  http://www.semanticweb.org/ontologies/2022/6/geological_taxonomy#Intraplate_earthquake
:Intraplate_earthquake rdf:type owl:Class ;
                       rdfs:subClassOf :Tectonic_Earthquakes ;
                       rdfs:comment """Earthquake that occurs within the interior of a tectonic plate

Resource: https://en.wikipedia.org/wiki/Intraplate_earthquake""" .


###  http://www.semanticweb.org/ontologies/2022/6/geological_taxonomy#Itacolumite
:Itacolumite rdf:type owl:Class ;
             rdfs:subClassOf :Sedimentary_rocks ;
             rdfs:comment """Itacolumite is a naturally occurring porous, yellow sandstone that is flexible when cut into relatively thin slabs.

Resource: https://en.wikipedia.org/wiki/Itacolumite""" .


###  http://www.semanticweb.org/ontologies/2022/6/geological_taxonomy#Jaspillite
:Jaspillite rdf:type owl:Class ;
            rdfs:subClassOf :Sedimentary_rocks ;
            rdfs:comment """An iron-rich chemical sedimentary rock similar to chert or banded iron formation

Resource: https://geology.fandom.com/wiki/List_of_rock_types""" .


###  http://www.semanticweb.org/ontologies/2022/6/geological_taxonomy#Kimberlite
:Kimberlite rdf:type owl:Class ;
            rdfs:subClassOf :Igneous_rocks ;
            rdfs:comment """Kimberlite is an igneous rock and a rare variant of peridotite.

Resource: https://en.wikipedia.org/wiki/Kimberlite""" .


###  http://www.semanticweb.org/ontologies/2022/6/geological_taxonomy#Komatiite
:Komatiite rdf:type owl:Class ;
           rdfs:subClassOf :Igneous_rocks ;
           rdfs:comment """Komatiite is a type of ultramafic mantle-derived volcanic rock defined as having crystallised from a lava of at least 18 wt% MgO.

Resource: https://en.wikipedia.org/wiki/Komatiite""" .


###  http://www.semanticweb.org/ontologies/2022/6/geological_taxonomy#Lamproite
:Lamproite rdf:type owl:Class ;
           rdfs:subClassOf :Igneous_rocks ;
           rdfs:comment """Lamproite is an ultrapotassic mantle-derived volcanic or subvolcanic rock.

Resource: https://en.wikipedia.org/wiki/Lamproite""" .


###  http://www.semanticweb.org/ontologies/2022/6/geological_taxonomy#Lamprophyre
:Lamprophyre rdf:type owl:Class ;
             rdfs:subClassOf :Igneous_rocks ;
             rdfs:comment """Ultrapotassic igneous rocks – An ultramafic, ultrapotassic intrusive rock dominated by mafic phenocrysts in a feldspar groundmass

Resource: https://en.wikipedia.org/wiki/Lamprophyre""" .


###  http://www.semanticweb.org/ontologies/2022/6/geological_taxonomy#Landslide
:Landslide rdf:type owl:Class ;
           rdfs:subClassOf :Natural_disasters ;
           rdfs:comment """Landslides, also known as landslips, are several forms of mass wasting that may include a wide range of ground movements, such as rockfalls, deep-seated slope failures, mudflows, and debris flows.

Resource: https://en.wikipedia.org/wiki/Landslide

Justification: Classified based on the different movements of material across the slope""" .


###  http://www.semanticweb.org/ontologies/2022/6/geological_taxonomy#Lateral_Spreads
:Lateral_Spreads rdf:type owl:Class ;
                 rdfs:subClassOf :Flows ;
                 rdfs:comment """Lateral spread or flow are terms referring to landslides that commonly form on gentle slopes and that have rapid fluid-like flow movement, like water.

Resource: https://earthquake.usgs.gov/learn/glossary/?term=lateral%20spread%20or%20flow

Justification: Classified based on type of material""" .


###  http://www.semanticweb.org/ontologies/2022/6/geological_taxonomy#Laterite
:Laterite rdf:type owl:Class ;
          rdfs:subClassOf :Sedimentary_rocks ;
          rdfs:comment """A residual sedimentary rock formed from a parent rock under tropical conditions

Resource: https://geology.fandom.com/wiki/List_of_rock_types""" .


###  http://www.semanticweb.org/ontologies/2022/6/geological_taxonomy#Latite
:Latite rdf:type owl:Class ;
        rdfs:subClassOf :Igneous_rocks ;
        rdfs:comment """Latite is an igneous, volcanic rock, with aphanitic-aphyric to aphyric-porphyritic texture.

Resource: https://en.wikipedia.org/wiki/Latite""" .


###  http://www.semanticweb.org/ontologies/2022/6/geological_taxonomy#Lherzolite
:Lherzolite rdf:type owl:Class ;
            rdfs:subClassOf :Igneous_rocks ;
            rdfs:comment """Lherzolite is a type of ultramafic igneous rock. 

Resource: https://en.wikipedia.org/wiki/Lherzolite""" .


###  http://www.semanticweb.org/ontologies/2022/6/geological_taxonomy#Lignite
:Lignite rdf:type owl:Class ;
         rdfs:subClassOf :Sedimentary_rocks ;
         rdfs:comment """A sedimentary rock composed of organic material; otherwise known as Brown Coal

Resource: https://geology.fandom.com/wiki/List_of_rock_types""" .


###  http://www.semanticweb.org/ontologies/2022/6/geological_taxonomy#Limburgite
:Limburgite rdf:type owl:Class ;
            rdfs:subClassOf :Igneous_rocks ;
            rdfs:comment """imburgite is a dark-colored volcanic rock resembling basalt in appearance, but containing normally no feldspar.

Resource: https://en.wikipedia.org/wiki/Limburgite""" .


###  http://www.semanticweb.org/ontologies/2022/6/geological_taxonomy#Limestone
:Limestone rdf:type owl:Class ;
           rdfs:subClassOf :Sedimentary_rocks ;
           rdfs:comment """A sedimentary rock composed primarily of carbonate minerals

Resource: https://geology.fandom.com/wiki/List_of_rock_types""" .


###  http://www.semanticweb.org/ontologies/2022/6/geological_taxonomy#Limnic_Eruptions
:Limnic_Eruptions rdf:type owl:Class ;
                  rdfs:subClassOf :Natural_disasters ;
                  rdfs:comment """type of natural disaster in which dissolved carbon dioxide (CO2) suddenly erupts from deep lake waters, forming a gas cloud capable of suffocating wildlife, livestock, and humans. 	

Resource: https://en.wikipedia.org/wiki/Limnic_eruption""" .


###  http://www.semanticweb.org/ontologies/2022/6/geological_taxonomy#Litchfieldite
:Litchfieldite rdf:type owl:Class ;
               rdfs:subClassOf :Metamorphic_rocks ;
               rdfs:comment """Nepheline syenite gneiss

Resource: https://en.wikipedia.org/wiki/List_of_rock_types""" .


###  http://www.semanticweb.org/ontologies/2022/6/geological_taxonomy#Lithosphere
:Lithosphere rdf:type owl:Class ;
             rdfs:subClassOf :Upper_mantle ;
             rdfs:comment """outer, solid portion of the Earth. Also called the geosphere

Resource: https://education.nationalgeographic.org/resource/mantle

Justification: depending upon which crust it is associated""" .


###  http://www.semanticweb.org/ontologies/2022/6/geological_taxonomy#Local_tsunamis
:Local_tsunamis rdf:type owl:Class ;
                rdfs:subClassOf :Tsunami ;
                owl:disjointWith :Teletsunamis ;
                rdfs:comment """waves affecting coastlines close to the generating area (whether by tectonic or landslide activity)	

Resource: http://www.sfu.ca/geog355fall01/cobryne/types_of_tsunamis.html""" .


###  http://www.semanticweb.org/ontologies/2022/6/geological_taxonomy#Lower_mantle
:Lower_mantle rdf:type owl:Class ;
              rdfs:subClassOf :Mantle ;
              rdfs:comment """the region from 660 to 2900 km below Earth's surface; between the transition zone and the outer core.

Resource: https://en.wikipedia.org/wiki/Lower_mantle_(Earth)""" .


###  http://www.semanticweb.org/ontologies/2022/6/geological_taxonomy#Major_Hurricane
:Major_Hurricane rdf:type owl:Class ;
                 rdfs:subClassOf :Tropical_cyclone ;
                 rdfs:comment """A tropical cyclone with maximum sustained winds of 111 mph (96 knots) or higher,	

Resource: https://www.nhc.noaa.gov/climo/""" .


###  http://www.semanticweb.org/ontologies/2022/6/geological_taxonomy#Mantle
:Mantle rdf:type owl:Class ;
        rdfs:subClassOf :Units_of_Earth_structure ;
        rdfs:comment """part of the interior of the planet Earth

Resource: https://en.wikipedia.org/wiki/Mantle_(geology)

Justification: depending on changes in seismic velocity""" .


###  http://www.semanticweb.org/ontologies/2022/6/geological_taxonomy#Marble
:Marble rdf:type owl:Class ;
        rdfs:subClassOf :Metamorphic_rocks ;
        rdfs:comment """Marble is a metamorphic rock composed of recrystallized carbonate minerals, most commonly calcite or dolomite.

Resource: https://en.wikipedia.org/wiki/Marble""" .


###  http://www.semanticweb.org/ontologies/2022/6/geological_taxonomy#Marl
:Marl rdf:type owl:Class ;
      rdfs:subClassOf :Sedimentary_rocks ;
      rdfs:comment """A limestone with a considerable proportion of silicate material

Resource: https://geology.fandom.com/wiki/List_of_rock_types""" .


###  http://www.semanticweb.org/ontologies/2022/6/geological_taxonomy#Metamorphic_rocks
:Metamorphic_rocks rdf:type owl:Class ;
                   rdfs:subClassOf :Rock ;
                   rdfs:comment """Metamorphic rocks arise from the transformation of existing rock to new types of rock in a process called metamorphism

Resource: https://en.wikipedia.org/wiki/Metamorphic_rock

Justification: Classification of metamorphic rocks is based on mineral assemblage, texture, protolith, and bulk chemical composition of the rock.
https://www.geologyin.com/2014/07/classification-of-metamorphic-rocks.html""" .


###  http://www.semanticweb.org/ontologies/2022/6/geological_taxonomy#Metapelite
:Metapelite rdf:type owl:Class ;
            rdfs:subClassOf :Metamorphic_rocks ;
            rdfs:comment """A metamorphic rock with a protolith of clay-rich (siltstone) sedimentary rock

Resource: https://en.wikipedia.org/wiki/Metapelite""" .


###  http://www.semanticweb.org/ontologies/2022/6/geological_taxonomy#Metapsammite
:Metapsammite rdf:type owl:Class ;
              rdfs:subClassOf :Metamorphic_rocks ;
              rdfs:comment """A metamorphic rock with a protolith of quartz-rich (sandstone) sedimentary rock

Resource: https://en.wikipedia.org/wiki/List_of_rock_types""" .


###  http://www.semanticweb.org/ontologies/2022/6/geological_taxonomy#Migmatite
:Migmatite rdf:type owl:Class ;
           rdfs:subClassOf :Metamorphic_rocks ;
           rdfs:comment """Migmatite is a composite rock found in medium and high-grade metamorphic environments.

Resource: https://en.wikipedia.org/wiki/Migmatite""" .


###  http://www.semanticweb.org/ontologies/2022/6/geological_taxonomy#Mineral
:Mineral rdf:type owl:Class ;
         rdfs:subClassOf :Geological_Object ;
         rdfs:comment """Mineral or mineral species is, broadly speaking, a solid chemical compound with a fairly well-defined chemical composition and a specific crystal structure that occurs naturally in pure form.

Resource: https://en.wikipedia.org/wiki/Mineral

Justification: Classified based on chemical composition, mineral properties, crystal systems and silicate structures
https://sternberg.fhsu.edu/research-collections/geology/mineral-classification-page.html""" .


###  http://www.semanticweb.org/ontologies/2022/6/geological_taxonomy#Moderate_Drought
:Moderate_Drought rdf:type owl:Class ;
                  rdfs:subClassOf :Drought ;
                  rdfs:comment """It is D1 category, causes some damage to crops, pastures, streams, reservoirs, or wells low, some water shortages developing or imminent.

Resource: https://droughtmonitor.unl.edu/About/WhatistheUSDM.aspx""" .


###  http://www.semanticweb.org/ontologies/2022/6/geological_taxonomy#Mollisols
:Mollisols rdf:type owl:Class ;
           rdfs:subClassOf :Soil ;
           rdfs:comment """The central concept of Mollisols is that of soils that have a dark colored surface horizon and are base rich. Nearly all have a mollic epipedon.

Resource: https://www.nrcs.usda.gov/wps/portal/nrcs/detail/soils/survey/class/maps/?cid=nrcs142p2_053603

Justification: Soil temperature and moisture are principally used to separate.
https://www.sciencedirect.com/topics/agricultural-and-biological-sciences/mollisol""" .


###  http://www.semanticweb.org/ontologies/2022/6/geological_taxonomy#Monzogranite
:Monzogranite rdf:type owl:Class ;
              rdfs:subClassOf :Igneous_rocks ;
              rdfs:comment """Monzogranites are biotite granite rocks that are considered to be the final fractionation product of magma. 

Resource: https://en.wikipedia.org/wiki/Monzogranite""" .


###  http://www.semanticweb.org/ontologies/2022/6/geological_taxonomy#Monzonite
:Monzonite rdf:type owl:Class ;
           rdfs:subClassOf :Igneous_rocks ;
           rdfs:comment """Monzonite is an igneous intrusive rock, formed by slow cooling of underground magma that has a moderate silica content and is enriched in alkali metal oxides.

Resource: https://en.wikipedia.org/wiki/Monzonite""" .


###  http://www.semanticweb.org/ontologies/2022/6/geological_taxonomy#Mudstone
:Mudstone rdf:type owl:Class ;
          rdfs:subClassOf :Sedimentary_rocks ;
          rdfs:comment """A sedimentary rock composed of clay and muds

Resource: https://geology.fandom.com/wiki/List_of_rock_types""" .


###  http://www.semanticweb.org/ontologies/2022/6/geological_taxonomy#Mugearite
:Mugearite rdf:type owl:Class ;
           rdfs:subClassOf :Trachyandesite ;
           rdfs:comment """Sodic basaltic trachyandesite

Resource: https://geology.fandom.com/wiki/List_of_rock_types""" .


###  http://www.semanticweb.org/ontologies/2022/6/geological_taxonomy#Mylonite
:Mylonite rdf:type owl:Class ;
          rdfs:subClassOf :Metamorphic_rocks ;
          rdfs:comment """Mylonite is a fine-grained, compact metamorphic rock produced by dynamic recrystallization of the constituent minerals resulting in a reduction of the grain size of the rock.

Resource: https://en.wikipedia.org/wiki/Mylonite""" .


###  http://www.semanticweb.org/ontologies/2022/6/geological_taxonomy#Napoleonite
:Napoleonite rdf:type owl:Class ;
             rdfs:subClassOf :Diorite ;
             rdfs:comment """Napoleonite is a variety of diorite which is characterized by orbicular structure.

Resource: https://en.wikipedia.org/wiki/Napoleonite""" .


###  http://www.semanticweb.org/ontologies/2022/6/geological_taxonomy#Natural_disasters
:Natural_disasters rdf:type owl:Class ;
                   rdfs:subClassOf :Geological_phenomena ;
                   owl:disjointWith :Weather_conditions ;
                   rdfs:comment """A natural disaster is \"the negative impact following an actual occurrence of natural hazard in the event that it significantly harms a community\".

Resource: https://en.wikipedia.org/wiki/Natural_disaster

Justification: Classified based on origin, cause of the disaster and due to weather conditions.""" .


###  http://www.semanticweb.org/ontologies/2022/6/geological_taxonomy#Nepheline_syenite
:Nepheline_syenite rdf:type owl:Class ;
                   rdfs:subClassOf :Igneous_rocks ;
                   rdfs:comment """Nepheline syenite is a holocrystalline plutonic rock that consists largely of nepheline and alkali feldspar. 

Resource: https://en.wikipedia.org/wiki/Nepheline_syenite""" .


###  http://www.semanticweb.org/ontologies/2022/6/geological_taxonomy#Nephelinite
:Nephelinite rdf:type owl:Class ;
             rdfs:subClassOf :Igneous_rocks ;
             rdfs:comment """Nephelinite is a fine-grained or aphanitic igneous rock made up almost entirely of nepheline and clinopyroxene.

Resource: https://en.wikipedia.org/wiki/Nephelinite""" .


###  http://www.semanticweb.org/ontologies/2022/6/geological_taxonomy#Norite
:Norite rdf:type owl:Class ;
        rdfs:subClassOf :Igneous_rocks ;
        rdfs:comment """Norite is a mafic intrusive igneous rock composed largely of the calcium-rich plagioclase labradorite, orthopyroxene, and olivine.

Resource: https://en.wikipedia.org/wiki/Norite""" .


###  http://www.semanticweb.org/ontologies/2022/6/geological_taxonomy#Obsidian
:Obsidian rdf:type owl:Class ;
          rdfs:subClassOf :Igneous_rocks ;
          rdfs:comment """Obsidian is an igneous rock that forms when molten rock material cools so rapidly that atoms are unable to arrange themselves into a crystalline structure.

Resource: https://geology.com/rocks/obsidian.shtml""" .


###  http://www.semanticweb.org/ontologies/2022/6/geological_taxonomy#Oceanic_crust
:Oceanic_crust rdf:type owl:Class ;
               rdfs:subClassOf :Crust ;
               rdfs:comment """Oceanic crust is the uppermost layer of the oceanic portion of the tectonic plates composed of dense (mafic) iron magnesium silicate igneous rocks, like basalt.

Resource: https://en.wikipedia.org/wiki/Oceanic_crust""" .


###  http://www.semanticweb.org/ontologies/2022/6/geological_taxonomy#Oceanic_lithosphere
:Oceanic_lithosphere rdf:type owl:Class ;
                     rdfs:subClassOf :Lithosphere ;
                     rdfs:comment """Oceanic lithosphere is associated with oceanic crust and exists in the ocean basins

Resource: https://en.wikipedia.org/wiki/Lithosphere""" .


###  http://www.semanticweb.org/ontologies/2022/6/geological_taxonomy#Oil_shale
:Oil_shale rdf:type owl:Class ;
           rdfs:subClassOf :Sedimentary_rocks ;
           rdfs:comment """A sedimentary rock composed dominantly of organic material

Resource: https://geology.fandom.com/wiki/List_of_rock_types""" .


###  http://www.semanticweb.org/ontologies/2022/6/geological_taxonomy#Oolite
:Oolite rdf:type owl:Class ;
        rdfs:subClassOf :Sedimentary_rocks ;
        rdfs:comment """Sedimentary rock formed from ooids

Resource: https://en.wikipedia.org/wiki/List_of_rock_types""" .


###  http://www.semanticweb.org/ontologies/2022/6/geological_taxonomy#Organic_compounds
:Organic_compounds rdf:type owl:Class ;
                   rdfs:subClassOf :Mineral ;
                   rdfs:comment """The nitrate minerals are characterized by their triangular (NO3)– groups that resemble the (CO3)2– groups of the carbonates, making the two mineral classes similar in structure.	

Resource: https://www.britannica.com/science/nitrate-mineral""" .


###  http://www.semanticweb.org/ontologies/2022/6/geological_taxonomy#Orthels
:Orthels rdf:type owl:Class ;
         rdfs:subClassOf :Gelisols ;
         rdfs:comment """Soils that show little or no cryoturbation (less than one-third of the depth of the active layer)

Resource: https://en.wikipedia.org/wiki/Gelisol#Suborders""" .


###  http://www.semanticweb.org/ontologies/2022/6/geological_taxonomy#Orthents
:Orthents rdf:type owl:Class ;
          rdfs:subClassOf :Entisols ;
          rdfs:comment """Entisols lacking in pedogenic development

Resource: \"Illustrated Guide to Soil Taxonomy\" book by Unites States Department of Agriculture""" .


###  http://www.semanticweb.org/ontologies/2022/6/geological_taxonomy#Orthods
:Orthods rdf:type owl:Class ;
         rdfs:subClassOf :Spodosols ;
         rdfs:comment """Simple Spodosols with varying amounts of illuvial carbon, aluminum, and iron in the spodic horizon

Resource: \"Illustrated Guide to Soil Taxonomy\" book by Unites States Department of Agriculture""" .


###  http://www.semanticweb.org/ontologies/2022/6/geological_taxonomy#Outer_core
:Outer_core rdf:type owl:Class ;
            rdfs:subClassOf :Planetary_core ;
            owl:disjointWith <http://www.semanticweb.org/ontologies/2022/6/geological_taxonomy#Earth's_inner_core> ;
            rdfs:comment """Earth's outer core is a fluid layer about 2,260 km (1,400 mi) thick, composed of mostly iron and nickel that lies above Earth's solid inner core and below its mantle. Pressure of 135–330GPa (from 1.3 to 3.3million atmospheres).

Resource: https://en.wikipedia.org/wiki/Earth%27s_outer_core""" .


###  http://www.semanticweb.org/ontologies/2022/6/geological_taxonomy#Overtopping_of_a_barrier
:Overtopping_of_a_barrier rdf:type owl:Class ;
                          rdfs:subClassOf :Coastal_Floods ;
                          rdfs:comment """the barrier may be natural or human-engineered and overtopping occurs due to swelling conditions during storms or high tides often on open stretches of the coast.	

Resource: https://en.wikipedia.org/wiki/Coastal_flooding""" .


###  http://www.semanticweb.org/ontologies/2022/6/geological_taxonomy#Oxides
:Oxides rdf:type owl:Class ;
        rdfs:subClassOf :Mineral ;
        rdfs:comment """The oxide mineral class includes those minerals in which the oxide anion (O2−) is bonded to one or more metal alloys.	

Resource: https://en.wikipedia.org/wiki/Oxide_mineral

Justification: Classified based on the combination of oxygen with one metal or more than one metals""" .


###  http://www.semanticweb.org/ontologies/2022/6/geological_taxonomy#Oxisols
:Oxisols rdf:type owl:Class ;
         rdfs:subClassOf :Soil ;
         rdfs:comment """The central concept of Oxisols is that of soils of the tropical and subtropical regions. They have gentle slopes on surfaces of great age.

Resource: https://www.nrcs.usda.gov/wps/portal/nrcs/detail/soils/survey/class/maps/?cid=nrcs142p2_053605

Justification: Depening upon soil moisture regime""" .


###  http://www.semanticweb.org/ontologies/2022/6/geological_taxonomy#Pantellerite
:Pantellerite rdf:type owl:Class ;
              rdfs:subClassOf :Rhyolite ;
              rdfs:comment """Pantellerite is a type of volcanic rock, specifically a peralkaline rhyolite. It has a higher iron and lower aluminium composition than comendite.

Resource: https://en.wikipedia.org/wiki/Pantellerite""" .


###  http://www.semanticweb.org/ontologies/2022/6/geological_taxonomy#Pegmatite
:Pegmatite rdf:type owl:Class ;
           rdfs:subClassOf :Igneous_rocks ;
           rdfs:comment """A pegmatite is an igneous rock showing a very coarse texture, with large interlocking crystals usually greater in size than 1 cm (0.4 in) and sometimes greater than 1 meter (3 ft).

Resource: https://en.wikipedia.org/wiki/Pegmatite""" .


###  http://www.semanticweb.org/ontologies/2022/6/geological_taxonomy#Peridotite
:Peridotite rdf:type owl:Class ;
            rdfs:subClassOf :Igneous_rocks ;
            rdfs:comment """Peridotite is a dense, coarse-grained igneous rock consisting mostly of the silicate minerals olivine and pyroxene.

Resource: https://en.wikipedia.org/wiki/Peridotite""" .


###  http://www.semanticweb.org/ontologies/2022/6/geological_taxonomy#Perox
:Perox rdf:type owl:Class ;
       rdfs:subClassOf :Oxisols ;
       rdfs:comment """Oxisols that have a perudic moisture regime

Resource: https://sites.google.com/site/dinpuithai/Home/key10/key10e""" .


###  http://www.semanticweb.org/ontologies/2022/6/geological_taxonomy#Phonolite
:Phonolite rdf:type owl:Class ;
           rdfs:subClassOf :Igneous_rocks ;
           rdfs:comment """Phonolite is an uncommon extrusive rock, of intermediate chemical composition between felsic and mafic, with texture ranging from aphanitic (fine-grained) to porphyritic.

Resource: https://en.wikipedia.org/wiki/Phonolite""" .


###  http://www.semanticweb.org/ontologies/2022/6/geological_taxonomy#Phonotephrite
:Phonotephrite rdf:type owl:Class ;
               rdfs:subClassOf :Igneous_rocks ;
               rdfs:comment """Phonotephrite is a strongly alkaline volcanic rock with a composition between phonolite and tephrite.

Resource: https://en.wikipedia.org/wiki/Phonotephrite""" .


###  http://www.semanticweb.org/ontologies/2022/6/geological_taxonomy#Phosphates_Arsenates_Vanadates
:Phosphates_Arsenates_Vanadates rdf:type owl:Class ;
                                rdfs:subClassOf :Mineral ;
                                rdfs:comment """Phosphate minerals contain the tetrahedrally coordinated phosphate anion along sometimes with arsenate and vanadate substitutions, and chloride, fluoride, and hydroxide anions that also fit into the crystal structure.	

Resource: https://en.wikipedia.org/wiki/Phosphate_mineral""" .


###  http://www.semanticweb.org/ontologies/2022/6/geological_taxonomy#Phosphorite
:Phosphorite rdf:type owl:Class ;
             rdfs:subClassOf :Sedimentary_rocks ;
             rdfs:comment """Phosphorite is a sedimentary rock containing significant amount of phosphate material.

Resource: https://www.sandatlas.org/rock-types/""" .


###  http://www.semanticweb.org/ontologies/2022/6/geological_taxonomy#Phyllite
:Phyllite rdf:type owl:Class ;
          rdfs:subClassOf :Metamorphic_rocks ;
          rdfs:comment """Type of foliated metamorphic rock – A low grade metamorphic rock composed mostly of micaceous minerals

Resource: https://en.wikipedia.org/wiki/Phyllite""" .


###  http://www.semanticweb.org/ontologies/2022/6/geological_taxonomy#Picrite
:Picrite rdf:type owl:Class ;
         rdfs:subClassOf :Igneous_rocks ;
         rdfs:comment """Picrite, intrusive igneous rock of ultramafic (very silica-poor) composition that is composed largely of olivine and augite and is somewhat similar to peridotite. Picrites are dark, heavy rocks and contain a small but variable amount of plagioclase feldspar; hornblende and biotite may also be present.

Resource: https://www.britannica.com/science/picrite""" .


###  http://www.semanticweb.org/ontologies/2022/6/geological_taxonomy#Planetary_core
:Planetary_core rdf:type owl:Class ;
                rdfs:subClassOf :Units_of_Earth_structure ;
                rdfs:comment """Innermost layers of a planet

Resource: https://en.wikipedia.org/wiki/Planetary_core

Justification: Classified based on temperature , pressure , radius""" .


###  http://www.semanticweb.org/ontologies/2022/6/geological_taxonomy#Porphyry
:Porphyry rdf:type owl:Class ;
          rdfs:subClassOf :Igneous_rocks ;
          rdfs:comment """Porphyry is a textural term for an igneous rock consisting of coarse-grained crystals such as feldspar or quartz dispersed in a fine-grained silicate-rich, generally aphanitic matrix or groundmass.

Resource: https://en.wikipedia.org/wiki/Porphyry_(geology)""" .


###  http://www.semanticweb.org/ontologies/2022/6/geological_taxonomy#Primary_rockfalls
:Primary_rockfalls rdf:type owl:Class ;
                   rdfs:subClassOf :Rockfall ;
                   owl:disjointWith :Secondary_rockfalls ;
                   rdfs:comment """The material then descends mainly through the air by falling, bouncing, or rolling

Resource: https://en.wikipedia.org/wiki/Landslide_classification#Types_and_classification""" .


###  http://www.semanticweb.org/ontologies/2022/6/geological_taxonomy#Progressive_creep
:Progressive_creep rdf:type owl:Class ;
                   rdfs:subClassOf :Creep ;
                   rdfs:comment """Slopes are reaching the point of failure as other types of mass movements.

Resource: https://www.nature.scot/landforms-and-geology/scotlands-rocks-landforms-and-soils/landforms/landslides/types-landslide""" .


###  http://www.semanticweb.org/ontologies/2022/6/geological_taxonomy#Psamments
:Psamments rdf:type owl:Class ;
           rdfs:subClassOf :Entisols ;
           rdfs:comment """Entisols dominated by sandy textures

Resource: \"Illustrated Guide to Soil Taxonomy\" book by Unites States Department of Agriculture""" .


###  http://www.semanticweb.org/ontologies/2022/6/geological_taxonomy#Pseudotachylite
:Pseudotachylite rdf:type owl:Class ;
                 rdfs:subClassOf :Metamorphic_rocks ;
                 rdfs:comment """Pseudotachylyte or Pseudotachylite is a cohesive glassy or very fine-grained rock that occurs as veins and often contains inclusions of wall-rock fragments.

Resource: https://en.wikipedia.org/wiki/Pseudotachylite""" .


###  http://www.semanticweb.org/ontologies/2022/6/geological_taxonomy#Pumice
:Pumice rdf:type owl:Class ;
        rdfs:subClassOf :Igneous_rocks ;
        rdfs:comment """Pumice, called pumicite in its powdered or dust form, is a volcanic rock that consists of highly vesicular rough-textured volcanic glass, which may or may not contain crystals. It is typically light-colored.

Resource: https://en.wikipedia.org/wiki/Pumice""" .


###  http://www.semanticweb.org/ontologies/2022/6/geological_taxonomy#Pyroxenite
:Pyroxenite rdf:type owl:Class ;
            rdfs:subClassOf :Igneous_rocks ;
            rdfs:comment """Igneous rock - a coarse grained plutonic rock composed of >90% pyroxene

Resource: https://en.wikipedia.org/wiki/Pyroxenite""" .


###  http://www.semanticweb.org/ontologies/2022/6/geological_taxonomy#Pāhoehoe
:Pāhoehoe rdf:type owl:Class ;
          rdfs:subClassOf :Basalt ;
          rdfs:comment """Basaltic lava with a flowing, often ropy appearance

Resource: https://en.wikipedia.org/wiki/P%C4%81hoehoe""" .


###  http://www.semanticweb.org/ontologies/2022/6/geological_taxonomy#Quartz_diorite
:Quartz_diorite rdf:type owl:Class ;
                rdfs:subClassOf :Igneous_rocks ;
                rdfs:comment """Igneous, plutonic rock – A diorite with >5% modal quartz

Resource: https://en.wikipedia.org/wiki/Quartz_diorite""" .


###  http://www.semanticweb.org/ontologies/2022/6/geological_taxonomy#Quartz_monzonite
:Quartz_monzonite rdf:type owl:Class ;
                  rdfs:subClassOf :Igneous_rocks ;
                  rdfs:comment """Type of igneous rock – An intermediate plutonic rock, essentially a monzonite with 5–10% modal quartz

Resource: https://en.wikipedia.org/wiki/Quartz_monzonite""" .


###  http://www.semanticweb.org/ontologies/2022/6/geological_taxonomy#Quartzite
:Quartzite rdf:type owl:Class ;
           rdfs:subClassOf :Metamorphic_rocks ;
           rdfs:comment """A metamorphosed sandstone typically composed of >95% quartz

Resource: https://geology.fandom.com/wiki/List_of_rock_types""" .


###  http://www.semanticweb.org/ontologies/2022/6/geological_taxonomy#Quartzolite
:Quartzolite rdf:type owl:Class ;
             rdfs:subClassOf :Igneous_rocks ;
             rdfs:comment """Extremely rare igneous rock made mostly of quartz – An intrusive rock composed mostly of quartz

Resource: https://en.wikipedia.org/wiki/Quartzolite""" .


###  http://www.semanticweb.org/ontologies/2022/6/geological_taxonomy#Rain
:Rain rdf:type owl:Class ;
      rdfs:subClassOf :Weather_conditions ;
      rdfs:comment """Rain is the condensed moisture of the atmosphere above falling under the form of liquid droplets. It is an extremely important phenomenon that allows life to flourish on continents

Resource: https://weather.fandom.com/wiki/Types_of_Weather#Rain""" .


###  http://www.semanticweb.org/ontologies/2022/6/geological_taxonomy#Rapakivi
:Rapakivi rdf:type owl:Class ;
          rdfs:subClassOf :Igneous_rocks ;
          rdfs:comment """Rapakivi is a variety of granite with K-feldspar phenocrysts that are mantled with plagioclase

Resource: https://www.sandatlas.org/rock-types/#Rapakivi""" .


###  http://www.semanticweb.org/ontologies/2022/6/geological_taxonomy#Rendolls
:Rendolls rdf:type owl:Class ;
          rdfs:subClassOf :Mollisols ;
          rdfs:comment """Rendolls are shallow and stony soils formed on limestone and have an udic Soil moisture regime

Resource: https://www.sciencedirect.com/topics/agricultural-and-biological-sciences/mollisol""" .


###  http://www.semanticweb.org/ontologies/2022/6/geological_taxonomy#Rhomb-porphyry
:Rhomb-porphyry rdf:type owl:Class ;
                rdfs:subClassOf :Igneous_rocks ;
                rdfs:comment """Rhomb-porphyry is a porphyritic igneous rock with abundant wedge- or lens-shaped anorthoclase (feldspar) phenocrysts. Rhomb-porphyry is a rare rock type.

Resource: https://www.sandatlas.org/rhomb-porphyry/""" .


###  http://www.semanticweb.org/ontologies/2022/6/geological_taxonomy#Rhyodacite
:Rhyodacite rdf:type owl:Class ;
            rdfs:subClassOf :Igneous_rocks ;
            rdfs:comment """Volcanic rock rich in silica and low in alkali metal oxides – A felsic volcanic rock which is intermediate between a rhyolite and a dacite

Resource: https://en.wikipedia.org/wiki/Rhyodacite""" .


###  http://www.semanticweb.org/ontologies/2022/6/geological_taxonomy#Rhyolite
:Rhyolite rdf:type owl:Class ;
          rdfs:subClassOf :Igneous_rocks ;
          rdfs:comment """Rhyolite is the most silica-rich of volcanic rocks. It is generally glassy or fine-grained (aphanitic) in texture, but may be porphyritic, containing larger mineral crystals (phenocrysts) in an otherwise fine-grained groundmass.

Resource: https://en.wikipedia.org/wiki/Rhyolite

Justification: Depending upon the composition of iron and aluminium.""" .


###  http://www.semanticweb.org/ontologies/2022/6/geological_taxonomy#Rock
:Rock rdf:type owl:Class ;
      rdfs:subClassOf :Geological_Object ;
      rdfs:comment """In geology, a rock (or stone) is any naturally occurring solid mass or aggregate of minerals or mineraloid matter without any chemical composition

Resource: https://en.wikipedia.org/wiki/Rock_(geology)

Justification: Depending upon the mode of their formation""" .


###  http://www.semanticweb.org/ontologies/2022/6/geological_taxonomy#Rock_Gypsum-
:Rock_Gypsum- rdf:type owl:Class ;
              rdfs:subClassOf :Sedimentary_rocks ;
              rdfs:comment """Rock gypsum (a.k.a. gyprock) is a chemical sedimentary rock.  It is an example of an evaporite - it forms by the evaporation of water (usually seawater) and the precipitation of dissolved minerals.

Resource: http://www.jsjgeology.net/Rock-gypsum.htm""" .


###  http://www.semanticweb.org/ontologies/2022/6/geological_taxonomy#Rock_slide
:Rock_slide rdf:type owl:Class ;
            rdfs:subClassOf :Block_slide ;
            rdfs:comment """sliding of rock material down a mountain

Resource: https://www.geologyin.com/2015/02/types-of-wasting-slump-rockslide-debris.html""" .


###  http://www.semanticweb.org/ontologies/2022/6/geological_taxonomy#Rock_topples
:Rock_topples rdf:type owl:Class ;
              rdfs:subClassOf :Topples ;
              rdfs:comment """A topple is the forward rotation, out of the slope, of a mass of soil and rock about a point or axis below the centre of gravity of the displaced mass.

Resource: http://www.ukgeohazards.info/pages/eng_geol/landslide_geohazard/eng_geol_landslides_rocktopple_index.htm""" .


###  http://www.semanticweb.org/ontologies/2022/6/geological_taxonomy#Rockfall
:Rockfall rdf:type owl:Class ;
          rdfs:subClassOf :Falls ;
          rdfs:comment """A rockfall is a quantity of rock that has fallen freely from a cliff face.

Resource: https://en.wikipedia.org/wiki/Rockfall

Justification: Classified based on how detaching of bodies happen""" .


###  http://www.semanticweb.org/ontologies/2022/6/geological_taxonomy#Rotational_slides
:Rotational_slides rdf:type owl:Class ;
                   rdfs:subClassOf :Slides ;
                   owl:disjointWith :Translational_slide ;
                   rdfs:comment """Rotational slides move along a surface of rupture that is curved and concave

Resource: https://en.wikipedia.org/wiki/Landslide_classification#Types_and_classification""" .


###  http://www.semanticweb.org/ontologies/2022/6/geological_taxonomy#Salids
:Salids rdf:type owl:Class ;
        rdfs:subClassOf :Aridisols ;
        rdfs:comment """Characterized by accumulation of salts more soluble than gypsum; the typical soils of the playas or desert depressions, or closed basins.

Resource: https://www.sciencedirect.com/topics/agricultural-and-biological-sciences/aridisol""" .


###  http://www.semanticweb.org/ontologies/2022/6/geological_taxonomy#Sandstone
:Sandstone rdf:type owl:Class ;
           rdfs:subClassOf :Sedimentary_rocks ;
           rdfs:comment """A clastic sedimentary rock defined by its grain size

Resource: https://geology.fandom.com/wiki/List_of_rock_types""" .


###  http://www.semanticweb.org/ontologies/2022/6/geological_taxonomy#Saprists
:Saprists rdf:type owl:Class ;
          rdfs:subClassOf :Histosols ;
          rdfs:comment """Histosols that are primarily made up of highly decomposed organic materials, often called muck.

Resource: https://en.wikipedia.org/wiki/Histosol""" .


###  http://www.semanticweb.org/ontologies/2022/6/geological_taxonomy#Schist
:Schist rdf:type owl:Class ;
        rdfs:subClassOf :Metamorphic_rocks ;
        rdfs:comment """Schist is a medium-grained metamorphic rock showing pronounced schistosity.

Resource: https://en.wikipedia.org/wiki/Schist""" .


###  http://www.semanticweb.org/ontologies/2022/6/geological_taxonomy#Scoria
:Scoria rdf:type owl:Class ;
        rdfs:subClassOf :Igneous_rocks ;
        rdfs:comment """Scoria is a pyroclastic, highly vesicular, dark-colored volcanic rock that was ejected from a volcano as a molten blob and cooled in the air to form discrete grains or clasts.

Resource: https://en.wikipedia.org/wiki/Scoria""" .


###  http://www.semanticweb.org/ontologies/2022/6/geological_taxonomy#Seasonal_creep
:Seasonal_creep rdf:type owl:Class ;
                rdfs:subClassOf :Creep ;
                rdfs:comment """Movement is within the depth of soil affected by seasonal changes in soil moisture and soil temperature

Resource: https://courses.lumenlearning.com/geo/chapter/reading-slump-and-creep/""" .


###  http://www.semanticweb.org/ontologies/2022/6/geological_taxonomy#Secondary_rockfalls
:Secondary_rockfalls rdf:type owl:Class ;
                     rdfs:subClassOf :Rockfall ;
                     rdfs:comment """Secondary falls involves rock bodies already physically detached from cliff and merely lodged upon it

Resource: https://en.wikipedia.org/wiki/Landslide_classification#Types_and_classification""" .


###  http://www.semanticweb.org/ontologies/2022/6/geological_taxonomy#Sedimentary_rocks
:Sedimentary_rocks rdf:type owl:Class ;
                   rdfs:subClassOf :Rock ;
                   rdfs:comment """Sedimentary rocks are types of rock that are formed by the accumulation or deposition of mineral or organic particles at Earth's surface, followed by cementation.

Resource: https://en.wikipedia.org/wiki/Sedimentary_rock

Justification: depending upon the composition of different minerals and amount of organic material""" .


###  http://www.semanticweb.org/ontologies/2022/6/geological_taxonomy#Serpentinite
:Serpentinite rdf:type owl:Class ;
              rdfs:subClassOf :Metamorphic_rocks ;
              rdfs:comment """Serpentinite is a rock composed of one or more serpentine group minerals, the name originating from the similarity of the texture of the rock to that of the skin of a snake.

Resource: https://en.wikipedia.org/wiki/Serpentinite""" .


###  http://www.semanticweb.org/ontologies/2022/6/geological_taxonomy#Severe_Drought
:Severe_Drought rdf:type owl:Class ;
                rdfs:subClassOf :Drought ;
                rdfs:comment """It is D2 category and causes water shortages

Resource: https://droughtmonitor.unl.edu/About/WhatistheUSDM.aspx""" .


###  http://www.semanticweb.org/ontologies/2022/6/geological_taxonomy#Shale
:Shale rdf:type owl:Class ;
       rdfs:subClassOf :Sedimentary_rocks ;
       rdfs:comment """Shale is a fine-grained, clastic sedimentary rock formed from mud that is a mix of flakes of clay minerals and tiny fragments (silt-sized particles) of other minerals, especially quartz and calcite.

Resource: https://en.wikipedia.org/wiki/Shale""" .


###  http://www.semanticweb.org/ontologies/2022/6/geological_taxonomy#Shonkinite
:Shonkinite rdf:type owl:Class ;
            rdfs:subClassOf :Igneous_rocks ;
            rdfs:comment """Shonkinite is an intrusive igneous rock found in few places in the world. It is unique in having low silica, feldspathoid minerals, and large blocky crystals of black augite.

Resource: https://en.wikipedia.org/wiki/Shonkinite""" .


###  http://www.semanticweb.org/ontologies/2022/6/geological_taxonomy#Shoshonite
:Shoshonite rdf:type owl:Class ;
            rdfs:subClassOf :Trachyandesite ;
            rdfs:comment """Shoshonite is a potassium-rich variety of basaltic trachyandesite, composed of olivine, augite and plagioclase phenocrysts in a groundmass with calcic plagioclase and sanidine and some dark-colored volcanic glass.

Resource: https://en.wikipedia.org/wiki/List_of_rock_types""" .


###  http://www.semanticweb.org/ontologies/2022/6/geological_taxonomy#Shungite
:Shungite rdf:type owl:Class ;
          rdfs:subClassOf :Metamorphic_rocks ;
          rdfs:comment """Shungite is a metamorphosed oil shale consisting of structureless carbon.

Resource: https://www.sandatlas.org/rock-types/""" .


###  http://www.semanticweb.org/ontologies/2022/6/geological_taxonomy#Silicates
:Silicates rdf:type owl:Class ;
           rdfs:subClassOf :Mineral ;
           rdfs:comment """Silicate minerals are rock-forming minerals made up of silicate groups.	

Resource: https://en.wikipedia.org/wiki/Silicate_mineral

Justification: Classified according to structural configuration, which arises from the sharing of one, two, three, or all oxygen ions of a tetrahedron.
https://www.britannica.com/science/mineral-chemical-compound/Silicates""" .


###  http://www.semanticweb.org/ontologies/2022/6/geological_taxonomy#Siltstone
:Siltstone rdf:type owl:Class ;
           rdfs:subClassOf :Sedimentary_rocks ;
           rdfs:comment """A clastic sedimentary rock defined by its grain size

Resource: https://geology.fandom.com/wiki/List_of_rock_types""" .


###  http://www.semanticweb.org/ontologies/2022/6/geological_taxonomy#Skarn
:Skarn rdf:type owl:Class ;
       rdfs:subClassOf :Metamorphic_rocks ;
       rdfs:comment """Skarns or tactites are hard, coarse-grained metamorphic rocks that form by a process called metasomatism.

Resource: https://en.wikipedia.org/wiki/Skarn""" .


###  http://www.semanticweb.org/ontologies/2022/6/geological_taxonomy#Slate
:Slate rdf:type owl:Class ;
       rdfs:subClassOf :Metamorphic_rocks ;
       rdfs:comment """Slate is a fine-grained, foliated, homogeneous metamorphic rock derived from an original shale-type sedimentary rock composed of clay or volcanic ash through low-grade regional metamorphism.

Resource: https://en.wikipedia.org/wiki/Slate""" .


###  http://www.semanticweb.org/ontologies/2022/6/geological_taxonomy#Slides
:Slides rdf:type owl:Class ;
        rdfs:subClassOf :Landslide ;
        rdfs:comment """A slide is a downslope movement of soil or rock mass occurring dominantly on the surface of rupture or on relatively thin zones of intense shear strain

Resource: https://en.wikipedia.org/wiki/Landslide_classification#Types_and_classification

Justification: Classified based on how the land of mass slides""" .


###  http://www.semanticweb.org/ontologies/2022/6/geological_taxonomy#Snow
:Snow rdf:type owl:Class ;
      rdfs:subClassOf :Weather_conditions ;
      rdfs:comment """Snow is atmospheric water that froze and fell to the ground, covering it. It happens when the temperature of the air falls at 0 °C (32 °F). Snow remains as long as the temperature of the ground doesn't go beyond 0 °C (32 °F).

Resource: https://weather.fandom.com/wiki/Types_of_Weather#Snow""" .


###  http://www.semanticweb.org/ontologies/2022/6/geological_taxonomy#Soapstone
:Soapstone rdf:type owl:Class ;
           rdfs:subClassOf :Talc_carbonate ;
           rdfs:comment """Soapstone is a soft rock composed of talc with other silicates like micas, pyroxene, amphibole, chlorite, etc.

Resource: https://www.sandatlas.org/rock-types/""" .


###  http://www.semanticweb.org/ontologies/2022/6/geological_taxonomy#Soil
:Soil rdf:type owl:Class ;
      rdfs:subClassOf :Geological_Object ;
      rdfs:comment """Soil, also commonly referred to as earth or dirt, is a mixture of organic matter, minerals, gases, liquids, and organisms that together support life.Soil consists of a solid phase of minerals and organic matter (the soil matrix), as well as a porous phase that holds gases (the soil atmosphere) and water (the soil solution).

Resource: https://en.wikipedia.org/wiki/Soil

Justification: Categorized based on the soil properties like depth, moisture, temperature, texture, structure, cation exchange capacity, base saturation, clay mineralogy, organic matter content and salt content. 
https://en.wikipedia.org/wiki/USDA_soil_taxonomy""" .


###  http://www.semanticweb.org/ontologies/2022/6/geological_taxonomy#Sovite
:Sovite rdf:type owl:Class ;
        rdfs:subClassOf :Igneous_rocks ;
        rdfs:comment """Sövite is a type of plutonic carbonatite where the dominant carbonate mineral is calcite. Sövite is the most common variety of carbonatite.

Resource: https://www.sandatlas.org/rock-types/#S%C3%B6vite""" .


###  http://www.semanticweb.org/ontologies/2022/6/geological_taxonomy#Spodosols
:Spodosols rdf:type owl:Class ;
           rdfs:subClassOf :Soil ;
           rdfs:comment """The central concept of Spodosols is that of soils in which amorphous mixtures of organic matter and aluminum, with or without iron, have accumulated.

Resource: https://www.nrcs.usda.gov/wps/portal/nrcs/detail/soils/survey/class/maps/?cid=nrcs142p2_053607

Justification: Based on soil wetness, cold soil temperatures, spodic horizons dominated by illuvial accumulation of organic matter, and varying amounts of illuvial carbon, aluminum, and iron in the spodic horizons
\"Illustrated Guide to Soil Taxonomy\" book by Unites States Department of Agriculture""" .


###  http://www.semanticweb.org/ontologies/2022/6/geological_taxonomy#Stormy
:Stormy rdf:type owl:Class ;
        rdfs:subClassOf :Weather_conditions ;
        rdfs:comment """A storm is any disturbed state of the natural environment or the atmosphere of an astronomical body. It may be marked by significant disruptions to normal conditions such as strong wind, tornadoes, hail, thunder and lightning (a thunderstorm), heavy precipitation (snowstorm, rainstorm), heavy freezing rain (ice storm), strong winds (tropical cyclone, windstorm), wind transporting some substance through the atmosphere such as in a dust storm, among other forms of severe weather.

Resource: https://en.wikipedia.org/wiki/Storm""" .


###  http://www.semanticweb.org/ontologies/2022/6/geological_taxonomy#Subsidence
:Subsidence rdf:type owl:Class ;
            rdfs:subClassOf :Landslide ;
            rdfs:comment "Subsidence is a general term for downward vertical movement of the Earth's surface, which can be caused by both natural processes and human activities." .


###  http://www.semanticweb.org/ontologies/2022/6/geological_taxonomy#Suevite
:Suevite rdf:type owl:Class ;
         rdfs:subClassOf :Metamorphic_rocks ;
         rdfs:comment """Suevite is a rock consisting partly of melted material, typically forming a breccia containing glass and crystal or lithic fragments, formed during an impact event.

Resource: https://en.wikipedia.org/wiki/Suevite""" .


###  http://www.semanticweb.org/ontologies/2022/6/geological_taxonomy#Sulfates
:Sulfates rdf:type owl:Class ;
          rdfs:subClassOf :Mineral ;
          rdfs:comment """The sulfate minerals are a class of minerals that include the sulfate ion within their structure.	

Resource: https://en.wikipedia.org/wiki/Sulfate_mineral

Justification: Classification depending upon presence of water in the chemical structure""" .


###  http://www.semanticweb.org/ontologies/2022/6/geological_taxonomy#Sulfides_and_Sulfosalts
:Sulfides_and_Sulfosalts rdf:type owl:Class ;
                         rdfs:subClassOf :Mineral ;
                         rdfs:comment """The sulfide minerals are a class of minerals containing sulfide or disulfide as the major anion.	

Resource: https://en.wikipedia.org/wiki/Sulfide_mineral""" .


###  http://www.semanticweb.org/ontologies/2022/6/geological_taxonomy#Sunny
:Sunny rdf:type owl:Class ;
       rdfs:subClassOf :Weather_conditions ;
       rdfs:comment """A sunny day, or clear sky during nighttime, is when there are clouds above the horizon.

Resource: https://weather.fandom.com/wiki/Types_of_Weather#Sunny/Clear""" .


###  http://www.semanticweb.org/ontologies/2022/6/geological_taxonomy#Surface_Fire
:Surface_Fire rdf:type owl:Class ;
              rdfs:subClassOf :Wildfire ;
              rdfs:comment """A surface fire refers to a fire that ranges from low to high intensity depending on the conditions.  burn on the surface of the ground and are primarily fueled by low-lying vegetation such as twigs or dried leaves.	

Resource: https://www.supplycache.com/blogs/news/the-different-types-of-wildland-fires""" .


###  http://www.semanticweb.org/ontologies/2022/6/geological_taxonomy#Syenite
:Syenite rdf:type owl:Class ;
         rdfs:subClassOf :Igneous_rocks ;
         rdfs:comment """Intrusive igneous rock – A plutonic rock dominated by orthoclase feldspar; a type of granitoid

Resource: https://en.wikipedia.org/wiki/Syenite""" .


###  http://www.semanticweb.org/ontologies/2022/6/geological_taxonomy#Sylvinite
:Sylvinite rdf:type owl:Class ;
           rdfs:subClassOf :Sedimentary_rocks ;
           rdfs:comment """A sedimentary rock made of a mechanical mixture of sylvite and halite

Resource: https://en.wikipedia.org/wiki/List_of_rock_types""" .


###  http://www.semanticweb.org/ontologies/2022/6/geological_taxonomy#Sövite
:Sövite rdf:type owl:Class ;
        rdfs:subClassOf :Igneous_rocks ;
        rdfs:comment """Sovite (or sövite) is the coarse-grained variety (or facies) of carbonatite, an intrusive, igneous rock. 

Resource: https://en.wikipedia.org/wiki/Sovite""" .


###  http://www.semanticweb.org/ontologies/2022/6/geological_taxonomy#Tachylyte
:Tachylyte rdf:type owl:Class ;
           rdfs:subClassOf :Igneous_rocks ;
           rdfs:comment """Tachylite is a form of basaltic volcanic glass. This glass is formed naturally by the rapid cooling of molten basalt. It is a type of mafic igneous rock.

Resource: https://en.wikipedia.org/wiki/Tachylite""" .


###  http://www.semanticweb.org/ontologies/2022/6/geological_taxonomy#Talc_carbonate
:Talc_carbonate rdf:type owl:Class ;
                rdfs:subClassOf :Metamorphic_rocks ;
                rdfs:comment """Talc carbonates are a suite of rock and mineral compositions found in metamorphosed ultramafic rocks.

Resource: https://en.wikipedia.org/wiki/Talc_carbonate

Justification: Depending upon the amounts of chlorite and amphiboles""" .


###  http://www.semanticweb.org/ontologies/2022/6/geological_taxonomy#Tectonic_Earthquakes
:Tectonic_Earthquakes rdf:type owl:Class ;
                      rdfs:subClassOf :Earthquakes ;
                      rdfs:comment """Tectonic earthquakes are produced by sudden movement along faults and plate boundaries.

Resource: https://www.phivolcs.dost.gov.ph/index.php/earthquake/introduction-to-earthquake

Justification: depending upon where the earthquake takes place considering the plates""" .


###  http://www.semanticweb.org/ontologies/2022/6/geological_taxonomy#Tectonite
:Tectonite rdf:type owl:Class ;
           rdfs:subClassOf :Metamorphic_rocks ;
           rdfs:comment """Tectonites are metamorphic or tectonically deformed rocks whose fabric reflects the history of their deformation, or rocks with fabric that clearly displays coordinated geometric features that indicate continuous solid (ductile) flow during formation.

Resource: https://en.wikipedia.org/wiki/Tectonite""" .


###  http://www.semanticweb.org/ontologies/2022/6/geological_taxonomy#Teletsunamis
:Teletsunamis rdf:type owl:Class ;
              rdfs:subClassOf :Tsunami ;
              rdfs:comment """waves generated more then 1000 kilometers from the affected shore. 	

Resource: http://www.sfu.ca/geog355fall01/cobryne/types_of_tsunamis.html""" .


###  http://www.semanticweb.org/ontologies/2022/6/geological_taxonomy#Tephriphonolite
:Tephriphonolite rdf:type owl:Class ;
                 rdfs:subClassOf :Igneous_rocks ;
                 rdfs:comment """Tephriphonolite is a mafic to intermediate extrusive igneous rock in composition between phonotephrite and phonolite.[1] It contains 9 to 14% alkali content and 48 to 57% silica content.

Resource: https://en.wikipedia.org/wiki/Tephriphonolite""" .


###  http://www.semanticweb.org/ontologies/2022/6/geological_taxonomy#Tephrite
:Tephrite rdf:type owl:Class ;
          rdfs:subClassOf :Igneous_rocks ;
          rdfs:comment """Tephrite is an igneous, volcanic (extrusive) rock, with aphanitic to porphyritic texture

Resource: https://en.wikipedia.org/wiki/Tephrite""" .


###  http://www.semanticweb.org/ontologies/2022/6/geological_taxonomy#Tillite
:Tillite rdf:type owl:Class ;
         rdfs:subClassOf :Sedimentary_rocks ;
         rdfs:comment """Tillite is a poorly sorted glacial sedimentary rock — consolidated glacial till.

Resource: https://www.sandatlas.org/rock-types/""" .


###  http://www.semanticweb.org/ontologies/2022/6/geological_taxonomy#Tonalite
:Tonalite rdf:type owl:Class ;
          rdfs:subClassOf :Igneous_rocks ;
          rdfs:comment """Tonalite is an igneous, plutonic (intrusive) rock, of felsic composition, with phaneritic (coarse-grained) texture.

Resource: https://en.wikipedia.org/wiki/Tonalite""" .


###  http://www.semanticweb.org/ontologies/2022/6/geological_taxonomy#Topples
:Topples rdf:type owl:Class ;
         rdfs:subClassOf :Landslide ;
         rdfs:comment """Toppling is the forward rotation out of the slope of a mass of soil or rock about a point or axis below the centre of gravity of the displaced mass.

Resource: https://en.wikipedia.org/wiki/Landslide_classification#Types_and_classification

Justification: Divided based on type of material""" .


###  http://www.semanticweb.org/ontologies/2022/6/geological_taxonomy#Torrands
:Torrands rdf:type owl:Class ;
          rdfs:subClassOf :Andisols ;
          rdfs:comment """Andisols that have an aridic moisture regime. 

Resource: https://sites.google.com/site/dinpuithai/Home/key10/key10d""" .


###  http://www.semanticweb.org/ontologies/2022/6/geological_taxonomy#Torrerts
:Torrerts rdf:type owl:Class ;
          rdfs:subClassOf :Vertisols ;
          rdfs:comment """Vertisols that, if not irrigated during the year, have cracks in normal years that remain closed for less than 60 consecutive days during a period when the soil temperature at a depth of 50 cm from the soil surface is higher than 8 oC.

Resource: https://sites.google.com/site/dinpuithai/Home/key10/key10f""" .


###  http://www.semanticweb.org/ontologies/2022/6/geological_taxonomy#Torrox
:Torrox rdf:type owl:Class ;
        rdfs:subClassOf :Oxisols ;
        rdfs:comment """Oxisols that have an aridic moisture regime

Resource: https://sites.google.com/site/dinpuithai/Home/key10/key10e""" .


###  http://www.semanticweb.org/ontologies/2022/6/geological_taxonomy#Trachyandesite
:Trachyandesite rdf:type owl:Class ;
                rdfs:subClassOf :Igneous_rocks ;
                rdfs:comment """Trachyandesite is an extrusive igneous rock with a composition between trachyte and andesite.

Resource: https://en.wikipedia.org/wiki/Trachyandesite

Justification: divided into sodium-rich benmoreite and potassium-rich latite.""" .


###  http://www.semanticweb.org/ontologies/2022/6/geological_taxonomy#Trachybasalt
:Trachybasalt rdf:type owl:Class ;
              rdfs:subClassOf :Igneous_rocks ;
              rdfs:comment """Trachybasalt is a volcanic rock with a composition between trachyte and basalt. It resembles basalt but has a high content of alkali metal oxides.

Resource: https://en.wikipedia.org/wiki/Trachybasalt""" .


###  http://www.semanticweb.org/ontologies/2022/6/geological_taxonomy#Trachyte
:Trachyte rdf:type owl:Class ;
          rdfs:subClassOf :Igneous_rocks ;
          rdfs:comment """Trachyte is an extrusive igneous rock composed mostly of alkali feldspar.

Resource: https://en.wikipedia.org/wiki/Trachyte""" .


###  http://www.semanticweb.org/ontologies/2022/6/geological_taxonomy#Translational_slide
:Translational_slide rdf:type owl:Class ;
                     rdfs:subClassOf :Slides ;
                     rdfs:comment """In translational slides the mass displaces along a planar or undulating surface of rupture, sliding out over the original ground surface.

Resource: https://en.wikipedia.org/wiki/Landslide_classification#Types_and_classification""" .


###  http://www.semanticweb.org/ontologies/2022/6/geological_taxonomy#Travertine
:Travertine rdf:type owl:Class ;
            rdfs:subClassOf :Sedimentary_rocks ;
            rdfs:comment """A sedimentary rock containing calcite and iron oxides

Resource: https://geology.fandom.com/wiki/List_of_rock_types""" .


###  http://www.semanticweb.org/ontologies/2022/6/geological_taxonomy#Troctolite
:Troctolite rdf:type owl:Class ;
            rdfs:subClassOf :Igneous_rocks ;
            rdfs:comment """Troctolite is a mafic intrusive rock type. It consists essentially of major but variable amounts of olivine and calcic plagioclase along with minor pyroxene.

Resource: https://en.wikipedia.org/wiki/Troctolite""" .


###  http://www.semanticweb.org/ontologies/2022/6/geological_taxonomy#Trondhjemite
:Trondhjemite rdf:type owl:Class ;
              rdfs:subClassOf :Igneous_rocks ;
              rdfs:comment """Light-colored intrusive igneous rock – A form of tonalite where plagioclase-group feldspar is oligoclase

Resource: https://en.wikipedia.org/wiki/Trondhjemite""" .


###  http://www.semanticweb.org/ontologies/2022/6/geological_taxonomy#Tropical_Depression
:Tropical_Depression rdf:type owl:Class ;
                     rdfs:subClassOf :Tropical_cyclone ;
                     rdfs:comment """A tropical cyclone with maximum sustained winds of 38 mph (33 knots) or less

Resource: https://www.nhc.noaa.gov/climo/""" .


###  http://www.semanticweb.org/ontologies/2022/6/geological_taxonomy#Tropical_Storm
:Tropical_Storm rdf:type owl:Class ;
                rdfs:subClassOf :Tropical_cyclone ;
                rdfs:comment """A tropical cyclone with maximum sustained winds of 39 to 73 mph (34 to 63 knots).	

Resource: https://www.nhc.noaa.gov/climo/""" .


###  http://www.semanticweb.org/ontologies/2022/6/geological_taxonomy#Tropical_cyclone
:Tropical_cyclone rdf:type owl:Class ;
                  rdfs:subClassOf :Cyclone ;
                  rdfs:comment """Tropical cyclones originate only over the seas.

Resource: https://www.insightsonindia.com/world-geography/physical-geography-of-the-world/climatology/cyclones-and-anticyclones/difference-between-extratropical-and-tropical-cyclones/#:~:text=Extratropical%20cyclones%20cover%20a%20larger,compared%20to%20the%20tropical%20cyclone.

Justification: depending upon speed and region
https://www.nhc.noaa.gov/climo/""" .


###  http://www.semanticweb.org/ontologies/2022/6/geological_taxonomy#Tsunami
:Tsunami rdf:type owl:Class ;
         rdfs:subClassOf :Natural_disasters ;
         rdfs:comment """series of waves in a water body caused by the displacement of a large volume of water, generally in an ocean or a large lake.	

Resource: https://en.wikipedia.org/wiki/Tsunami

Justification: catagorized by the magnitude of the largest wave of the set
http://www.sfu.ca/geog355fall01/cobryne/types_of_tsunamis.html""" .


###  http://www.semanticweb.org/ontologies/2022/6/geological_taxonomy#Tufa
:Tufa rdf:type owl:Class ;
      rdfs:subClassOf :Sedimentary_rocks ;
      rdfs:comment """Tufa is a highly porous, sedimentary rock (limestone) composed of calcium carbonate, CaCO3. It is formed by biological and chemical precipitation of Calcite or aragonite from cold, supersaturated surface or ground waters.

Resource: http://chc.sbg.ac.at/sri/thesaurus/node.php?id=58""" .


###  http://www.semanticweb.org/ontologies/2022/6/geological_taxonomy#Tuff
:Tuff rdf:type owl:Class ;
      rdfs:subClassOf :Igneous_rocks ;
      rdfs:comment """Tuff is an igneous rock that forms from the products of an explosive volcanic eruption. In these eruptions, the volcano blasts rock, ash, magma and other materials from its vent.

Resource: https://geology.com/rocks/tuff.shtml""" .


###  http://www.semanticweb.org/ontologies/2022/6/geological_taxonomy#Turbels
:Turbels rdf:type owl:Class ;
         rdfs:subClassOf :Gelisols ;
         rdfs:comment """Gelisols that have one or more horizons showing cryoturbation in the form of irregular, broken, or distorted horizon boundaries, involutions, the accumulation of organic matter on top of the permafrost, ice or sand wedges, and oriented rock fragments.

Resource: https://sites.google.com/site/dinpuithai/Home/key10/key10a
https://acsess.onlinelibrary.wiley.com/doi/full/10.2136/sh2013-54-4-gc""" .


###  http://www.semanticweb.org/ontologies/2022/6/geological_taxonomy#Turbidite
:Turbidite rdf:type owl:Class ;
           rdfs:subClassOf :Sedimentary_rocks ;
           rdfs:comment """A particular sequence of sedimentary rocks which form within the deep ocean environment

Resource: https://geology.fandom.com/wiki/List_of_rock_types""" .


###  http://www.semanticweb.org/ontologies/2022/6/geological_taxonomy#Udalfs
:Udalfs rdf:type owl:Class ;
        rdfs:subClassOf :Alfisols ;
        rdfs:comment """Alfisols which are located in humid or subhumid climates.

Resource: https://en.wikipedia.org/wiki/Alfisol#Suborders""" .


###  http://www.semanticweb.org/ontologies/2022/6/geological_taxonomy#Udands
:Udands rdf:type owl:Class ;
        rdfs:subClassOf :Andisols ;
        rdfs:comment """Andisols of humid climates.

Resource: https://en.wikipedia.org/wiki/Andisol""" .


###  http://www.semanticweb.org/ontologies/2022/6/geological_taxonomy#Udepts
:Udepts rdf:type owl:Class ;
        rdfs:subClassOf :Inceptisols ;
        rdfs:comment """Inceptisols that have a udic soil moisture regime.

Resource: https://sites.google.com/site/dinpuithai/Home/taxonomy/k-inceptisols/kg""" .


###  http://www.semanticweb.org/ontologies/2022/6/geological_taxonomy#Uderts
:Uderts rdf:type owl:Class ;
        rdfs:subClassOf :Vertisols ;
        rdfs:comment """Vertisols with seasonal cracking pattern indicative of a udic
moisture regime (seasonally well-distributed rainfall)

Resource: \"Illustrated Guide to Soil Taxonomy\" book by Unites States Department of Agriculture""" .


###  http://www.semanticweb.org/ontologies/2022/6/geological_taxonomy#Udolls
:Udolls rdf:type owl:Class ;
        rdfs:subClassOf :Mollisols ;
        rdfs:comment """Udolls have an udic Soil Moisture Regime

Resource: https://www.sciencedirect.com/topics/agricultural-and-biological-sciences/mollisol""" .


###  http://www.semanticweb.org/ontologies/2022/6/geological_taxonomy#Udox
:Udox rdf:type owl:Class ;
      rdfs:subClassOf :Oxisols ;
      rdfs:comment """Udox are well drained Oxisols with a udic soil moisture regime.

Resource: https://www.nrcs.usda.gov/wps/portal/nrcs/detail/soils/survey/class/maps/?cid=nrcs142p2_053606""" .


###  http://www.semanticweb.org/ontologies/2022/6/geological_taxonomy#Udults
:Udults rdf:type owl:Class ;
        rdfs:subClassOf :Ultisols ;
        rdfs:comment """Ultisols that have a udic moisture regime.

Resource: https://sites.google.com/site/dinpuithai/Home/key10/key10h""" .


###  http://www.semanticweb.org/ontologies/2022/6/geological_taxonomy#Ultisols
:Ultisols rdf:type owl:Class ;
          rdfs:subClassOf :Soil ;
          rdfs:comment """The central concept of Ultisols is that of soils that have a horizon that contains an appreciable amount of translocated silicate clay (an argillic or kandic horizon) and few bases (base saturation less than 35 percent).

Resource: https://www.nrcs.usda.gov/wps/portal/nrcs/detail/soils/survey/class/maps/?cid=nrcs142p2_053609

Justification: Depending upon soil moisture regime and different horizons""" .


###  http://www.semanticweb.org/ontologies/2022/6/geological_taxonomy#Umber
:Umber rdf:type owl:Class ;
       rdfs:subClassOf :Sedimentary_rocks ;
       rdfs:comment """Umber is a marine sediment associated with black smokers.

Resource: https://www.sandatlas.org/rock-types/""" .


###  http://www.semanticweb.org/ontologies/2022/6/geological_taxonomy#Units_of_Earth_structure
:Units_of_Earth_structure rdf:type owl:Class ;
                          rdfs:subClassOf :Geological_entities ;
                          rdfs:comment """inner structure of the planet Earth, consisting of several concentric spherical layers

Resource: https://en.wikipedia.org/wiki/Structure_of_Earth

Justification: Layers are classified based on chemical composition""" .


###  http://www.semanticweb.org/ontologies/2022/6/geological_taxonomy#Upper_mantle
:Upper_mantle rdf:type owl:Class ;
              rdfs:subClassOf :Mantle ;
              rdfs:comment """The upper mantle of Earth is a very thick layer of rock inside the planet, which begins just beneath the crust and ends at the top of the lower mantle

Resource: https://en.wikipedia.org/wiki/Upper_mantle_(Earth)

Justification: Classified based on different mechanical properties""" .


###  http://www.semanticweb.org/ontologies/2022/6/geological_taxonomy#Ustalfs
:Ustalfs rdf:type owl:Class ;
         rdfs:subClassOf :Alfisols ;
         rdfs:comment """Alfisols that have an ustic moisture regime.

Resource: https://sites.google.com/site/dinpuithai/Home/taxonomy/j-alfisols""" .


###  http://www.semanticweb.org/ontologies/2022/6/geological_taxonomy#Ustands
:Ustands rdf:type owl:Class ;
         rdfs:subClassOf :Andisols ;
         rdfs:comment """Andisols that have an ustic moisture regime.

Resource: https://sites.google.com/site/dinpuithai/Home/key10/key10d""" .


###  http://www.semanticweb.org/ontologies/2022/6/geological_taxonomy#Ustepts
:Ustepts rdf:type owl:Class ;
         rdfs:subClassOf :Inceptisols ;
         rdfs:comment """Inceptisols that have an ustic soil moisture regime

Resource: https://sites.google.com/site/dinpuithai/Home/key10/key10k""" .


###  http://www.semanticweb.org/ontologies/2022/6/geological_taxonomy#Usterts
:Usterts rdf:type owl:Class ;
         rdfs:subClassOf :Vertisols ;
         rdfs:comment """Vertisols that, if not irrigated during the year, have cracks in normal years that are 5 mm or more wide, through a thickness of 25 cm or more within 50 cm of the mineral soil surface, for 90 or more cumulative days per year.

Resource: https://sites.google.com/site/dinpuithai/Home/key10/key10f""" .


###  http://www.semanticweb.org/ontologies/2022/6/geological_taxonomy#Ustolls
:Ustolls rdf:type owl:Class ;
         rdfs:subClassOf :Mollisols ;
         rdfs:comment """Ustolls have an ustic or an aridic Soil Moisture Regime

Resource: https://www.sciencedirect.com/topics/agricultural-and-biological-sciences/mollisol""" .


###  http://www.semanticweb.org/ontologies/2022/6/geological_taxonomy#Ustox
:Ustox rdf:type owl:Class ;
       rdfs:subClassOf :Oxisols ;
       rdfs:comment """Oxisols that have an ustic or xeric moisture regime

Resource: https://sites.google.com/site/dinpuithai/Home/key10/key10e""" .


###  http://www.semanticweb.org/ontologies/2022/6/geological_taxonomy#Ustults
:Ustults rdf:type owl:Class ;
         rdfs:subClassOf :Ultisols ;
         rdfs:comment """Ultisols that have an ustic moisture regime

Resource: https://sites.google.com/site/dinpuithai/Home/key10/key10h""" .


###  http://www.semanticweb.org/ontologies/2022/6/geological_taxonomy#Vertisols
:Vertisols rdf:type owl:Class ;
           rdfs:subClassOf :Soil ;
           rdfs:comment """The central concept of Vertisols is that of soils that have a high content of expanding clay and that have at some time of the year deep wide cracks.

Resource: https://www.nrcs.usda.gov/wps/portal/nrcs/detail/soils/survey/class/maps/?cid=nrcs142p2_053611

Justification: Based on moisture regime and one is based on temperature regime""" .


###  http://www.semanticweb.org/ontologies/2022/6/geological_taxonomy#Vitrands
:Vitrands rdf:type owl:Class ;
          rdfs:subClassOf :Andisols ;
          rdfs:comment """Andisols that have a 1500 kPa water retention of less than 15 percent on air-dried samples and less than 30 percent on undried samples throughout 60 percent or more of the thickness.
Relatively young Andisols that are coarse-textured and dominated by glass.

Resource: https://sites.google.com/site/dinpuithai/Home/key10/key10d
https://en.wikipedia.org/wiki/Andisol""" .


###  http://www.semanticweb.org/ontologies/2022/6/geological_taxonomy#Volcanic_earthquakes
:Volcanic_earthquakes rdf:type owl:Class ;
                      rdfs:subClassOf :Earthquakes ;
                      rdfs:comment """Earthquakes induced by rising lava or magma beneath active volcanoes is called volcanic earthquakes.

Resource: https://www.phivolcs.dost.gov.ph/index.php/earthquake/introduction-to-earthquake""" .


###  http://www.semanticweb.org/ontologies/2022/6/geological_taxonomy#Wackestone
:Wackestone rdf:type owl:Class ;
            rdfs:subClassOf :Sedimentary_rocks ;
            rdfs:comment """A matrix-supported carbonate sedimentary rock.

Resource: https://geology.fandom.com/wiki/List_of_rock_types""" .


###  http://www.semanticweb.org/ontologies/2022/6/geological_taxonomy#Weather_conditions
:Weather_conditions rdf:type owl:Class ;
                    rdfs:subClassOf :Geological_phenomena ;
                    rdfs:comment """The atmospheric conditions that comprise the state of the atmosphere in terms of temperature and wind and clouds and precipitation

Resource: https://www.vocabulary.com/dictionary/weather%20condition

Justification: Classified based on the different conditions of the earth’s atmosphere.""" .


###  http://www.semanticweb.org/ontologies/2022/6/geological_taxonomy#Websterite
:Websterite rdf:type owl:Class ;
            rdfs:subClassOf :Igneous_rocks ;
            rdfs:comment """Websterite is ultramafic igneous rock that consists of roughly equal proportions of orthopyroxene and clinopyroxene. 

Resource: https://en.wikipedia.org/wiki/Websterite""" .


###  http://www.semanticweb.org/ontologies/2022/6/geological_taxonomy#Wehrlite
:Wehrlite rdf:type owl:Class ;
          rdfs:subClassOf :Igneous_rocks ;
          rdfs:comment """Wehrlite is an ultramafic and ultrabasic rock that is a mixture of olivine and clinopyroxene.

Resource: https://en.wikipedia.org/wiki/Wehrlite""" .


###  http://www.semanticweb.org/ontologies/2022/6/geological_taxonomy#Whiteschist
:Whiteschist rdf:type owl:Class ;
             rdfs:subClassOf :Metamorphic_rocks ;
             rdfs:comment """A whiteschist is an uncommon metamorphic rock formed at high to ultra-high pressures.

Resource: https://en.wikipedia.org/wiki/Whiteschist""" .


###  http://www.semanticweb.org/ontologies/2022/6/geological_taxonomy#Wildfire
:Wildfire rdf:type owl:Class ;
          rdfs:subClassOf :Natural_disasters ;
          rdfs:comment """A wildfire, forest fire, bushfire, wildland fire or rural fire is an unplanned, uncontrolled and unpredictable fire in an area of combustible vegetation starting in rural and urban areas.	

Resource: https://en.wikipedia.org/wiki/Wildfire

Justification: Classification based on the type of vegetation that fuels them and intensity of the wildfire""" .


###  http://www.semanticweb.org/ontologies/2022/6/geological_taxonomy#Windy
:Windy rdf:type owl:Class ;
       rdfs:subClassOf :Weather_conditions ;
       rdfs:comment """Wind can be defined as air under motion. Air moves whenever there’s an imbalance between the pressure in any two locations.

Resource: https://outforia.com/types-of-weather/""" .


###  http://www.semanticweb.org/ontologies/2022/6/geological_taxonomy#Xeralfs
:Xeralfs rdf:type owl:Class ;
         rdfs:subClassOf :Alfisols ;
         rdfs:comment """Alfisols that have a xeric moisture regime

Resource: https://sites.google.com/site/dinpuithai/Home/taxonomy/j-alfisols""" .


###  http://www.semanticweb.org/ontologies/2022/6/geological_taxonomy#Xerands
:Xerands rdf:type owl:Class ;
         rdfs:subClassOf :Andisols ;
         rdfs:comment """Andisols that have a xeric moisture regime.

Resource: https://sites.google.com/site/dinpuithai/Home/key10/key10d""" .


###  http://www.semanticweb.org/ontologies/2022/6/geological_taxonomy#Xerepts
:Xerepts rdf:type owl:Class ;
         rdfs:subClassOf :Inceptisols ;
         rdfs:comment """Inceptisols that have a xeric soil moisture regime.

Resource: https://sites.google.com/site/dinpuithai/Home/key10/key10k""" .


###  http://www.semanticweb.org/ontologies/2022/6/geological_taxonomy#Xererts
:Xererts rdf:type owl:Class ;
         rdfs:subClassOf :Vertisols ;
         rdfs:comment """They have a thermic, mesic, or frigid soil temperature regime. They show cracks that are open at least 60 consecutive days during the summer, but are closed at least 60 consecutive days during winter.

Resource: https://en.wikipedia.org/wiki/Vertisol""" .


###  http://www.semanticweb.org/ontologies/2022/6/geological_taxonomy#Xerolls
:Xerolls rdf:type owl:Class ;
         rdfs:subClassOf :Mollisols ;
         rdfs:comment """Xerolls have a xeric Soil Moisture Regime

Resource: https://www.sciencedirect.com/topics/agricultural-and-biological-sciences/mollisol""" .


###  http://www.semanticweb.org/ontologies/2022/6/geological_taxonomy#Xerults
:Xerults rdf:type owl:Class ;
         rdfs:subClassOf :Ultisols ;
         rdfs:comment """A suborder of the soil order Ultisol, formed in a xeric moisture regime; brownish or reddish soil with a low to moderate organic-carbon content.

Resource: https://encyclopedia2.thefreedictionary.com/Xerult""" .


###  http://www.semanticweb.org/ontologies/2022/6/geological_taxonomy#protolith
:protolith rdf:type owl:Class ;
           rdfs:subClassOf :Metamorphic_rocks ;
           rdfs:comment """A protolith is the original, unmetamorphosed rock from which a given metamorphic rock is formed.

Resource: https://en.wikipedia.org/wiki/List_of_rock_types""" .


###  http://www.semanticweb.org/ontologies/2022/6/geological_taxonomy#ʻAʻā
:ʻAʻā rdf:type owl:Class ;
      rdfs:subClassOf :Basalt ;
      rdfs:comment """Basaltic lava with a crumpled appearance

Resource: https://en.wikipedia.org/wiki/%CA%BBA%CA%BB%C4%81""" .


###  http://www.semanticweb.org/ontologies/2022/6/geological_taxonomy#D_Double-Prime_(D’’)
<http://www.semanticweb.org/ontologies/2022/6/geological_taxonomy#D_Double-Prime_(D’’)> rdf:type owl:Class ;
                                                                                        rdfs:subClassOf :Mantle ;
                                                                                        rdfs:comment """D\" is the layer which separates the mantle from the core, a region with anomalous seismic properties.

Resource: https://www.newworldencyclopedia.org/entry/Mantle_(geology)""" .


###  http://www.semanticweb.org/ontologies/2022/6/geological_taxonomy#Dolomite_(rock)
<http://www.semanticweb.org/ontologies/2022/6/geological_taxonomy#Dolomite_(rock)> rdf:type owl:Class ;
                                                                                   rdfs:subClassOf :Sedimentary_rocks ;
                                                                                   rdfs:comment """Dolomite (also known as dolomite rock, dolostone or dolomitic rock) is a sedimentary carbonate rock that contains a high percentage of the mineral dolomite, CaMg(CO3)2. 

Resource: https://en.wikipedia.org/wiki/Dolomite_(rock)""" .


###  http://www.semanticweb.org/ontologies/2022/6/geological_taxonomy#Earth's_inner_core
<http://www.semanticweb.org/ontologies/2022/6/geological_taxonomy#Earth's_inner_core> rdf:type owl:Class ;
                                                                                      rdfs:subClassOf :Planetary_core ;
                                                                                      rdfs:comment """Earth's inner core is the innermost geologic layer of planet Earth. It is primarily a solid ball with a radius of about 1,220 km (760 mi). Pressure ranges from about 330 to 360 gigapascals (3,300,000 to 3,600,000 atm)

Resource: https://en.wikipedia.org/wiki/Earth%27s_inner_core""" .


###  http://www.semanticweb.org/ontologies/2022/6/geological_taxonomy#Lithosphere–asthenosphere_boundary
<http://www.semanticweb.org/ontologies/2022/6/geological_taxonomy#Lithosphere–asthenosphere_boundary> rdf:type owl:Class ;
                                                                                                      rdfs:subClassOf :Upper_mantle ;
                                                                                                      rdfs:comment """represents a mechanical difference between layers in Earth's inner structure.

Resource: https://en.wikipedia.org/wiki/Lithosphere%E2%80%93asthenosphere_boundary""" .


###  http://www.semanticweb.org/ontologies/2022/6/geological_taxonomy#Nor'easter
<http://www.semanticweb.org/ontologies/2022/6/geological_taxonomy#Nor'easter> rdf:type owl:Class ;
                                                                              rdfs:subClassOf :Extratropical_cyclone ;
                                                                              rdfs:comment """A synoptic-scale extratropical cyclone in the western North Atlantic Ocean with combination of northeast winds and moisture content of the swirling clouds.

Resource: https://en.wikipedia.org/wiki/Nor%27easter""" .


###  http://www.semanticweb.org/ontologies/2022/6/geological_taxonomy#Riverine_(Channel)_Floods
<http://www.semanticweb.org/ontologies/2022/6/geological_taxonomy#Riverine_(Channel)_Floods> rdf:type owl:Class ;
                                                                                             rdfs:subClassOf :Floods ;
                                                                                             rdfs:comment """Riverine Flooding is when streams and rivers exceed the capacity of their natural or constructed channels to accommodate water flow and water overflows the banks, spilling out into adjacent low-lying, dry land	

Resource: https://hazards.fema.gov/nri/riverine-flooding""" .


###  http://www.semanticweb.org/ontologies/2022/6/geological_taxonomy#Transition_zone_(Earth)
<http://www.semanticweb.org/ontologies/2022/6/geological_taxonomy#Transition_zone_(Earth)> rdf:type owl:Class ;
                                                                                           rdfs:subClassOf :Mantle ;
                                                                                           rdfs:comment """The transition zone is part of the Earth's mantle, and is located between the lower mantle and the upper mantle

Resource: https://en.wikipedia.org/wiki/Transition_zone_(Earth)""" .


###  https://en.wikipedia.org/wiki/Atmosphere#Overcast
<https://en.wikipedia.org/wiki/Atmosphere#Overcast> rdf:type owl:Class ;
                                                    rdfs:subClassOf :Cloudy ;
                                                    owl:disjointWith <https://en.wikipedia.org/wiki/Atmosphere#Partially_cloudy> ;
                                                    rdfs:comment """Overcast weather is when the sky is completely covered by a cloud blanket.

Resource: https://weather.fandom.com/wiki/Types_of_Weather#Overcast""" .


###  https://en.wikipedia.org/wiki/Atmosphere#Partially_cloudy
<https://en.wikipedia.org/wiki/Atmosphere#Partially_cloudy> rdf:type owl:Class ;
                                                            rdfs:subClassOf :Cloudy ;
                                                            rdfs:comment """Partially cloudy weather is when some clouds are hovering above the horizon level; however, most of the sky remains clear and there is no precipitation of any kind.

Resource: https://weather.fandom.com/wiki/Types_of_Weather#Partially_cloudy""" .


#################################################################
#    Individuals
#################################################################

###  http://www.semanticweb.org/ontologies/2022/6/geological_taxonomy#Actinolite
:Actinolite rdf:type owl:NamedIndividual ,
                     :Silicates ;
            rdfs:comment """Actinolite is an amphibole silicate mineral with the chemical formula Ca2(Mg4.5-2.5Fe2+0.5-2.5)Si8O22(OH)2.

Resource: https://en.wikipedia.org/wiki/Actinolite""" .


###  http://www.semanticweb.org/ontologies/2022/6/geological_taxonomy#Afghanite
:Afghanite rdf:type owl:NamedIndividual ,
                    :Silicates ;
           rdfs:comment """Afghanite, (Na,K)22Ca10[Si24Al24O96](SO4)6Cl6,[2] is a hydrous sodium, calcium, potassium, sulfate, chloride, carbonate alumino-silicate mineral. Afghanite is a feldspathoid of the cancrinite group and typically occurs with sodalite group minerals.

Resource: https://en.wikipedia.org/wiki/Afghanite""" .


###  http://www.semanticweb.org/ontologies/2022/6/geological_taxonomy#Alarsite
:Alarsite rdf:type owl:NamedIndividual ,
                   :Phosphates_Arsenates_Vanadates ;
          rdfs:comment """Alarsite (AlAsO4) is an aluminium arsenate mineral with its name derived from its composition: aluminium and arsenate.
Chemical Formula: AlAsO4

Resource: http://webmineral.com/data/Alarsite.shtml#.Yy8RcnZBzIU
https://en.wikipedia.org/wiki/Alarsite""" .


###  http://www.semanticweb.org/ontologies/2022/6/geological_taxonomy#Albite
:Albite rdf:type owl:NamedIndividual ,
                 :Silicates ;
        rdfs:comment """Albite is a plagioclase feldspar mineral. The pure albite endmember has the formula NaAlSi3O8.

Resource: https://en.wikipedia.org/wiki/Albite""" .


###  http://www.semanticweb.org/ontologies/2022/6/geological_taxonomy#Alfredstelznerite
:Alfredstelznerite rdf:type owl:NamedIndividual ,
                            :Borates ;
                   rdfs:comment """Chemical Formula: Ca4(H2O)4 [B4O4(OH)6]4 {H2O}15

Resource: http://www.webmineral.com/data/Alfredstelznerite.shtml#.Yy8RnnZBzIU""" .


###  http://www.semanticweb.org/ontologies/2022/6/geological_taxonomy#Algodonite
:Algodonite rdf:type owl:NamedIndividual ,
                     :Sulfides_and_Sulfosalts ;
            rdfs:comment """Algodonite is a copper arsenide mineral. It is a gray white metallic mineral crystallizing in the hexagonal system.
Chemical formula: Cu6As

Resource: https://en.wikipedia.org/wiki/Algodonite""" .


###  http://www.semanticweb.org/ontologies/2022/6/geological_taxonomy#Almandine
:Almandine rdf:type owl:NamedIndividual ,
                    :Silicates ;
           rdfs:comment """Almandine, also known as almandite, is a species of mineral belonging to the garnet group. The almandine crystal formula is: Fe3Al2(SiO4)3.

Resource: https://en.wikipedia.org/wiki/Almandine""" .


###  http://www.semanticweb.org/ontologies/2022/6/geological_taxonomy#Amalgam
:Amalgam rdf:type owl:NamedIndividual ,
                  :Elements ;
         rdfs:comment """An amalgam is an alloy of mercury with another metal. It may be a liquid, a soft paste or a solid, depending upon the proportion of mercury.
Chemical Formula: Ag2Hg3

Resource: https://en.wikipedia.org/wiki/Amalgam_(chemistry)
http://webmineral.com/data/Amalgam.shtml#.Yy8SM3ZBzIU""" .


###  http://www.semanticweb.org/ontologies/2022/6/geological_taxonomy#Amblygonite
:Amblygonite rdf:type owl:NamedIndividual ,
                      :Phosphates_Arsenates_Vanadates ;
             rdfs:comment """Amblygonite, is a fluorophosphate mineral, (Li,Na)AlPO4(F,OH), composed of lithium, sodium, aluminium, phosphate, fluoride and hydroxide.

Resource: https://en.wikipedia.org/wiki/Amblygonite""" .


###  http://www.semanticweb.org/ontologies/2022/6/geological_taxonomy#Andalusite
:Andalusite rdf:type owl:NamedIndividual ,
                     :Silicates ;
            rdfs:comment """Andalusite is an aluminium nesosilicate mineral with the chemical formula Al2SiO5.

Resource: https://en.wikipedia.org/wiki/Andalusite""" .


###  http://www.semanticweb.org/ontologies/2022/6/geological_taxonomy#Andradite
:Andradite rdf:type owl:NamedIndividual ,
                    :Silicates ;
           rdfs:comment """Andradite is a mineral species of the garnet group. It is a nesosilicate, with formula Ca3Fe2Si3O12.

Resource: https://en.wikipedia.org/wiki/Andradite""" .


###  http://www.semanticweb.org/ontologies/2022/6/geological_taxonomy#Anhydrite
:Anhydrite rdf:type owl:NamedIndividual ,
                    :Sulfates ;
           rdfs:comment """Anhydrite, or anhydrous calcium sulfate, is a mineral with the chemical formula CaSO4.

Resource: https://en.wikipedia.org/wiki/Anhydrite""" .


###  http://www.semanticweb.org/ontologies/2022/6/geological_taxonomy#Anorthite
:Anorthite rdf:type owl:NamedIndividual ,
                    :Silicates ;
           rdfs:comment """Anorthite is the calcium endmember of the plagioclase feldspar mineral series. The chemical formula of pure anorthite is CaAl2Si2O8.

Resource: https://en.wikipedia.org/wiki/Anorthite""" .


###  http://www.semanticweb.org/ontologies/2022/6/geological_taxonomy#Antigorite
:Antigorite rdf:type owl:NamedIndividual ,
                     :Silicates ;
            rdfs:comment """Antigorite is a lamellated, monoclinic mineral in the phylosilicate serpentine subgroup with the ideal chemical formula of (Mg,Fe2+)3Si2O5(OH)4

Resource: https://en.wikipedia.org/wiki/Antigorite""" .


###  http://www.semanticweb.org/ontologies/2022/6/geological_taxonomy#Aragonite
:Aragonite rdf:type owl:NamedIndividual ,
                    :Carbonates ;
           rdfs:comment """Aragonite is a carbonate mineral, one of the three most common naturally occurring crystal forms of calcium carbonate, CaCO3

Resource: https://en.wikipedia.org/wiki/Aragonite""" .


###  http://www.semanticweb.org/ontologies/2022/6/geological_taxonomy#Arcanite
:Arcanite rdf:type owl:NamedIndividual ,
                   :Sulfates ;
          rdfs:comment "" ,
                       """Arcanite is a potassium sulfate mineral with formula: K2SO4.

Resource: https://en.wikipedia.org/wiki/Arcanite""" .


###  http://www.semanticweb.org/ontologies/2022/6/geological_taxonomy#Atheneite
:Atheneite rdf:type owl:NamedIndividual ,
                    :Sulfides_and_Sulfosalts ;
           rdfs:comment """Atheneite is a rare palladium, mercury arsenide mineral with the chemical formula (Pd,Hg)3 associated with palladium–gold deposits.

Resource: https://en.wikipedia.org/wiki/Atheneite""" .


###  http://www.semanticweb.org/ontologies/2022/6/geological_taxonomy#Benitoite
:Benitoite rdf:type owl:NamedIndividual ,
                    :Silicates ;
           rdfs:comment """Benitoite is a rare blue barium titanium cyclosilicate.
Chemical Formula: BaTi(Si3O9)

Resource: https://en.wikipedia.org/wiki/Benitoite
https://www.mindat.org/min-624.html""" .


###  http://www.semanticweb.org/ontologies/2022/6/geological_taxonomy#Berborite
:Berborite rdf:type owl:NamedIndividual ,
                    :Borates ;
           rdfs:comment """Berborite is a beryllium borate mineral with the chemical formula Be2(BO3)(OH,F)·(H2O). It is colorless and leaves a white streak. Its crystals are hexagonal to pyramidal. It is transparent and has vitreous luster.

Resource: https://en.wikipedia.org/wiki/Berborite""" .


###  http://www.semanticweb.org/ontologies/2022/6/geological_taxonomy#Berlinite
:Berlinite rdf:type owl:NamedIndividual ,
                    :Phosphates_Arsenates_Vanadates ;
           rdfs:comment """Berlinite (aluminium phosphate, chemical formula AlPO4 or Al(PO4))) is a rare high-temperature hydrothermal or metasomatic phosphate mineral.

Resource: https://en.wikipedia.org/wiki/Berlinite""" .


###  http://www.semanticweb.org/ontologies/2022/6/geological_taxonomy#Beryl
:Beryl rdf:type owl:NamedIndividual ,
                :Silicates ;
       rdfs:comment """Beryl is a mineral composed of beryllium aluminium silicate with the chemical formula Be3Al2Si6O18.

Resource: https://en.wikipedia.org/wiki/Beryl""" .


###  http://www.semanticweb.org/ontologies/2022/6/geological_taxonomy#Brazilianite
:Brazilianite rdf:type owl:NamedIndividual ,
                       :Phosphates_Arsenates_Vanadates ;
              rdfs:comment """Brazilianite, whose name derives from its country of origin, Brazil, is a typically yellow-green phosphate mineral, most commonly found in phosphate-rich pegmatites.
Chemical Formula: NaAl3(PO4)2(OH)4

Resource: https://en.wikipedia.org/wiki/Brazilianite
https://www.mindat.org/min-760.html""" .


###  http://www.semanticweb.org/ontologies/2022/6/geological_taxonomy#Brownmillerite
:Brownmillerite rdf:type owl:NamedIndividual ,
                         :Oxides ;
                rdfs:comment """Brownmillerite is a rare oxide mineral with chemical formula Ca2(Al,Fe)2O5.

Resource: https://en.wikipedia.org/wiki/Brownmillerite""" .


###  http://www.semanticweb.org/ontologies/2022/6/geological_taxonomy#Cadmium
:Cadmium rdf:type owl:NamedIndividual ,
                  :Elements ;
         rdfs:comment """Cadmium is a chemical element with the symbol Cd and atomic number 48. This soft, silvery-white metal is chemically similar to the two other stable metals in group 12, zinc and mercury.

Resource: https://en.wikipedia.org/wiki/Cadmium""" .


###  http://www.semanticweb.org/ontologies/2022/6/geological_taxonomy#Calcite
:Calcite rdf:type owl:NamedIndividual ,
                  :Carbonates ;
         rdfs:comment """Calcite, the most common form of natural calcium carbonate (CaCO3), a widely distributed mineral known for the beautiful development and great variety of its crystals.

Resource: https://www.britannica.com/science/calcite""" .


###  http://www.semanticweb.org/ontologies/2022/6/geological_taxonomy#Caminite
:Caminite rdf:type owl:NamedIndividual ,
                   :Sulfates ;
          rdfs:comment """A tetragonal-ditetragonal dipyramidal mineral containing hydrogen, magnesium, oxygen, and sulfur.
Chemical Formula: Mg7(SO4)5(OH)4•(H2O)

Resource: https://en.wiktionary.org/wiki/caminite
http://webmineral.com/data/Caminite.shtml#.Yy8YXHZBzIU""" .


###  http://www.semanticweb.org/ontologies/2022/6/geological_taxonomy#Carnallite
:Carnallite rdf:type owl:NamedIndividual ,
                     :Halides ;
            rdfs:comment """Carnallite, a soft, white halide mineral, hydrated potassium and magnesium chloride (KMgCl3·6H2O), that is a source of potassium for fertilizers. 

Resource: https://www.britannica.com/science/carnallite""" .


###  http://www.semanticweb.org/ontologies/2022/6/geological_taxonomy#Cerussite
:Cerussite rdf:type owl:NamedIndividual ,
                    :Carbonates ;
           rdfs:comment """Cerussite (also known as lead carbonate or white lead ore) is a mineral consisting of lead carbonate (PbCO3), and is an important ore of lead.

Resource: https://en.wikipedia.org/wiki/Cerussite""" .


###  http://www.semanticweb.org/ontologies/2022/6/geological_taxonomy#Chalcocite
:Chalcocite rdf:type owl:NamedIndividual ,
                     :Sulfides_and_Sulfosalts ;
            rdfs:comment """Chalcocite, copper(I) sulfide (Cu2S), is an important copper ore mineral. It is opaque and dark gray to black, with a metallic luster.

Resource: https://en.wikipedia.org/wiki/Chalcocite""" .


###  http://www.semanticweb.org/ontologies/2022/6/geological_taxonomy#Charoite
:Charoite rdf:type owl:NamedIndividual ,
                   :Silicates ;
          rdfs:comment """Charoite K(Ca,Na)2Si4O10(OH,F)•H2O is a rare silicate mineral, first described in 1978

Resource: https://en.wikipedia.org/wiki/Charoite""" .


###  http://www.semanticweb.org/ontologies/2022/6/geological_taxonomy#Chondrodite
:Chondrodite rdf:type owl:NamedIndividual ,
                      :Silicates ;
             rdfs:comment """Chondrodite is a nesosilicate mineral with formula (Mg,Fe)5(SiO4)2(F,OH,O)2.

Resource: https://en.wikipedia.org/wiki/Chondrodite""" .


###  http://www.semanticweb.org/ontologies/2022/6/geological_taxonomy#Chromium-dravite
:Chromium-dravite rdf:type owl:NamedIndividual ,
                           :Silicates ;
                  rdfs:comment """Chemical Formula: NaMg3Cr3+6(Si6O18)(BO3)3(OH)3(OH)

Resource: https://www.mindat.org/min-1031.html""" .


###  http://www.semanticweb.org/ontologies/2022/6/geological_taxonomy#Chrysoberyl
:Chrysoberyl rdf:type owl:NamedIndividual ,
                      :Oxides ;
             rdfs:comment """The mineral or gemstone chrysoberyl is an aluminate of beryllium with the formula BeAl2O4.

Resource: https://en.wikipedia.org/wiki/Chrysoberyl""" .


###  http://www.semanticweb.org/ontologies/2022/6/geological_taxonomy#Clinohumite
:Clinohumite rdf:type owl:NamedIndividual ,
                      :Silicates ;
             rdfs:comment """Clinohumite is an uncommon member of the humite group, a magnesium silicate according to the chemical formula (Mg, Fe)9(SiO4)4(F,OH)2. 

Resource: https://en.wikipedia.org/wiki/Clinohumite""" .


###  http://www.semanticweb.org/ontologies/2022/6/geological_taxonomy#Clinozoisite
:Clinozoisite rdf:type owl:NamedIndividual ,
                       :Silicates ;
              rdfs:comment """Clinozoisite is a complex calcium aluminium sorosilicate mineral with formula: Ca2Al3(Si2O7)(SiO4)O(OH).

Resource: https://en.wikipedia.org/wiki/Clinozoisite""" .


###  http://www.semanticweb.org/ontologies/2022/6/geological_taxonomy#Coccinite
:Coccinite rdf:type owl:NamedIndividual ,
                    :Halides ;
           rdfs:comment """Coccinite is a rare mercury iodide mineral with chemical formula of HgI2, mercury(II) iodide.[5][6] It was first discovered in Casas Viejas, Mexico

Resource: https://en.wikipedia.org/wiki/Coccinite""" .


###  http://www.semanticweb.org/ontologies/2022/6/geological_taxonomy#Copper
:Copper rdf:type owl:NamedIndividual ,
                 :Elements ;
        rdfs:comment """Copper is a chemical element with the symbol Cu (from Latin: cuprum) and atomic number 29. It is a soft, malleable, and ductile metal with very high thermal and electrical conductivity.

Resource: https://en.wikipedia.org/wiki/Copper""" .


###  http://www.semanticweb.org/ontologies/2022/6/geological_taxonomy#Cordierite
:Cordierite rdf:type owl:NamedIndividual ,
                     :Silicates ;
            rdfs:comment """Cordierite (mineralogy) is a magnesium iron aluminium cyclosilicate.
Chemical Formula: (Mg,Fe)2Al4Si5O18

Resource: https://en.wikipedia.org/wiki/Cordierite""" .


###  http://www.semanticweb.org/ontologies/2022/6/geological_taxonomy#Corundum
:Corundum rdf:type owl:NamedIndividual ,
                   :Oxides ;
          rdfs:comment """Corundum is a crystalline form of aluminium oxide (Al2O3) typically containing traces of iron, titanium, vanadium and chromium.

Resource: https://en.wikipedia.org/wiki/Corundum""" .


###  http://www.semanticweb.org/ontologies/2022/6/geological_taxonomy#Crednerite
:Crednerite rdf:type owl:NamedIndividual ,
                     :Oxides ;
            rdfs:comment """A dark grey mineral that is a mixed oxide of copper and manganese.
Chemical Formula: CuMnO2

Resource: https://en.wiktionary.org/wiki/crednerite
http://webmineral.com/data/Crednerite.shtml#.Yy8Z4HZBzIU""" .


###  http://www.semanticweb.org/ontologies/2022/6/geological_taxonomy#Cuprite
:Cuprite rdf:type owl:NamedIndividual ,
                  :Oxides ;
         rdfs:comment """Cuprite is an oxide mineral composed of copper(I) oxide Cu2O, and is a minor ore of copper.

Resource: https://en.wikipedia.org/wiki/Cuprite""" .


###  http://www.semanticweb.org/ontologies/2022/6/geological_taxonomy#Danburite
:Danburite rdf:type owl:NamedIndividual ,
                    :Silicates ;
           rdfs:comment """Danburite is a calcium boron silicate mineral with a chemical formula of CaB2(SiO4)2.

Resource: https://en.wikipedia.org/wiki/Danburite""" .


###  http://www.semanticweb.org/ontologies/2022/6/geological_taxonomy#Dashkovaite
:Dashkovaite rdf:type owl:NamedIndividual ,
                      :Organic_compounds ;
             rdfs:comment """A monoclinic-prismatic white mineral containing carbon, hydrogen, magnesium, and oxygen.
Chemical Formula: Mg(HCOO)2•2(H2O)

Resource: https://en.wiktionary.org/wiki/dashkovaite
http://webmineral.com/data/Dashkovaite.shtml#.Yy8aZnZBzIU""" .


###  http://www.semanticweb.org/ontologies/2022/6/geological_taxonomy#Datolite
:Datolite rdf:type owl:NamedIndividual ,
                   :Silicates ;
          rdfs:comment """Datolite is a calcium boron hydroxide nesosilicate, CaBSiO4(OH).

Resource: https://en.wikipedia.org/wiki/Datolite""" .


###  http://www.semanticweb.org/ontologies/2022/6/geological_taxonomy#Diamond
:Diamond rdf:type owl:NamedIndividual ,
                  :Elements ;
         rdfs:comment """Diamond is a solid form of the element carbon with its atoms arranged in a crystal structure called diamond cubic.
Chemical Formula: C

Resource: https://en.wikipedia.org/wiki/Diamond
https://www.mindat.org/min-1282.html""" .


###  http://www.semanticweb.org/ontologies/2022/6/geological_taxonomy#Diaspore
:Diaspore rdf:type owl:NamedIndividual ,
                   :Oxides ;
          rdfs:comment """Diaspore, also known as diasporite, empholite, kayserite, or tanatarite, is an aluminium oxide hydroxide mineral, α-AlO(OH)

Resource: https://en.wikipedia.org/wiki/Diaspore""" .


###  http://www.semanticweb.org/ontologies/2022/6/geological_taxonomy#Diopside
:Diopside rdf:type owl:NamedIndividual ,
                   :Silicates ;
          rdfs:comment """Diopside is a monoclinic pyroxene mineral with composition MgCaSi2O6.

Resource: https://en.wikipedia.org/wiki/Diopside""" .


###  http://www.semanticweb.org/ontologies/2022/6/geological_taxonomy#Djurleite
:Djurleite rdf:type owl:NamedIndividual ,
                    :Sulfides_and_Sulfosalts ;
           rdfs:comment """Djurleite is a copper sulfide mineral of secondary origin with formula Cu31S16 that crystallizes with monoclinic-prismatic symmetry.

Resource: https://en.wikipedia.org/wiki/Djurleite""" .


###  http://www.semanticweb.org/ontologies/2022/6/geological_taxonomy#Dolomite
:Dolomite rdf:type owl:NamedIndividual ,
                   :Carbonates .


###  http://www.semanticweb.org/ontologies/2022/6/geological_taxonomy#Domeykite
:Domeykite rdf:type owl:NamedIndividual ,
                    :Sulfides_and_Sulfosalts ;
           rdfs:comment """Domeykite is a copper arsenide mineral, Cu3As. It crystallizes in the isometric system, although crystals are very rare. 

Resource: https://en.wikipedia.org/wiki/Domeykite""" .


###  http://www.semanticweb.org/ontologies/2022/6/geological_taxonomy#Dravite
:Dravite rdf:type owl:NamedIndividual ,
                  :Silicates ;
         rdfs:comment """Dravite is best known as the \"Brown Tourmaline\". It is a relatively common form of Tourmaline, and often forms in crude uninteresting formation.
Chemical Formula: NaMg3Al6(BO3)3Si6O18(OH)3F

Resource: https://www.minerals.net/mineral/dravite.aspx""" .


###  http://www.semanticweb.org/ontologies/2022/6/geological_taxonomy#Earlandite
:Earlandite rdf:type owl:NamedIndividual ,
                     :Organic_compounds ;
            rdfs:comment """Earlandite, [Ca3(C6H5O7)2(H2O)2]·2H2O, is the mineral form of calcium citrate tetrahydrate. It was first reported in 1936.

Resource: https://en.wikipedia.org/wiki/Earlandite""" .


###  http://www.semanticweb.org/ontologies/2022/6/geological_taxonomy#Eitelite
:Eitelite rdf:type owl:NamedIndividual ,
                   :Carbonates ;
          rdfs:comment """Chemical Formula: Na2Mg(CO3)2

Resource: http://webmineral.com/data/Eitelite.shtml#.Yy8bFHZBzIU""" .


###  http://www.semanticweb.org/ontologies/2022/6/geological_taxonomy#Elbaite
:Elbaite rdf:type owl:NamedIndividual ,
                  :Silicates ;
         rdfs:comment """Elbaite, a sodium, lithium, aluminium boro-silicate, with the chemical composition Na(Li1.5Al1.5)Al6Si6O18(BO3)3(OH)4,[4] is a mineral species belonging to the six-member ring cyclosilicate tourmaline group.

Resource: https://en.wikipedia.org/wiki/Elbaite""" .


###  http://www.semanticweb.org/ontologies/2022/6/geological_taxonomy#Enstatite
:Enstatite rdf:type owl:NamedIndividual ,
                    :Silicates ;
           rdfs:comment """Enstatite is a mineral; the magnesium endmember of the pyroxene silicate mineral series enstatite (MgSiO3) – ferrosilite (FeSiO3).

Resource: https://en.wikipedia.org/wiki/Enstatite""" .


###  http://www.semanticweb.org/ontologies/2022/6/geological_taxonomy#Epidote
:Epidote rdf:type owl:NamedIndividual ,
                  :Silicates ;
         rdfs:comment """Epidote is a calcium aluminium iron sorosilicate mineral.
Chemical Formula: {Ca2}{Al2Fe3+}(Si2O7)(SiO4)O(OH)

Resource: https://en.wikipedia.org/wiki/Epidote
https://www.mindat.org/min-1389.html""" .


###  http://www.semanticweb.org/ontologies/2022/6/geological_taxonomy#Euclase
:Euclase rdf:type owl:NamedIndividual ,
                  :Silicates ;
         rdfs:comment """Euclase is a beryllium aluminium hydroxide silicate mineral (BeAlSiO4(OH)). It crystallizes in the monoclinic crystal system and is typically massive to fibrous as well as in slender prismatic crystals.

Resource: https://en.wikipedia.org/wiki/Euclase""" .


###  http://www.semanticweb.org/ontologies/2022/6/geological_taxonomy#Eucryptite
:Eucryptite rdf:type owl:NamedIndividual ,
                     :Silicates ;
            rdfs:comment """Eucryptite is a lithium bearing aluminium silicate mineral with formula LiAlSiO4. It crystallizes in the trigonal - rhombohedral crystal system.

Resource: https://en.wikipedia.org/wiki/Eucryptite""" .


###  http://www.semanticweb.org/ontologies/2022/6/geological_taxonomy#Farringtonite
:Farringtonite rdf:type owl:NamedIndividual ,
                        :Phosphates_Arsenates_Vanadates ;
               rdfs:comment """Chemical Formula: Mg3(PO4)2

Resource: https://www.webmineral.com/data/Farringtonite.shtml""" .


###  http://www.semanticweb.org/ontologies/2022/6/geological_taxonomy#Ferrisicklerite
:Ferrisicklerite rdf:type owl:NamedIndividual ,
                          :Phosphates_Arsenates_Vanadates ;
                 rdfs:comment """An orthorhombic-dipyramidal mineral containing iron, lithium, manganese, oxygen, and phosphorus.
Chemical Formula: Li(Fe+++,Mn++)PO4

Resource: https://en.wiktionary.org/wiki/ferrisicklerite
http://www.webmineral.com/data/Ferrisicklerite.shtml#.Yy8btXZBzIU""" .


###  http://www.semanticweb.org/ontologies/2022/6/geological_taxonomy#Ferro-actinolite
:Ferro-actinolite rdf:type owl:NamedIndividual ,
                           :Silicates ;
                  rdfs:comment """Ferro-actinolite is the ferrous iron-rich endmember of the actinolite-tremolite continuous solid solution series of the double chain calcareous amphibole group of inosilicate minerals.
Chemical Formula: Ca2Fe2+5(Si8O22)OH2

Resource: https://en.wikipedia.org/wiki/Ferro-actinolite
https://www.mindat.org/min-1505.html""" .


###  http://www.semanticweb.org/ontologies/2022/6/geological_taxonomy#Fluorapatite
:Fluorapatite rdf:type owl:NamedIndividual ,
                       :Phosphates_Arsenates_Vanadates ;
              rdfs:comment """Fluorapatite, is a phosphate mineral with the formula Ca5(PO4)3F (calcium fluorophosphate). Fluorapatite is a hard crystalline solid.

Resource: https://en.wikipedia.org/wiki/Fluorapatite""" .


###  http://www.semanticweb.org/ontologies/2022/6/geological_taxonomy#Fluorite
:Fluorite rdf:type owl:NamedIndividual ,
                   :Halides ;
          rdfs:comment """Fluorite (also called fluorspar) is the mineral form of calcium fluoride, CaF2.

Resource: https://en.wikipedia.org/wiki/Fluorite""" .


###  http://www.semanticweb.org/ontologies/2022/6/geological_taxonomy#Formicaite
:Formicaite rdf:type owl:NamedIndividual ,
                     :Organic_compounds ;
            rdfs:comment """A tetragonal-trapezohedral mineral containing calcium, carbon, hydrogen, and oxygen.
Chemical Formula: Ca(HCOO)2

Resource: https://en.wiktionary.org/wiki/formicaite
http://www.webmineral.com/data/Formicaite.shtml#.Yy8b5HZBzIU""" .


###  http://www.semanticweb.org/ontologies/2022/6/geological_taxonomy#Forsterite
:Forsterite rdf:type owl:NamedIndividual ,
                     :Silicates ;
            rdfs:comment """Chemical Formula: Mg2SiO4

Resource: https://www.mindat.org/min-1584.html""" .


###  http://www.semanticweb.org/ontologies/2022/6/geological_taxonomy#Friedelite
:Friedelite rdf:type owl:NamedIndividual ,
                     :Silicates ;
            rdfs:comment """Friedelite is a mineral in the pyrosmalite group.
Chemical Formula: Mn2+8Si6O15(OH,Cl)10

Resource: https://en.wikipedia.org/wiki/Friedelite
https://www.mindat.org/min-1609.html""" .


###  http://www.semanticweb.org/ontologies/2022/6/geological_taxonomy#Gaspeite
:Gaspeite rdf:type owl:NamedIndividual ,
                   :Carbonates ;
          rdfs:comment """Gaspéite, a very rare nickel carbonate mineral, with the formula (Ni,Fe,Mg)CO3, is named for the place it was first described, in the Gaspé Peninsula, Québec, Canada.

Resource: https://en.wikipedia.org/wiki/Gasp%C3%A9ite""" .


###  http://www.semanticweb.org/ontologies/2022/6/geological_taxonomy#Grandidierite
:Grandidierite rdf:type owl:NamedIndividual ,
                        :Silicates ;
               rdfs:comment """Grandidierite is a rare mineral that was first discovered in 1902 in southern Madagascar.
Chemical Formula: (Mg,Fe2+)(Al,Fe3+)3(SiO4)(BO3)O2

Resource: https://en.wikipedia.org/wiki/Grandidierite
https://www.mindat.org/min-1737.html""" .


###  http://www.semanticweb.org/ontologies/2022/6/geological_taxonomy#Gregoryite
:Gregoryite rdf:type owl:NamedIndividual ,
                     :Carbonates ;
            rdfs:comment """Gregoryite is an anhydrous carbonate mineral that is rich in potassium and sodium[5] with the chemical formula (Na2,K2,Ca)CO3.[

Resource: https://en.wikipedia.org/wiki/Gregoryite""" .


###  http://www.semanticweb.org/ontologies/2022/6/geological_taxonomy#Grossular
:Grossular rdf:type owl:NamedIndividual ,
                    :Silicates ;
           rdfs:comment """Grossular is a calcium-aluminium species of the garnet group of minerals. It has the chemical formula of Ca3Al2(SiO4)3

Resource: https://en.wikipedia.org/wiki/Grossular""" .


###  http://www.semanticweb.org/ontologies/2022/6/geological_taxonomy#Hambergite
:Hambergite rdf:type owl:NamedIndividual ,
                     :Borates ;
            rdfs:comment """Hambergite (Be2BO3OH) is a beryllium borate mineral named after Swedish explorer and mineralogist Axel Hamberg (1863–1933). The mineral occurs as white or colorless orthorhombic crystals.

Resource: https://en.wikipedia.org/wiki/Hambergite""" .


###  http://www.semanticweb.org/ontologies/2022/6/geological_taxonomy#Hauckite
:Hauckite rdf:type owl:NamedIndividual ,
                   :Sulfates ;
          rdfs:comment """Chemical Formula: Fe3+3(Mg,Mn2+)24Zn18(SO4)4(CO3)2(OH)81

Resource: https://www.mindat.org/min-1830.html""" .


###  http://www.semanticweb.org/ontologies/2022/6/geological_taxonomy#Haüyne
:Haüyne rdf:type owl:NamedIndividual ,
                 :Silicates ;
        rdfs:comment """Hauyne or haüyne, also called hauynite or haüynite, is a tectosilicate sulfate mineral with endmember formula Na3Ca(Si3Al3)O12(SO4).

Resource: https://en.wikipedia.org/wiki/Hauyne""" .


###  http://www.semanticweb.org/ontologies/2022/6/geological_taxonomy#Hematite
:Hematite rdf:type owl:NamedIndividual ,
                   :Oxides ;
          rdfs:comment """Hematite, also spelled as haematite, is a common iron oxide compound with the formula, Fe2O3.

Resource: https://en.wikipedia.org/wiki/Hematite""" .


###  http://www.semanticweb.org/ontologies/2022/6/geological_taxonomy#Hemimorphite
:Hemimorphite rdf:type owl:NamedIndividual ,
                       :Silicates ;
              rdfs:comment """Hemimorphite is the chemical compound Zn4(Si2O7)(OH)2·H2O, a component of mineral calamine.

Resource: https://en.wikipedia.org/wiki/Hemimorphite""" .


###  http://www.semanticweb.org/ontologies/2022/6/geological_taxonomy#Herderite
:Herderite rdf:type owl:NamedIndividual ,
                    :Phosphates_Arsenates_Vanadates ;
           rdfs:comment """Herderite is a phosphate mineral belonging to the apatite, phosphate group, with formula CaBe(PO4)(F,OH).

Resource: https://en.wikipedia.org/wiki/Herderite""" .


###  http://www.semanticweb.org/ontologies/2022/6/geological_taxonomy#Howardevansite
:Howardevansite rdf:type owl:NamedIndividual ,
                         :Phosphates_Arsenates_Vanadates ;
                rdfs:comment """A triclinic-pinacoidal black mineral containing copper, iron, oxygen, sodium, and vanadium.
Chemical Formula: NaCuFe2(VO4)3

Resource: https://en.wiktionary.org/wiki/howardevansite
https://www.mindat.org/min-1934.html""" .


###  http://www.semanticweb.org/ontologies/2022/6/geological_taxonomy#Howlite
:Howlite rdf:type owl:NamedIndividual ,
                  :Borates ;
         rdfs:comment """Howlite, a calcium borosilicate hydroxide (Ca2B5SiO9(OH)5), is a borate mineral found in evaporite deposits.

Resource: https://en.wikipedia.org/wiki/Howlite""" .


###  http://www.semanticweb.org/ontologies/2022/6/geological_taxonomy#Humboldtine
:Humboldtine rdf:type owl:NamedIndividual ,
                      :Organic_compounds ;
             rdfs:comment """Humboldtine is a rarely occurring mineral from the mineral class of \"organic compounds\" with the chemical composition FeC2O4•2H2O and is therefore a water-containing iron(II) oxalate or the iron salt of oxalic acid.

Resource: https://en.wikipedia.org/wiki/Humboldtine""" .


###  http://www.semanticweb.org/ontologies/2022/6/geological_taxonomy#Hydrohalite
:Hydrohalite rdf:type owl:NamedIndividual ,
                      :Halides ;
             rdfs:comment """Hydrohalite is a mineral that occurs in saturated halite brines at cold temperatures (below 0.1 °C). It was first described in 1847 in Dürrnberg, Austria. It exists in cold weather.

Resource: https://en.wikipedia.org/wiki/Hydrohalite""" .


###  http://www.semanticweb.org/ontologies/2022/6/geological_taxonomy#IMA2008-029
:IMA2008-029 rdf:type owl:NamedIndividual ,
                      :Sulfates ;
             rdfs:comment """Chemical Formula: (NH4)3Fe(SO4)3

Resource: https://www.mindat.org/min-39464.html""" .


###  http://www.semanticweb.org/ontologies/2022/6/geological_taxonomy#IMA2008-054
:IMA2008-054 rdf:type owl:NamedIndividual ,
                      :Phosphates_Arsenates_Vanadates ;
             rdfs:comment """Chemical Formula: NaCaMn2(PO4)[PO3(OH)]2

Resource: http://webmineral.com/data/IMA2008-054.shtml#.Yy8d1XZBzIU""" .


###  http://www.semanticweb.org/ontologies/2022/6/geological_taxonomy#Ice
:Ice rdf:type owl:NamedIndividual ,
              :Oxides ;
     rdfs:comment """Ice is water frozen into a solid state, typically forming at or below temperatures of 0 degrees Celsius or 32 °F 
Chemical Formula: H2O

Resource: https://en.wikipedia.org/wiki/Ice
https://www.mindat.org/min-2001.html""" .


###  http://www.semanticweb.org/ontologies/2022/6/geological_taxonomy#Indium
:Indium rdf:type owl:NamedIndividual ,
                 :Elements ;
        rdfs:comment """Indium is a chemical element with the symbol In and atomic number 49. Indium is the softest metal that is not an alkali metal.

Resource: https://en.wikipedia.org/wiki/Indium""" .


###  http://www.semanticweb.org/ontologies/2022/6/geological_taxonomy#Ivanyukite-Cu
:Ivanyukite-Cu rdf:type owl:NamedIndividual ,
                        :Silicates ;
               rdfs:comment """Chemical Formula: C uTi4(SiO4)3(OH)2O2 · 7H2O

Resource: https://www.mindat.org/min-32620.html""" .


###  http://www.semanticweb.org/ontologies/2022/6/geological_taxonomy#Ivanyukite-Na
:Ivanyukite-Na rdf:type owl:NamedIndividual ,
                        :Silicates ;
               rdfs:comment """Chemical Formula: Na2Ti4(SiO4)3(OH)2O2 · 6H2O

Resource: https://www.mindat.org/min-32618.html""" .


###  http://www.semanticweb.org/ontologies/2022/6/geological_taxonomy#Jadeite
:Jadeite rdf:type owl:NamedIndividual ,
                  :Silicates ;
         rdfs:comment """Jadeite is a pyroxene mineral with composition NaAlSi2O6. It is hard (Mohs hardness of about 6.5 to 7.0), very tough, and dense, with a specific gravity of about 3.4.

Resource: https://en.wikipedia.org/wiki/Jadeite""" .


###  http://www.semanticweb.org/ontologies/2022/6/geological_taxonomy#Jeremejevite
:Jeremejevite rdf:type owl:NamedIndividual ,
                       :Borates ;
              rdfs:comment """Jeremejevite is an aluminium borate mineral with variable fluoride and hydroxide ions. Its chemical formula is Al6B5O15(F,OH)3.

Resource: https://en.wikipedia.org/wiki/Jeremejevite""" .


###  http://www.semanticweb.org/ontologies/2022/6/geological_taxonomy#Johachidolite
:Johachidolite rdf:type owl:NamedIndividual ,
                        :Borates ;
               rdfs:comment """An orthorhombic-dipyramidal mineral containing aluminum, boron, calcium, and oxygen.
Chemical Formula: CaAlB3O7

Resource: https://en.wiktionary.org/wiki/johachidolite
https://www.mindat.org/min-2101.html""" .


###  http://www.semanticweb.org/ontologies/2022/6/geological_taxonomy#Julienite
:Julienite rdf:type owl:NamedIndividual ,
                    :Organic_compounds ;
           rdfs:comment """Chemical Formula: Na2[Co(SCN)4] · 8H2O

Resource: https://www.mindat.org/min-2121.html""" .


###  http://www.semanticweb.org/ontologies/2022/6/geological_taxonomy#Kafehydrocyanite
:Kafehydrocyanite rdf:type owl:NamedIndividual ,
                           :Organic_compounds ;
                  rdfs:comment """Chemical Formula: K4[Fe(CN)6] · H2O

Resource: https://www.mindat.org/min-2130.html""" .


###  http://www.semanticweb.org/ontologies/2022/6/geological_taxonomy#Kornerupine
:Kornerupine rdf:type owl:NamedIndividual ,
                      :Silicates ;
             rdfs:comment """Kornerupine (also called Prismatine) is a rare boro-silicate mineral with the chemical formula (Mg,Fe2+)4(Al,Fe3+)6(SiO4,BO4)5(O,OH)2. It crystallizes in the orthorhombic - dipyramidal crystal system as brown, green, yellow to colorless slender tourmaline like prisms or in massive fibrous forms. 

Resource: https://en.wikipedia.org/wiki/Kornerupine""" .


###  http://www.semanticweb.org/ontologies/2022/6/geological_taxonomy#Kyanite
:Kyanite rdf:type owl:NamedIndividual ,
                  :Silicates ;
         rdfs:comment """Kyanite, also spelled cyanite, also called disthene, silicate mineral that is formed during the regional metamorphism of clay-rich sediments.
Chemical Formula: Al2(SiO4)

Resource: https://www.britannica.com/science/kyanite
https://www.mindat.org/min-2303.html""" .


###  http://www.semanticweb.org/ontologies/2022/6/geological_taxonomy#Larsenite
:Larsenite rdf:type owl:NamedIndividual ,
                    :Silicates ;
           rdfs:comment """A nesosilicate mineral.
Chemical Formula: PbZnSiO4

Resource: https://www.wikidata.org/wiki/Q3827220
https://www.mindat.org/min-2335.html""" .


###  http://www.semanticweb.org/ontologies/2022/6/geological_taxonomy#Lazulite
:Lazulite rdf:type owl:NamedIndividual ,
                   :Phosphates_Arsenates_Vanadates ;
          rdfs:comment """Lazulite ((Mg,Fe2+)Al2(PO4)2(OH)2)[3] is a blue, phosphate mineral containing magnesium, iron, and aluminium phosphate.

Resource: https://en.wikipedia.org/wiki/Lazulite""" .


###  http://www.semanticweb.org/ontologies/2022/6/geological_taxonomy#Lead
:Lead rdf:type owl:NamedIndividual ,
               :Elements ;
      rdfs:comment """Lead is a soft, malleable, ductile and dense metallic element.
Chemical Formula: Pb

Resource: https://www.nrcan.gc.ca/our-natural-resources/minerals-mining/minerals-metals-facts/lead-facts/20518
https://www.mindat.org/min-2358.html""" .


###  http://www.semanticweb.org/ontologies/2022/6/geological_taxonomy#Leucite
:Leucite rdf:type owl:NamedIndividual ,
                  :Silicates ;
         rdfs:comment """Leucite is a rock-forming mineral of the feldspathoid group, silica-undersaturated and composed of potassium and aluminium tectosilicate KAlSi2O6.

Resource: https://en.wikipedia.org/wiki/Leucite""" .


###  http://www.semanticweb.org/ontologies/2022/6/geological_taxonomy#Lindbergite
:Lindbergite rdf:type owl:NamedIndividual ,
                      :Organic_compounds ;
             rdfs:comment """A monoclinic-prismatic mineral containing aluminum, carbon, hydrogen, manganese, oxygen, and sodium.
Chemical Formula: Mn2+(C2O4) · 2H2O

Resource: https://en.wiktionary.org/wiki/lindbergite
https://www.mindat.org/min-26578.html""" .


###  http://www.semanticweb.org/ontologies/2022/6/geological_taxonomy#Lizardite
:Lizardite rdf:type owl:NamedIndividual ,
                    :Silicates ;
           rdfs:comment """Lizardite is a mineral from the serpentine group with formula Mg3(Si2O5)(OH)4, and the most common type of mineral in the group. It is also a member of the kaolinite-serpentine group.

Resource: https://en.wikipedia.org/wiki/Lizardite""" .


###  http://www.semanticweb.org/ontologies/2022/6/geological_taxonomy#Magnesite
:Magnesite rdf:type owl:NamedIndividual ,
                    :Carbonates ;
           rdfs:comment """Magnesite is a mineral with the chemical formula MgCO
3 (magnesium carbonate). Iron, manganese, cobalt, and nickel may occur as admixtures, but only in small amounts.

Resource: https://en.wikipedia.org/wiki/Magnesite""" .


###  http://www.semanticweb.org/ontologies/2022/6/geological_taxonomy#Malachite
:Malachite rdf:type owl:NamedIndividual ,
                    :Carbonates ;
           rdfs:comment """Malachite is a copper carbonate hydroxide mineral, with the formula Cu2CO3(OH)2. This opaque, green-banded mineral crystallizes in the monoclinic crystal system, and most often forms botryoidal, fibrous, or stalagmitic masses, in fractures and deep, underground spaces, where the water table and hydrothermal fluids provide the means for chemical precipitation. Individual crystals are rare, but occur as slender to acicular prisms.

Resource: https://en.wikipedia.org/wiki/Malachite""" .


###  http://www.semanticweb.org/ontologies/2022/6/geological_taxonomy#Manganostibite
:Manganostibite rdf:type owl:NamedIndividual ,
                         :Oxides ;
                rdfs:comment """Chemical Formula: (Mn,Fe)7SbAsO12

Resource: https://www.mindat.org/min-2528.html""" .


###  http://www.semanticweb.org/ontologies/2022/6/geological_taxonomy#Marialite
:Marialite rdf:type owl:NamedIndividual ,
                    :Silicates ;
           rdfs:comment """Marialite is a silicate mineral with a chemical formula of Na4Al3Si9O24Cl

Resource: https://en.wikipedia.org/wiki/Marialite""" .


###  http://www.semanticweb.org/ontologies/2022/6/geological_taxonomy#Mascagnite
:Mascagnite rdf:type owl:NamedIndividual ,
                     :Sulfates ;
            rdfs:comment """Mascagnite is a rare ammonium sulfate mineral (NH4)2SO4.

Resource: https://en.wikipedia.org/wiki/Mascagnite""" .


###  http://www.semanticweb.org/ontologies/2022/6/geological_taxonomy#Maucherite
:Maucherite rdf:type owl:NamedIndividual ,
                     :Sulfides_and_Sulfosalts ;
            rdfs:comment """Maucherite is a grey to reddish silver white nickel arsenide mineral. It crystallizes in the tetragonal crystal system. 
Chemical Formula: Ni11As8

Resource: https://en.wikipedia.org/wiki/Maucherite
https://www.mindat.org/min-2599.html""" .


###  http://www.semanticweb.org/ontologies/2022/6/geological_taxonomy#Mellite
:Mellite rdf:type owl:NamedIndividual ,
                  :Organic_compounds ;
         rdfs:comment """Mellite, also called honeystone, is an unusual mineral being also an organic chemical. It is chemically identified as an aluminium salt of mellitic acid, and specifically as aluminium benzene hexacarboxylate hydrate, with the chemical formula Al2C6(COO)6·16H2O.

Resource: https://en.wikipedia.org/wiki/Mellite""" .


###  http://www.semanticweb.org/ontologies/2022/6/geological_taxonomy#Mercury
:Mercury rdf:type owl:NamedIndividual ,
                  :Elements ;
         rdfs:comment """Mercury is a chemical element with the symbol Hg and atomic number 80. It is also known as quicksilver.

Resource: https://en.wikipedia.org/wiki/Mercury_(element)""" .


###  http://www.semanticweb.org/ontologies/2022/6/geological_taxonomy#Microcline
:Microcline rdf:type owl:NamedIndividual ,
                     :Silicates ;
            rdfs:comment """Microcline (KAlSi3O8) is an important igneous rock-forming tectosilicate mineral. It is a potassium-rich alkali feldspar.

Resource: https://en.wikipedia.org/wiki/Microcline""" .


###  http://www.semanticweb.org/ontologies/2022/6/geological_taxonomy#Mikasaite
:Mikasaite rdf:type owl:NamedIndividual ,
                    :Sulfates ;
           rdfs:comment """A trigonal-rhombohedral mineral containing iron, oxygen, and sulfur.
Chemical Formula: Fe2(SO4)3

Resource: https://en.wiktionary.org/wiki/mikasaite
https://www.mindat.org/min-2709.html""" .


###  http://www.semanticweb.org/ontologies/2022/6/geological_taxonomy#Millosevichite
:Millosevichite rdf:type owl:NamedIndividual ,
                         :Sulfates ;
                rdfs:comment """Millosevichite is a rare sulfate mineral with the chemical formula Al2(SO4)3.

Resource: https://en.wikipedia.org/wiki/Millosevichite""" .


###  http://www.semanticweb.org/ontologies/2022/6/geological_taxonomy#Molysite
:Molysite rdf:type owl:NamedIndividual ,
                   :Halides ;
          rdfs:comment """A trigonal-rhombohedral mineral containing chlorine and iron.
Chemical Formula: FeCl3

Resource: https://en.wiktionary.org/wiki/molysite
https://www.mindat.org/min-2749.html""" .


###  http://www.semanticweb.org/ontologies/2022/6/geological_taxonomy#Montebrasite
:Montebrasite rdf:type owl:NamedIndividual ,
                       :Phosphates_Arsenates_Vanadates ;
              rdfs:comment """Chemical Formula: LiAl(PO4)(OH)

Resource: https://www.mindat.org/min-2763.html""" .


###  http://www.semanticweb.org/ontologies/2022/6/geological_taxonomy#Nahpoite
:Nahpoite rdf:type owl:NamedIndividual ,
                   :Phosphates_Arsenates_Vanadates ;
          rdfs:comment """A monoclinic white mineral containing hydrogen, oxygen, phosphorus, and sodium.
Chemical Formula: Na2(PO3OH)

Resource: https://en.wiktionary.org/wiki/nahpoite
https://www.mindat.org/min-2832.html""" .


###  http://www.semanticweb.org/ontologies/2022/6/geological_taxonomy#Nantokite
:Nantokite rdf:type owl:NamedIndividual ,
                    :Halides ;
           rdfs:comment """An isometric-hextetrahedral mineral containing chlorine and copper.
Chemical Formula: CuCl

Resource: https://en.wiktionary.org/wiki/nantokite
https://www.mindat.org/min-2840.html""" .


###  http://www.semanticweb.org/ontologies/2022/6/geological_taxonomy#Natrolite
:Natrolite rdf:type owl:NamedIndividual ,
                    :Silicates ;
           rdfs:comment """Natrolite is a tectosilicate mineral species belonging to the zeolite group. It is a hydrated sodium and aluminium silicate with the formula Na2Al2Si3O10 · 2H2O.

Resource: https://en.wikipedia.org/wiki/Natrolite""" .


###  http://www.semanticweb.org/ontologies/2022/6/geological_taxonomy#Nordenskioldine
:Nordenskioldine rdf:type owl:NamedIndividual ,
                          :Borates ;
                 rdfs:comment """Nordenskioldine is a fairly rare tin-borate and is found in less than 15 localities worldwide. It typically occurs in alkaline pegmatites, (Arø Island, Norway); in a metasomatized marble (Arandis, Namibia); and in skarns deposits (Xianghualing mine, China & this occurence, the MW claim). 
Formula: CaSn4+[BO3]2

Resource: https://www.dakotamatrix.com/products/14984/nordenskioldine
https://www.mindat.org/min-2926.html""" .


###  http://www.semanticweb.org/ontologies/2022/6/geological_taxonomy#Nyerereite
:Nyerereite rdf:type owl:NamedIndividual ,
                     :Carbonates ;
            rdfs:comment """Nyerereite is a very rare sodium calcium carbonate mineral with formula Na2Ca(CO3)2. It forms colorless, platey pseudohexagonal orthorhombic crystals that are typically twinned.

Resource: https://en.wikipedia.org/wiki/Nyerereite""" .


###  http://www.semanticweb.org/ontologies/2022/6/geological_taxonomy#Opal
:Opal rdf:type owl:NamedIndividual ,
               :Oxides ;
      rdfs:comment """The opal is a fairly white rock mineral.
Chemical Formula: SiO2 · nH2O

Resource: https://simple.wikipedia.org/wiki/Opal
https://www.mindat.org/min-3004.html""" .


###  http://www.semanticweb.org/ontologies/2022/6/geological_taxonomy#Orcelite
:Orcelite rdf:type owl:NamedIndividual ,
                   :Sulfides_and_Sulfosalts ;
          rdfs:comment """A hexagonal-dihexagonal pyramidal orange white mineral containing arsenic and nickel.
Formula:Ni5-xAs2, x ~ 0.25

Resource: https://en.wiktionary.org/wiki/orcelite
https://www.mindat.org/min-3012.html""" .


###  http://www.semanticweb.org/ontologies/2022/6/geological_taxonomy#Orthoclase
:Orthoclase rdf:type owl:NamedIndividual ,
                     :Silicates ;
            rdfs:comment """Orthoclase, or orthoclase feldspar (endmember formula KAlSi3O8), is an important tectosilicate mineral which forms igneous rock.

Resource: https://en.wikipedia.org/wiki/Orthoclase""" .


###  http://www.semanticweb.org/ontologies/2022/6/geological_taxonomy#Panichiite
:Panichiite rdf:type owl:NamedIndividual ,
                     :Halides ;
            rdfs:comment """Chemical Formula:(NH4)2SnCl6

Resource: https://www.mindat.org/min-35969.html""" .


###  http://www.semanticweb.org/ontologies/2022/6/geological_taxonomy#Pargasite
:Pargasite rdf:type owl:NamedIndividual ,
                    :Silicates ;
           rdfs:comment """Pargasite is a complex inosilicate mineral of the amphibole group with formula NaCa2(Mg4Al)(Si6Al2)O22(OH)2.

Resource: https://en.wikipedia.org/wiki/Pargasite""" .


###  http://www.semanticweb.org/ontologies/2022/6/geological_taxonomy#Pectolite
:Pectolite rdf:type owl:NamedIndividual ,
                    :Silicates ;
           rdfs:comment """Pectolite is a white to gray mineral, NaCa2Si3O8(OH), sodium calcium hydroxide inosilicate. It crystallizes in the triclinic system typically occurring in radiated or fibrous crystalline masses.

Resource: https://en.wikipedia.org/wiki/Pectolite""" .


###  http://www.semanticweb.org/ontologies/2022/6/geological_taxonomy#Petalite
:Petalite rdf:type owl:NamedIndividual ,
                   :Silicates ;
          rdfs:comment """Petalite, also known as castorite, is a lithium aluminium phyllosilicate mineral LiAlSi4O10, crystallizing in the monoclinic system.

Resource: https://en.wikipedia.org/wiki/Petalite""" .


###  http://www.semanticweb.org/ontologies/2022/6/geological_taxonomy#Phenakite
:Phenakite rdf:type owl:NamedIndividual ,
                    :Silicates ;
           rdfs:comment """Phenakite or phenacite is a fairly rare nesosilicate mineral consisting of beryllium orthosilicate, Be2SiO4. Occasionally used as a gemstone.

Resource: https://en.wikipedia.org/wiki/Phenakite""" .


###  http://www.semanticweb.org/ontologies/2022/6/geological_taxonomy#Phosphosiderite
:Phosphosiderite rdf:type owl:NamedIndividual ,
                          :Phosphates_Arsenates_Vanadates ;
                 rdfs:comment """Phosphosiderite is a rare mineral named for its main components, phosphate and iron.
Chemical Formula: FePO4 · 2H2O

Resource: https://en.wikipedia.org/wiki/Phosphosiderite
https://www.mindat.org/min-3187.html""" .


###  http://www.semanticweb.org/ontologies/2022/6/geological_taxonomy#Pollucite
:Pollucite rdf:type owl:NamedIndividual ,
                    :Silicates ;
           rdfs:comment """Pollucite is a zeolite mineral with the formula (Cs,Na)2Al2Si4O12·2H2O with iron, calcium, rubidium and potassium as common substituting elements.

Resource: https://en.wikipedia.org/wiki/Pollucite""" .


###  http://www.semanticweb.org/ontologies/2022/6/geological_taxonomy#Prehnite
:Prehnite rdf:type owl:NamedIndividual ,
                   :Silicates ;
          rdfs:comment """Prehnite is an inosilicate of calcium and aluminium with the formula: Ca2Al(AlSi3O10)(OH)2.

Resource: https://en.wikipedia.org/wiki/Prehnite""" .


###  http://www.semanticweb.org/ontologies/2022/6/geological_taxonomy#Pyrope
:Pyrope rdf:type owl:NamedIndividual ,
                 :Silicates ;
        rdfs:comment """The mineral pyrope is a member of the garnet group. Pyrope is the only member of the garnet family to always display red colouration in natural samples
Chemical Formula: Mg3Al2(SiO4)3

Resource: https://en.wikipedia.org/wiki/Pyrope
https://www.mindat.org/min-3321.html""" .


###  http://www.semanticweb.org/ontologies/2022/6/geological_taxonomy#Quartz
:Quartz rdf:type owl:NamedIndividual ,
                 :Oxides ;
        rdfs:comment """Quartz is a hard, crystalline mineral composed of silica (silicon dioxide). 
Chemical Formula: SiO2

Resource: https://en.wikipedia.org/wiki/Quartz""" .


###  http://www.semanticweb.org/ontologies/2022/6/geological_taxonomy#Rhodochrosite
:Rhodochrosite rdf:type owl:NamedIndividual ,
                        :Carbonates ;
               rdfs:comment """Rhodochrosite is a manganese carbonate mineral with chemical composition MnCO3. 

Resource: https://en.wikipedia.org/wiki/Rhodochrosite""" .


###  http://www.semanticweb.org/ontologies/2022/6/geological_taxonomy#Rhodonite
:Rhodonite rdf:type owl:NamedIndividual ,
                    :Silicates ;
           rdfs:comment """Rhodonite, silicate mineral that occurs as rounded crystals, masses, or grains in various manganese ores, often with rhodochrosite.
Chemical Formula: CaMn3Mn[Si5O15]

Resource: https://www.britannica.com/science/rhodonite
https://www.mindat.org/min-3407.html""" .


###  http://www.semanticweb.org/ontologies/2022/6/geological_taxonomy#Rutile
:Rutile rdf:type owl:NamedIndividual ,
                 :Oxides ;
        rdfs:comment """Rutile is an oxide mineral composed of titanium dioxide (TiO2).

Resource: https://en.wikipedia.org/wiki/Rutile""" .


###  http://www.semanticweb.org/ontologies/2022/6/geological_taxonomy#Sanidine
:Sanidine rdf:type owl:NamedIndividual ,
                   :Silicates ;
          rdfs:comment """Sanidine is the high temperature form of potassium feldspar with a general formula K(AlSi3O8).[2] Sanidine is found most typically in felsic volcanic rocks such as obsidian, rhyolite and trachyte. 

Resource: https://en.wikipedia.org/wiki/Sanidine""" .


###  http://www.semanticweb.org/ontologies/2022/6/geological_taxonomy#Sapphirine
:Sapphirine rdf:type owl:NamedIndividual ,
                     :Silicates ;
            rdfs:comment """Sapphirine is a rare mineral, a silicate of magnesium and aluminium with the chemical formula (Mg,Al)8(Al,Si)6O20

Resource: https://en.wikipedia.org/wiki/Sapphirine""" .


###  http://www.semanticweb.org/ontologies/2022/6/geological_taxonomy#Sassolite
:Sassolite rdf:type owl:NamedIndividual ,
                    :Borates ;
           rdfs:comment """Sassolite is a borate mineral, specifically the mineral form of boric acid. It is usually white to gray, and colourless in transmitted light.
Chemical Formula: H3BO3

Resource: https://en.wikipedia.org/wiki/Sassolite
https://www.mindat.org/min-3540.html""" .


###  http://www.semanticweb.org/ontologies/2022/6/geological_taxonomy#Scheelite
:Scheelite rdf:type owl:NamedIndividual ,
                    :Sulfates ;
           rdfs:comment """Scheelite is a calcium tungstate mineral with the chemical formula CaWO4. It is an important ore of tungsten (wolfram).

Resource: https://en.wikipedia.org/wiki/Scheelite""" .


###  http://www.semanticweb.org/ontologies/2022/6/geological_taxonomy#Schorl
:Schorl rdf:type owl:NamedIndividual ,
                 :Silicates ;
        rdfs:comment """Chemical Formula:NaFe2+3Al6(Si6O18)(BO3)3(OH)3(OH)

Resource: https://www.mindat.org/min-3578.html""" .


###  http://www.semanticweb.org/ontologies/2022/6/geological_taxonomy#Scolecite
:Scolecite rdf:type owl:NamedIndividual ,
                    :Silicates ;
           rdfs:comment """Scolecite is a tectosilicate mineral belonging to the zeolite group; it is a hydrated calcium silicate, CaAl2Si3O10·3H2O.

Resource: https://en.wikipedia.org/wiki/Scolecite""" .


###  http://www.semanticweb.org/ontologies/2022/6/geological_taxonomy#Serendibite
:Serendibite rdf:type owl:NamedIndividual ,
                      :Silicates ;
             rdfs:comment """Serendibite is an extremely rare silicate mineral that was first discovered in 1902 in Sri Lanka
Chemical Formula: Ca4[Mg6Al6]O4[Si6B3Al3O36]

Resource: https://en.wikipedia.org/wiki/Serendibite
https://www.mindat.org/min-3623.html""" .


###  http://www.semanticweb.org/ontologies/2022/6/geological_taxonomy#Sillimanite
:Sillimanite rdf:type owl:NamedIndividual ,
                      :Silicates ;
             rdfs:comment """Sillimanite is an aluminosilicate mineral with the chemical formula Al2SiO5.

Resource: https://en.wikipedia.org/wiki/Sillimanite""" .


###  http://www.semanticweb.org/ontologies/2022/6/geological_taxonomy#Sinhalite
:Sinhalite rdf:type owl:NamedIndividual ,
                    :Borates ;
           rdfs:comment """Sinhalite is a borate mineral with formula MgAl(BO4). 
Sinhalite was first found in Sri Lanka (Ceylon) in 1952, and was named from Sinhala - the Sanskrit name for Sri Lanka.

Resource: https://en.wikipedia.org/wiki/Sinhalite""" .


###  http://www.semanticweb.org/ontologies/2022/6/geological_taxonomy#Smithsonite
:Smithsonite rdf:type owl:NamedIndividual ,
                      :Carbonates ;
             rdfs:comment """Smithsonite, also known as zinc spar, is the mineral form of zinc carbonate (ZnCO3).

Resource: https://en.wikipedia.org/wiki/Smithsonite""" .


###  http://www.semanticweb.org/ontologies/2022/6/geological_taxonomy#Sodalite
:Sodalite rdf:type owl:NamedIndividual ,
                   :Silicates ;
          rdfs:comment """Sodalite is a tectosilicate mineral with the formula Na8(Al6Si6O24)Cl2, with royal blue varieties widely used as an ornamental gemstone. 

Resource: https://en.wikipedia.org/wiki/Sodalite""" .


###  http://www.semanticweb.org/ontologies/2022/6/geological_taxonomy#Spessartine
:Spessartine rdf:type owl:NamedIndividual ,
                      :Silicates ;
             rdfs:comment """Spessartine is a nesosilicate, manganese aluminium garnet species, Mn2+3Al2(SiO4)3. This mineral is sometimes mistakenly referred to as spessartite.

Resource: https://en.wikipedia.org/wiki/Spessartine""" .


###  http://www.semanticweb.org/ontologies/2022/6/geological_taxonomy#Sphalerite
:Sphalerite rdf:type owl:NamedIndividual ,
                     :Sulfides_and_Sulfosalts ;
            rdfs:comment """Sphalerite (sometimes spelled sphaelerite) is a sulfide mineral with the chemical formula (Zn,Fe)S. It is the most important ore of zinc.

Resource: https://en.wikipedia.org/wiki/Sphalerite""" .


###  http://www.semanticweb.org/ontologies/2022/6/geological_taxonomy#Spinel
:Spinel rdf:type owl:NamedIndividual ,
                 :Oxides ;
        rdfs:comment """Spinel is the magnesium/aluminium member of the larger spinel group of minerals. It has the formula MgAl2O4 in the cubic crystal system.

Resource: https://en.wikipedia.org/wiki/Spinel""" .


###  http://www.semanticweb.org/ontologies/2022/6/geological_taxonomy#Spodumene
:Spodumene rdf:type owl:NamedIndividual ,
                    :Silicates ;
           rdfs:comment """Spodumene is a pyroxene mineral consisting of lithium aluminium inosilicate, LiAl(SiO3)2, and is a source of lithium.

Resource: https://en.wikipedia.org/wiki/Spodumene""" .


###  http://www.semanticweb.org/ontologies/2022/6/geological_taxonomy#Sugilite
:Sugilite rdf:type owl:NamedIndividual ,
                   :Silicates ;
          rdfs:comment """Sugilite is a relatively rare pink to purple cyclosilicate mineral with the complex chemical formula KNa2(Fe, Mn, Al)2Li3Si12O30. 

Resource: https://en.wikipedia.org/wiki/Sugilite""" .


###  http://www.semanticweb.org/ontologies/2022/6/geological_taxonomy#Svenekite
:Svenekite rdf:type owl:NamedIndividual ,
                    :Phosphates_Arsenates_Vanadates ;
           rdfs:comment """Chemical Formula: Ca(H2AsO4)2

Resource: https://www.mindat.org/min-7076.html""" .


###  http://www.semanticweb.org/ontologies/2022/6/geological_taxonomy#Swedenborgite
:Swedenborgite rdf:type owl:NamedIndividual ,
                        :Oxides ;
               rdfs:comment """A hexagonal-dihexagonal pyramidal mineral containing antimony, beryllium, oxygen, and sodium.
Formula:NaBe4Sb5+O7

Resource: https://en.wiktionary.org/wiki/swedenborgite
https://www.mindat.org/min-3845.html""" .


###  http://www.semanticweb.org/ontologies/2022/6/geological_taxonomy#Tenorite
:Tenorite rdf:type owl:NamedIndividual ,
                   :Oxides ;
          rdfs:comment """Tenorite is a copper oxide mineral with the chemical formula CuO.

Resource: https://en.wikipedia.org/wiki/Tenorite""" .


###  http://www.semanticweb.org/ontologies/2022/6/geological_taxonomy#Tin
:Tin rdf:type owl:NamedIndividual ,
              :Elements ;
     rdfs:comment """Tin is a chemical element with the symbol Sn (from Latin: stannum) and atomic number 50. Tin is a silvery-coloured metal.

Resource: https://en.wikipedia.org/wiki/Tin""" .


###  http://www.semanticweb.org/ontologies/2022/6/geological_taxonomy#Titanite
:Titanite rdf:type owl:NamedIndividual ,
                   :Silicates ;
          rdfs:comment """Titanite, or sphene (from the Greek sphenos (σφηνώ), meaning wedge[5]), is a calcium titanium nesosilicate mineral, CaTiSiO5.

Resource: https://en.wikipedia.org/wiki/Titanite""" .


###  http://www.semanticweb.org/ontologies/2022/6/geological_taxonomy#Tolbachite
:Tolbachite rdf:type owl:NamedIndividual ,
                     :Halides ;
            rdfs:comment """A monoclinic-prismatic mineral containing chlorine and copper.
Formula: CuCl2

Resource: https://en.wiktionary.org/wiki/tolbachite
https://www.mindat.org/min-3990.html""" .


###  http://www.semanticweb.org/ontologies/2022/6/geological_taxonomy#Topaz
:Topaz rdf:type owl:NamedIndividual ,
                :Silicates ;
       rdfs:comment """Topaz is a silicate mineral of aluminium and fluorine with the chemical formula Al2SiO4(F,OH)2.

Resource: https://en.wikipedia.org/wiki/Topaz""" .


###  http://www.semanticweb.org/ontologies/2022/6/geological_taxonomy#Trimerite
:Trimerite rdf:type owl:NamedIndividual ,
                    :Silicates ;
           rdfs:comment """A monoclinic-prismatic mineral containing beryllium, calcium, manganese, oxygen, and silicon.
Formula:CaMn2+2Be3(SiO4)3

Resource: https://en.wiktionary.org/wiki/trimerite
https://www.mindat.org/min-4018.html""" .


###  http://www.semanticweb.org/ontologies/2022/6/geological_taxonomy#Triplite
:Triplite rdf:type owl:NamedIndividual ,
                   :Phosphates_Arsenates_Vanadates ;
          rdfs:comment """Triplite is a rare phosphate mineral with formula: (Mn, Fe)2PO4(F, OH). It occurs in phosphate-rich granitic pegmatites typically as irregular brown opaque masses.

Resource: https://en.wikipedia.org/wiki/Triplite""" .


###  http://www.semanticweb.org/ontologies/2022/6/geological_taxonomy#Turquoise
:Turquoise rdf:type owl:NamedIndividual ,
                    :Phosphates_Arsenates_Vanadates ;
           rdfs:comment """Turquoise is an opaque, blue-to-green mineral that is a hydrated phosphate of copper and aluminium, with the chemical formula CuAl6(PO4)4(OH)8·4H2O.

Resource: https://en.wikipedia.org/wiki/Turquoise""" .


###  http://www.semanticweb.org/ontologies/2022/6/geological_taxonomy#Uvite
:Uvite rdf:type owl:NamedIndividual ,
                :Silicates ;
       rdfs:comment """Formula:CaMg3(Al5Mg)(Si6O18)(BO3)3(OH)3(OH)

Resource: https://www.mindat.org/min-54355.html""" .


###  http://www.semanticweb.org/ontologies/2022/6/geological_taxonomy#Vanthoffite
:Vanthoffite rdf:type owl:NamedIndividual ,
                      :Sulfates ;
             rdfs:comment """A monoclinic-prismatic colorless mineral containing magnesium, oxygen, sodium, and sulfur. 
Formula:Na6Mg(SO4)4

Resource: https://en.wiktionary.org/wiki/vanthoffite
https://www.mindat.org/min-4151.html""" .


###  http://www.semanticweb.org/ontologies/2022/6/geological_taxonomy#Variscite
:Variscite rdf:type owl:NamedIndividual ,
                    :Phosphates_Arsenates_Vanadates ;
           rdfs:comment """Variscite is a hydrated aluminium phosphate mineral (AlPO4 · 2 H2O). It is a relatively rare phosphate mineral.

Resource: https://en.wikipedia.org/wiki/Variscite""" .


###  http://www.semanticweb.org/ontologies/2022/6/geological_taxonomy#Vesuvianite
:Vesuvianite rdf:type owl:NamedIndividual ,
                      :Silicates ;
             rdfs:comment """Vesuvianite, also known as idocrase, is a green, brown, yellow, or blue silicate mineral.
Chemical Formula: Ca19Fe3+Al4(Al6Mg2)(◻4)◻[Si2O7]4[(SiO4)10]O(OH)9

Resource: https://en.wikipedia.org/wiki/Vesuvianite
https://www.mindat.org/min-4223.html""" .


###  http://www.semanticweb.org/ontologies/2022/6/geological_taxonomy#Vincentite
:Vincentite rdf:type owl:NamedIndividual ,
                     :Sulfides_and_Sulfosalts ;
            rdfs:comment """A monoclinic gray mineral containing antimony, arsenic, palladium, platinum, and tellurium.
Formula:Pd3As

Resource: https://en.wiktionary.org/wiki/vincentite
https://www.mindat.org/min-4184.html""" .


###  http://www.semanticweb.org/ontologies/2022/6/geological_taxonomy#Vlasovite
:Vlasovite rdf:type owl:NamedIndividual ,
                    :Silicates ;
           rdfs:comment """Vlasovite is a rare inosilicate (chain silicate) mineral with sodium and zirconium, with the chemical formula Na2ZrSi4O11. It was discovered in 1961 

Resource: https://en.wikipedia.org/wiki/Vlasovite""" .


###  http://www.semanticweb.org/ontologies/2022/6/geological_taxonomy#Väyrynenite
:Väyrynenite rdf:type owl:NamedIndividual ,
                      :Phosphates_Arsenates_Vanadates ;
             rdfs:comment """Väyrynenite is a rare phosphate mineral with formula MnBe(PO4)(OH,F).

Resource: https://en.wikipedia.org/wiki/V%C3%A4yrynenite""" .


###  http://www.semanticweb.org/ontologies/2022/6/geological_taxonomy#Zabuyelite
:Zabuyelite rdf:type owl:NamedIndividual ,
                     :Carbonates ;
            rdfs:comment """Zabuyelite is the natural mineral form of lithium carbonate, with a formula Li2CO3. 

Resource: https://en.wikipedia.org/wiki/Zabuyelite""" .


###  http://www.semanticweb.org/ontologies/2022/6/geological_taxonomy#Zharchikhite
:Zharchikhite rdf:type owl:NamedIndividual ,
                       :Halides ;
              rdfs:comment """Zharchikhite is a halide mineral, a hydroxyl fluoride of aluminium; formula AlF(OH)2. It forms colourless, transparent crystals.

Resource: https://en.wikipedia.org/wiki/Zharchikhite""" .


###  http://www.semanticweb.org/ontologies/2022/6/geological_taxonomy#Zinc
:Zinc rdf:type owl:NamedIndividual ,
               :Elements ;
      rdfs:comment """Zinc is a chemical element with the symbol Zn and atomic number 30.

Resource: https://en.wikipedia.org/wiki/Zinc""" .


###  http://www.semanticweb.org/ontologies/2022/6/geological_taxonomy#Zircon
:Zircon rdf:type owl:NamedIndividual ,
                 :Silicates ;
        rdfs:comment """Zircon is a mineral belonging to the group of nesosilicates and is a source of the metal zirconium. Its chemical name is zirconium(IV) silicate, and its corresponding chemical formula is ZrSiO4.

Resource: https://en.wikipedia.org/wiki/Zircon""" .


###  http://www.semanticweb.org/ontologies/2022/6/geological_taxonomy#Zoisite
:Zoisite rdf:type owl:NamedIndividual ,
                  :Silicates ;
         rdfs:comment """Zoisite, first known as saualpite, after its type locality, is a calcium aluminium hydroxy sorosilicate belonging to the epidote group of minerals. Its chemical formula is Ca2Al3(SiO4)(Si2O7)O(OH).

Resource:  https://en.wikipedia.org/wiki/Zoisite""" .


###  http://www.semanticweb.org/ontologies/2022/6/geological_taxonomy#Axinite-(Fe)
<http://www.semanticweb.org/ontologies/2022/6/geological_taxonomy#Axinite-(Fe)> rdf:type owl:NamedIndividual ,
                                                                                         :Silicates ;
                                                                                rdfs:comment """Axinite-(Fe) or ferroaxinite, Ca2Fe2+Al2BOSi4O15(OH) iron rich, clove-brown, brown, plum-blue, pearl-gray

Resource: https://en.wikipedia.org/wiki/Axinite""" .


###  http://www.semanticweb.org/ontologies/2022/6/geological_taxonomy#Axinite-(Mg)
<http://www.semanticweb.org/ontologies/2022/6/geological_taxonomy#Axinite-(Mg)> rdf:type owl:NamedIndividual ,
                                                                                         :Silicates ;
                                                                                rdfs:comment """Axinite-(Mg) is a borosilicate mineral of aluminum, calcium and magnesium of the axinite group, with magnesium as the dominant cation in the place of the structure that can also be occupied by iron and manganese.
Chemical Formula: Ca2MgAl2BSi4O15OH

Resource: https://en.wikipedia.org/wiki/Axinite-(Mg)
https://www.mindat.org/min-2490.html""" .


###  http://www.semanticweb.org/ontologies/2022/6/geological_taxonomy#Bastnäsite-(Ce)
<http://www.semanticweb.org/ontologies/2022/6/geological_taxonomy#Bastnäsite-(Ce)> rdf:type owl:NamedIndividual ,
                                                                                            :Carbonates ;
                                                                                   rdfs:comment """Chemical Formula: Ce(CO3)F

Resource: https://www.mindat.org/min-560.html""" .


###  http://www.semanticweb.org/ontologies/2022/6/geological_taxonomy#Gadolinite-(Y)
<http://www.semanticweb.org/ontologies/2022/6/geological_taxonomy#Gadolinite-(Y)> rdf:type owl:NamedIndividual ,
                                                                                           :Silicates ;
                                                                                  rdfs:comment """Chemical Formula: Y2Fe2+Be2Si2O10

Resource: https://www.mindat.org/min-1628.html""" .


###  http://www.semanticweb.org/ontologies/2022/6/geological_taxonomy#Remondite-(Ce)
<http://www.semanticweb.org/ontologies/2022/6/geological_taxonomy#Remondite-(Ce)> rdf:type owl:NamedIndividual ,
                                                                                           :Carbonates ;
                                                                                  rdfs:comment """Chemical Formula: Na3(Ca,Ce,La,Na,Sr)3(CO3)5 
The mineral is named in honor of Dr. Guy Rémond, a physicist for the Bureau de Recherches Géologiques et Minières in Orléans, France.
Found only in Cameroon, Canada, and purportedly Russia, Remondite occurs at its Cameroon locality in nepheline syenite, and as its Canadian locality “associated with an intrusive alkalic gabbro-syenite complex.”

Resource: https://www.dakotamatrix.com/mineralpedia/7351/remondite-ce""" .


###  http://www.semanticweb.org/ontologies/2022/6/geological_taxonomy#Sahamalite-(Ce)
<http://www.semanticweb.org/ontologies/2022/6/geological_taxonomy#Sahamalite-(Ce)> rdf:type owl:NamedIndividual ,
                                                                                            :Carbonates ;
                                                                                   rdfs:comment """Chemical Formula: (Mg,Fe++)Ce2(CO3)4

Resource: http://www.webmineral.com/data/Sahamalite-(Ce).shtml#.Yy70-HZBzIU""" .


#################################################################
#    Annotations
#################################################################

:Dolomite rdfs:comment """Dolomite (also known as dolomite rock, dolostone or dolomitic rock) is a sedimentary carbonate rock that contains a high percentage of the mineral dolomite, CaMg(CO3)2. 

Resource: https://en.wikipedia.org/wiki/Dolomite_(rock)""" .


#################################################################
#    General axioms
#################################################################

[ rdf:type owl:AllDisjointClasses ;
  owl:members ( :Abnormally_Dry
                :Exceptional_Drought
                :Extreme_Drought
                :Moderate_Drought
                :Severe_Drought
              )
] .


[ rdf:type owl:AllDisjointClasses ;
  owl:members ( :Adakite
                :Hawaiite
                :Pāhoehoe
                :ʻAʻā
              )
] .


[ rdf:type owl:AllDisjointClasses ;
  owl:members ( :Albolls
                :Aquolls
                :Cryolls
                :Gelolls
                :Rendolls
                :Udolls
                :Ustolls
                :Xerolls
              )
] .


[ rdf:type owl:AllDisjointClasses ;
  owl:members ( :Alfisols
                :Andisols
                :Aridisols
                :Entisols
                :Gelisols
                :Histosols
                :Inceptisols
                :Mollisols
                :Oxisols
                :Spodosols
                :Ultisols
                :Vertisols
              )
] .


[ rdf:type owl:AllDisjointClasses ;
  owl:members ( :Alkali_feldspar_granite
                :Andesite
                :Anorthosite
                :Aplite
                :Basalt
                :Basanite
                :Blairmorite
                :Boninite
                :Carbonatite
                :Charnockite
                :Dacite
                :Diabase
                :Diorite
                :Dunite
                :Essexite
                :Foidolite
                :Foyaite
                :Gabbro
                :Granite
                :Granodiorite
                :Granophyre
                :Harzburgite
                :Hornblendite
                :Hyaloclastite
                :Icelandite
                :Ignimbrite
                :Ijolite
                :Kimberlite
                :Komatiite
                :Lamproite
                :Lamprophyre
                :Latite
                :Lherzolite
                :Limburgite
                :Monzogranite
                :Monzonite
                :Nepheline_syenite
                :Nephelinite
                :Norite
                :Obsidian
                :Pegmatite
                :Peridotite
                :Phonolite
                :Phonotephrite
                :Picrite
                :Porphyry
                :Pumice
                :Pyroxenite
                :Quartz_diorite
                :Quartz_monzonite
                :Quartzolite
                :Rapakivi
                :Rhomb-porphyry
                :Rhyodacite
                :Rhyolite
                :Scoria
                :Shonkinite
                :Sovite
                :Syenite
                :Sövite
                :Tachylyte
                :Tephriphonolite
                :Tephrite
                :Tonalite
                :Trachyandesite
                :Trachybasalt
                :Trachyte
                :Troctolite
                :Trondhjemite
                :Tuff
                :Websterite
                :Wehrlite
              )
] .


[ rdf:type owl:AllDisjointClasses ;
  owl:members ( :Amphibolite
                :Anthracite
                :Blueschist
                :Cataclasite
                :Eclogite
                :Epidosite
                :Fenite
                :Gneiss
                :Gossan
                :Granulite
                :Greenschist
                :Greisen
                :Hornfels
                :Litchfieldite
                :Marble
                :Metapelite
                :Metapsammite
                :Migmatite
                :Mylonite
                :Phyllite
                :Pseudotachylite
                :Quartzite
                :Schist
                :Serpentinite
                :Shungite
                :Skarn
                :Slate
                :Suevite
                :Talc_carbonate
                :Tectonite
                :Whiteschist
                :protolith
              )
] .


[ rdf:type owl:AllDisjointClasses ;
  owl:members ( :Anthrepts
                :Aquepts
                :Cryepts
                :Gelepts
                :Udepts
                :Ustepts
                :Xerepts
              )
] .


[ rdf:type owl:AllDisjointClasses ;
  owl:members ( :Aqualfs
                :Cryalfs
                :Udalfs
                :Ustalfs
                :Xeralfs
              )
] .


[ rdf:type owl:AllDisjointClasses ;
  owl:members ( :Aquands
                :Cryands
                :Gelands
                :Torrands
                :Udands
                :Ustands
                :Vitrands
                :Xerands
              )
] .


[ rdf:type owl:AllDisjointClasses ;
  owl:members ( :Aquents
                :Arents
                :Fluvents
                :Orthents
                :Psamments
              )
] .


[ rdf:type owl:AllDisjointClasses ;
  owl:members ( :Aquerts
                :Cryerts
                :Torrerts
                :Uderts
                :Usterts
                :Xererts
              )
] .


[ rdf:type owl:AllDisjointClasses ;
  owl:members ( :Aquods
                :Cryods
                :Gelods
                :Humods
                :Orthods
              )
] .


[ rdf:type owl:AllDisjointClasses ;
  owl:members ( :Aquox
                :Perox
                :Torrox
                :Udox
                :Ustox
              )
] .


[ rdf:type owl:AllDisjointClasses ;
  owl:members ( :Aquults
                :Humults
                :Udults
                :Ustults
                :Xerults
              )
] .


[ rdf:type owl:AllDisjointClasses ;
  owl:members ( :Areal
                :Coastal_Floods
                :Flash_flood
                <http://www.semanticweb.org/ontologies/2022/6/geological_taxonomy#Riverine_(Channel)_Floods>
              )
] .


[ rdf:type owl:AllDisjointClasses ;
  owl:members ( :Argids
                :Calcids
                :Cambids
                :Cryids
                :Durids
                :Gypsids
                :Salids
              )
] .


[ rdf:type owl:AllDisjointClasses ;
  owl:members ( :Argillite
                :Arkose
                :Banded_iron_formation
                :Bauxite
                :Bog_iron
                :Breccia
                :Calcarenite
                :Chalk
                :Chert
                :Claystone
                :Coal
                :Conglomerate
                :Coquina
                :Diatomite
                :Dolomite
                :Evaporite
                :Flint
                :Geyserite
                :Graywacke
                :Greywacke
                :Gritstone
                :Gypsum
                :Itacolumite
                :Jaspillite
                :Laterite
                :Lignite
                :Limestone
                :Marl
                :Mudstone
                :Oil_shale
                :Oolite
                :Phosphorite
                :Rock_Gypsum-
                :Sandstone
                :Shale
                :Siltstone
                :Sylvinite
                :Tillite
                :Travertine
                :Tufa
                :Turbidite
                :Umber
                :Wackestone
                <http://www.semanticweb.org/ontologies/2022/6/geological_taxonomy#Dolomite_(rock)>
              )
] .


[ rdf:type owl:AllDisjointClasses ;
  owl:members ( :Asthenosphere
                :Lithosphere
                <http://www.semanticweb.org/ontologies/2022/6/geological_taxonomy#Lithosphere–asthenosphere_boundary>
              )
] .


[ rdf:type owl:AllDisjointClasses ;
  owl:members ( :Basaltic_trachyandesite
                :Benmoreite
                :Mugearite
                :Shoshonite
              )
] .


[ rdf:type owl:AllDisjointClasses ;
  owl:members ( :Borates
                :Carbonates
                :Elements
                :Halides
                :Organic_compounds
                :Oxides
                :Phosphates_Arsenates_Vanadates
                :Silicates
                :Sulfates
                :Sulfides_and_Sulfosalts
              )
] .


[ rdf:type owl:AllDisjointClasses ;
  owl:members ( :Breaching_of_a_barrier
                :Direct_flooding
                :Overtopping_of_a_barrier
              )
] .


[ rdf:type owl:AllDisjointClasses ;
  owl:members ( :Cloudy
                :Fog
                :Rain
                :Snow
                :Stormy
                :Sunny
                :Windy
              )
] .


[ rdf:type owl:AllDisjointClasses ;
  owl:members ( :Collapse_Earthquakes
                :Explosion_Earthquakes
                :Tectonic_Earthquakes
                :Volcanic_earthquakes
              )
] .


[ rdf:type owl:AllDisjointClasses ;
  owl:members ( :Continuous_creep
                :Progressive_creep
                :Seasonal_creep
              )
] .


[ rdf:type owl:AllDisjointClasses ;
  owl:members ( :Crown_Fire
                :Ground_Fire
                :Surface_Fire
              )
] .


[ rdf:type owl:AllDisjointClasses ;
  owl:members ( :Crust
                :Mantle
                :Planetary_core
              )
] .


[ rdf:type owl:AllDisjointClasses ;
  owl:members ( :Cyclone
                :Drought
                :Earthquakes
                :Extreme_Temperature
                :Floods
                :Landslide
                :Limnic_Eruptions
                :Tsunami
                :Wildfire
              )
] .


[ rdf:type owl:AllDisjointClasses ;
  owl:members ( :Falls
                :Flows
                :Slides
                :Subsidence
                :Topples
              )
] .


[ rdf:type owl:AllDisjointClasses ;
  owl:members ( :Fibrists
                :Folists
                :Hemists
                :Saprists
              )
] .


[ rdf:type owl:AllDisjointClasses ;
  owl:members ( :Geological_Object
                :Geological_phenomena
                :Units_of_Earth_structure
              )
] .


[ rdf:type owl:AllDisjointClasses ;
  owl:members ( :Histels
                :Orthels
                :Turbels
              )
] .


[ rdf:type owl:AllDisjointClasses ;
  owl:members ( :Hurricane
                :Major_Hurricane
                :Tropical_Depression
                :Tropical_Storm
              )
] .


[ rdf:type owl:AllDisjointClasses ;
  owl:members ( :Igneous_rocks
                :Metamorphic_rocks
                :Sedimentary_rocks
              )
] .


[ rdf:type owl:AllDisjointClasses ;
  owl:members ( :Lower_mantle
                :Upper_mantle
                <http://www.semanticweb.org/ontologies/2022/6/geological_taxonomy#D_Double-Prime_(D’’)>
                <http://www.semanticweb.org/ontologies/2022/6/geological_taxonomy#Transition_zone_(Earth)>
              )
] .


[ rdf:type owl:AllDisjointClasses ;
  owl:members ( :Mineral
                :Rock
                :Soil
              )
] .


###  Generated by the OWL API (version 4.5.9.2019-02-01T07:24:44Z) https://github.com/owlcs/owlapi
